wip rebuilding invariants and simulation of [MsiSv]; this more generalized version will hopefully apply to other protocols as well.

src/Ex/MsiSvSim.v
@@ -3,7 +3,7 @@ Require Import Common FMap HVector Syntax Topology Semantics SemFacts StepM.
 Require Import Invariant TrsInv Simulation Serial SerialFacts.
 Require Import RqRsLang RqRsCorrect.
 
-Require Import Msi MsiSv SpecSv MsiSvTopo MsiSvInv.
+Require Import Msi MsiSv SpecSv MsiSvTopo (* MsiSvInv *).
 
 Set Implicit Arguments.
 
@@ -14,6 +14,19 @@ Open Scope list.
 Open Scope hvec.
 Open Scope fmap.
 
+(** TODO: move to [MsiSvInv.v] *)
+Ltac solve_msi :=
+  unfold msiM, msiS, msiI in *; lia.
+
+Ltac solve_DisjList :=
+  match goal with
+  | [ |- DisjList ?ll ?rl] =>
+    let e := fresh "e" in
+    red; intro e;
+    destruct (in_dec eq_nat_dec e ll); [right|auto];
+    dest_in; intro; dest_in; discriminate
+  end.
+
 Section Sim.
 
   Local Definition spec := SpecSv.spec 1.
@@ -21,24 +34,104 @@ Section Sim.
 
   (** Simulation between states *)
 
-  Definition SpecState (v: nat) (oss: OStates SpecOStateIfc)
-             (orqs: ORqs Msg): Prop :=
-    sost <-- oss@[specIdx];
-      sorq <-- orqs@[specIdx];
-      sost#[specValueIdx] = v.
+  Definition ImplOStateMSI (cv: nat) (ost: OState ImplOStateIfc): Prop :=
+    ost#[implStatusIdx] >= msiS -> ost#[implValueIdx] = cv.
 
-  Definition SimState (ioss: OStates ImplOStateIfc) (iorqs: ORqs Msg)
-             (soss: OStates SpecOStateIfc) (sorqs: ORqs Msg): Prop :=
-    cost1 <-- ioss@[child1Idx];
-      cost2 <-- ioss@[child2Idx];
-      corq1 <-- iorqs@[child1Idx];
-      corq2 <-- iorqs@[child2Idx];
-      (exists cv,
-          ImplChildCoh1 cost1 corq1 cv /\
-          ImplChildCoh2 cost2 corq2 cv /\
-          SpecState cv soss sorqs).
+  Section ImplCoh.
+    Variables (cv: nat)
+              (post cost1 cost2: OState ImplOStateIfc)
+              (porq corq1 corq2: ORq Msg)
+              (msgs: MessagePool Msg).
 
-  Definition SimMP (imsgs: MessagePool Msg) (iorqs: ORqs Msg)
+    Definition ParentCoh: Prop :=
+      ImplOStateMSI cv post.
+    Definition ImplChildCoh1: Prop :=
+      !corq1@[upRq]; ImplOStateMSI cv cost1.
+    Definition ImplChildCoh2: Prop :=
+      !corq2@[upRq]; ImplOStateMSI cv cost2.
+
+    Definition ImplOStateCoh: Prop :=
+      ParentCoh /\ ImplChildCoh1 /\ ImplChildCoh2.
+
+    Definition ImplMsgsCoh :=
+      forall idm,
+        InMPI msgs idm ->
+        match case (sigOf idm) on sig_dec default True with
+        | (pc1, (MRs, msiRsS)): (valOf idm).(msg_value) = VNat cv
+        | (pc2, (MRs, msiRsS)): (valOf idm).(msg_value) = VNat cv
+        | (c1pRs, (MRs, msiDownRsS)): (valOf idm).(msg_value) = VNat cv
+        | (c2pRs, (MRs, msiDownRsS)): (valOf idm).(msg_value) = VNat cv
+        | (c1pRq, (MRq, msiRqI)):
+            (cost1#[implStatusIdx] >= msiS -> (valOf idm).(msg_value) = VNat cv)
+        | (c2pRq, (MRq, msiRqI)):
+            (cost2#[implStatusIdx] >= msiS -> (valOf idm).(msg_value) = VNat cv)
+        end.
+             
+    Definition ImplCoh :=
+      ImplOStateCoh /\ ImplMsgsCoh.
+
+  End ImplCoh.
+
+  Definition ChildInvalid (cost: OState ImplOStateIfc) (corq: ORq Msg) :=
+    cost#[implStatusIdx] = msiI \/ corq@[upRq] <> None.
+
+  Definition ChildExcl (cost: OState ImplOStateIfc) (corq: ORq Msg) :=
+    cost#[implStatusIdx] = msiM /\ corq@[upRq] = None.
+
+  Section ImplExcl.
+    Variables (post cost1 cost2: OState ImplOStateIfc)
+              (porq corq1 corq2: ORq Msg)
+              (msgs: MessagePool Msg).
+
+    Definition ImplNoCohMsgs: Prop :=
+      forall idm,
+        InMPI msgs idm ->
+        match case (sigOf idm) on sig_dec default True with
+        | (pc1, (MRs, msiRsS)): False
+        | (pc2, (MRs, msiRsS)): False
+        | (c1pRs, (MRs, msiDownRsS)): False
+        | (c2pRs, (MRs, msiDownRsS)): False
+        | (c1pRq, (MRq, msiRqI)): cost1#[implStatusIdx] = msiI
+        | (c2pRq, (MRq, msiRqI)): cost2#[implStatusIdx] = msiI
+        end.
+
+    Definition ImplExcl: Prop :=
+      (ChildExcl cost1 corq1 ->
+       post#[implStatusIdx] = msiI /\ ChildInvalid cost2 corq2 /\ ImplNoCohMsgs) /\
+      (ChildExcl cost2 corq2 ->
+       post#[implStatusIdx] = msiI /\ ChildInvalid cost1 corq1 /\ ImplNoCohMsgs).
+
+  End ImplExcl.
+
+  Definition ImplStateCoh (cv: nat) (st: MState ImplOStateIfc): Prop :=
+    post <-- (bst_oss st)@[parentIdx];
+      cost1 <-- (bst_oss st)@[child1Idx];
+      cost2 <-- (bst_oss st)@[child2Idx];
+      corq1 <-- (bst_orqs st)@[child1Idx];
+      corq2 <-- (bst_orqs st)@[child2Idx];
+      ImplCoh cv post cost1 cost2 corq1 corq2 (bst_msgs st).
+
+  Definition ImplStateExcl (st: MState ImplOStateIfc): Prop :=
+    post <-- (bst_oss st)@[parentIdx];
+      cost1 <-- (bst_oss st)@[child1Idx];
+      cost2 <-- (bst_oss st)@[child2Idx];
+      corq1 <-- (bst_orqs st)@[child1Idx];
+      corq2 <-- (bst_orqs st)@[child2Idx];
+      ImplExcl post cost1 cost2 corq1 corq2 (bst_msgs st).
+
+  Definition SpecStateCoh (cv: nat) (st: MState SpecOStateIfc): Prop :=
+    sost <-- (bst_oss st)@[specIdx];
+      sorq <-- (bst_orqs st)@[specIdx];
+      sost#[specValueIdx] = cv.
+
+  Inductive SimState: MState ImplOStateIfc -> MState SpecOStateIfc -> Prop :=
+  | SimStateIntro:
+      forall cv ist sst,
+        SpecStateCoh cv sst ->
+        ImplStateCoh cv ist ->
+        SimState ist sst.
+
+  Definition SimExtMP (imsgs: MessagePool Msg) (iorqs: ORqs Msg)
              (smsgs: MessagePool Msg) :=
     corq1 <-- iorqs@[child1Idx];
       corq2 <-- iorqs@[child2Idx];
@@ -50,28 +143,48 @@ Section Sim.
       findQ ce2 imsgs = findQ (ers 1) smsgs.
   
   Definition SimMSI (ist: MState ImplOStateIfc) (sst: MState SpecOStateIfc): Prop :=
-    SimState ist.(bst_oss) ist.(bst_orqs) sst.(bst_oss) sst.(bst_orqs) /\
-    SimMP ist.(bst_msgs) ist.(bst_orqs) sst.(bst_msgs).
+    SimState ist sst /\
+    SimExtMP ist.(bst_msgs) ist.(bst_orqs) sst.(bst_msgs).
+
+  Hint Unfold ImplOStateMSI ParentCoh
+       ImplChildCoh1 ImplChildCoh2 ImplOStateCoh ImplCoh
+       ChildInvalid ChildExcl ImplExcl: RuleConds.
 
   Section Facts.
+
+    Lemma implNoCohMsgs_ImplMsgsCoh:
+      forall cost1 cost2 msgs,
+        ImplNoCohMsgs cost1 cost2 msgs ->
+        forall cv, ImplMsgsCoh cv cost1 cost2 msgs.
+    Proof.
+      unfold ImplNoCohMsgs, ImplMsgsCoh; intros.
+      specialize (H _ H0).
+      unfold caseDec in *.
+      repeat (find_if_inside; [exfalso; auto; fail|]).
+      find_if_inside; [intros; exfalso; rewrite H in H1; solve_msi|].
+      find_if_inside; [intros; exfalso; rewrite H in H1; solve_msi|].
+      auto.
+    Qed.
 
     Lemma simMsiSv_init:
       SimMSI (initsOf impl) (initsOf spec).
     Proof.
-      vm_compute.
       split.
-      - exists 0; repeat split.
+      - apply SimStateIntro with (cv:= 0).
+        + reflexivity.
+        + repeat split.
+          vm_compute; intros; exfalso; auto.
       - repeat split.
     Qed.
 
-    Lemma SimMP_enqMsgs:
+    Lemma SimExtMP_enqMsgs:
       forall eins,
         NoDup (idsOf eins) ->
         forall imsgs orqs smsgs,
-          SimMP imsgs orqs smsgs ->
-          SimMP (enqMsgs eins imsgs) orqs (enqMsgs eins smsgs).
+          SimExtMP imsgs orqs smsgs ->
+          SimExtMP (enqMsgs eins imsgs) orqs (enqMsgs eins smsgs).
     Proof.
-      unfold SimMP; intros.
+      unfold SimExtMP; intros.
       disc_rule_conds_ex.
       repeat split.
       - destruct (in_dec eq_nat_dec ec1 (idsOf eins)).
@@ -104,25 +217,25 @@ Section Sim.
           assumption.
     Qed.
 
-    Lemma SimMP_enqMP:
+    Lemma SimExtMP_enqMP:
       forall midx msg imsgs orqs smsgs,
-        SimMP imsgs orqs smsgs ->
-        SimMP (enqMP midx msg imsgs) orqs (enqMP midx msg smsgs).
+        SimExtMP imsgs orqs smsgs ->
+        SimExtMP (enqMP midx msg imsgs) orqs (enqMP midx msg smsgs).
     Proof.
       intros.
-      eapply SimMP_enqMsgs with (eins:= [(midx, msg)]) in H; auto.
+      eapply SimExtMP_enqMsgs with (eins:= [(midx, msg)]) in H; auto.
       repeat constructor; intro; dest_in.
     Qed.
 
-    Lemma SimMP_ext_outs_deqMsgs:
+    Lemma SimExtMP_ext_outs_deqMsgs:
       forall eouts,
         ValidMsgsExtOut impl eouts ->
         forall imsgs orqs smsgs,
           Forall (FirstMPI imsgs) eouts ->
-          SimMP imsgs orqs smsgs ->
-          SimMP (deqMsgs (idsOf eouts) imsgs) orqs (deqMsgs (idsOf eouts) smsgs).
+          SimExtMP imsgs orqs smsgs ->
+          SimExtMP (deqMsgs (idsOf eouts) imsgs) orqs (deqMsgs (idsOf eouts) smsgs).
     Proof.
-      unfold SimMP; intros.
+      unfold SimExtMP; intros.
       disc_rule_conds_ex.
       repeat split.
       - destruct (in_dec eq_nat_dec ec1 (idsOf eouts)).
@@ -171,15 +284,15 @@ Section Sim.
           assumption.
     Qed.
 
-    Lemma SimMP_ext_outs_FirstMPI:
+    Lemma SimExtMP_ext_outs_FirstMPI:
       forall eouts,
         ValidMsgsExtOut impl eouts ->
         forall imsgs orqs smsgs,
-          SimMP imsgs orqs smsgs ->
+          SimExtMP imsgs orqs smsgs ->
           Forall (FirstMPI imsgs) eouts ->
           Forall (FirstMPI smsgs) eouts.
     Proof.
-      unfold SimMP; intros.
+      unfold SimExtMP; intros.
       destruct H.
       disc_rule_conds_ex.
       apply Forall_forall; intros [midx msg] ?.
@@ -192,21 +305,21 @@ Section Sim.
         rewrite H4 in H1; assumption.
     Qed.
 
-    Lemma SimMP_outs_deqMP_child_1:
+    Lemma SimExtMP_outs_deqMP_child_1:
       forall msg imsgs (orqs: ORqs Msg) smsgs corq1,
         orqs@[child1Idx] = Some corq1 ->
         corq1@[upRq] = None ->
         FirstMPI imsgs (ec1, msg) ->
-        SimMP imsgs orqs smsgs ->
-        SimMP (deqMP ec1 imsgs) orqs (deqMP ec1 smsgs).
+        SimExtMP imsgs orqs smsgs ->
+        SimExtMP (deqMP ec1 imsgs) orqs (deqMP ec1 smsgs).
     Proof.
-      unfold SimMP; intros.
+      unfold SimExtMP; intros.
       disc_rule_conds_ex.
       repeat split;
         try (do 2 (rewrite findQ_not_In_deqMP by discriminate);
              assumption).
 
-      (* TODO: extract to a lemma? *)
+      (* extract to a lemma? *)
       clear -H2.
       unfold deqMP.
       rewrite H2.
@@ -216,21 +329,21 @@ Section Sim.
       - unfold findQ; mred.
     Qed.
       
-    Lemma SimMP_outs_deqMP_child_2:
+    Lemma SimExtMP_outs_deqMP_child_2:
       forall msg imsgs (orqs: ORqs Msg) smsgs corq2,
         orqs@[child2Idx] = Some corq2 ->
         corq2@[upRq] = None ->
         FirstMPI imsgs (ec2, msg) ->
-        SimMP imsgs orqs smsgs ->
-        SimMP (deqMP ec2 imsgs) orqs (deqMP ec2 smsgs).
+        SimExtMP imsgs orqs smsgs ->
+        SimExtMP (deqMP ec2 imsgs) orqs (deqMP ec2 smsgs).
     Proof.
-      unfold SimMP; intros.
+      unfold SimExtMP; intros.
       disc_rule_conds_ex.
       repeat split;
         try (do 2 (rewrite findQ_not_In_deqMP by discriminate);
              assumption).
 
-      (* TODO: extract to a lemma? *)
+      (* extract to a lemma? *)
       clear -H3.
       unfold deqMP.
       rewrite H3.
@@ -240,13 +353,13 @@ Section Sim.
       - unfold findQ; mred.
     Qed.
 
-    Lemma SimMP_impl_deqMP_indep:
+    Lemma SimExtMP_impl_deqMP_indep:
       forall midx imsgs (orqs: ORqs Msg) smsgs,
         ~ In midx [ce1; ce2; ec1; ec2] ->
-        SimMP imsgs orqs smsgs ->
-        SimMP (deqMP midx imsgs) orqs smsgs.
+        SimExtMP imsgs orqs smsgs ->
+        SimExtMP (deqMP midx imsgs) orqs smsgs.
     Proof.
-      unfold SimMP; intros.
+      unfold SimExtMP; intros.
       disc_rule_conds_ex.
       repeat split;
         try (rewrite findQ_not_In_deqMP
@@ -254,14 +367,14 @@ Section Sim.
              assumption).
     Qed.
 
-    Lemma SimMP_spec_deqMP_unlocked_1:
+    Lemma SimExtMP_spec_deqMP_unlocked_1:
       forall imsgs (orqs: ORqs Msg) smsgs porq1 norq1,
         orqs@[child1Idx] = Some porq1 ->
         porq1@[upRq] <> None -> norq1@[upRq] = None ->
-        SimMP imsgs orqs smsgs ->
-        SimMP imsgs (orqs +[child1Idx <- norq1]) (deqMP ec1 smsgs).
+        SimExtMP imsgs orqs smsgs ->
+        SimExtMP imsgs (orqs +[child1Idx <- norq1]) (deqMP ec1 smsgs).
     Proof.
-      unfold SimMP; intros.
+      unfold SimExtMP; intros.
       disc_rule_conds_ex.
       repeat split;
         try (rewrite findQ_not_In_deqMP by discriminate;
@@ -272,14 +385,14 @@ Section Sim.
       unfold findQ; mred.
     Qed.
 
-    Lemma SimMP_spec_deqMP_unlocked_2:
+    Lemma SimExtMP_spec_deqMP_unlocked_2:
       forall imsgs (orqs: ORqs Msg) smsgs porq2 norq2,
         orqs@[child2Idx] = Some porq2 ->
         porq2@[upRq] <> None -> norq2@[upRq] = None ->
-        SimMP imsgs orqs smsgs ->
-        SimMP imsgs (orqs +[child2Idx <- norq2]) (deqMP ec2 smsgs).
+        SimExtMP imsgs orqs smsgs ->
+        SimExtMP imsgs (orqs +[child2Idx <- norq2]) (deqMP ec2 smsgs).
     Proof.
-      unfold SimMP; intros.
+      unfold SimExtMP; intros.
       disc_rule_conds_ex.
       repeat split;
         try (rewrite findQ_not_In_deqMP by discriminate;
@@ -289,9 +402,184 @@ Section Sim.
       rewrite <-H2.
       unfold findQ; mred.
     Qed.
+
+    Lemma ImplMsgsCoh_other_enqMP:
+      forall cv cost1 cost2 msgs,
+        ImplMsgsCoh cv cost1 cost2 msgs ->
+        forall midx msg,
+          ~ In midx [pc1; pc2; c1pRs; c2pRs; c1pRq; c2pRq] ->
+          ImplMsgsCoh cv cost1 cost2 (enqMP midx msg msgs).
+    Proof.
+    Admitted.
+
+    Lemma ImplMsgsCoh_other_enqMsgs:
+      forall cv cost1 cost2 msgs,
+        ImplMsgsCoh cv cost1 cost2 msgs ->
+        forall eins minds,
+          SubList (idsOf eins) minds ->
+          DisjList minds [pc1; pc2; c1pRs; c2pRs; c1pRq; c2pRq] ->
+          ImplMsgsCoh cv cost1 cost2 (enqMsgs eins msgs).
+    Proof.
+      intros.
+      generalize dependent msgs.
+      induction eins as [|ein eins]; simpl; intros; [assumption|].
+      simpl in H0; apply SubList_cons_inv in H0; dest.
+      destruct ein as [midx msg]; simpl in *.
+      eapply IHeins; eauto.
+      apply ImplMsgsCoh_other_enqMP; auto.
+      eapply DisjList_In_2; eauto.
+    Qed.
+
+    Lemma ImplMsgsCoh_deqMP:
+      forall cv cost1 cost2 msgs,
+        ImplMsgsCoh cv cost1 cost2 msgs ->
+        forall midx,
+          ImplMsgsCoh cv cost1 cost2 (deqMP midx msgs).
+    Proof.
+      unfold ImplMsgsCoh; intros.
+      apply InMP_deqMP in H0; auto.
+    Qed.
+
+    Lemma ImplMsgsCoh_other_deqMsgs:
+      forall cv cost1 cost2 msgs,
+        ImplMsgsCoh cv cost1 cost2 msgs ->
+        forall minds,
+          ImplMsgsCoh cv cost1 cost2 (deqMsgs minds msgs).
+    Proof.
+      unfold ImplMsgsCoh; intros.
+      apply InMP_deqMsgs in H0; auto.
+    Qed.
+
+    Lemma SimState_impl_ext_enqMsgs:
+      forall ioss iorqs imsgs sst,
+        SimState {| bst_oss := ioss; bst_orqs := iorqs; bst_msgs := imsgs |} sst ->
+        forall nmsgs,
+          SubList (idsOf nmsgs) (sys_merqs impl) ->
+          SimState {| bst_oss := ioss; bst_orqs := iorqs;
+                      bst_msgs := enqMsgs nmsgs imsgs |} sst.
+    Proof.
+      intros.
+      inv H.
+      apply SimStateIntro with (cv:= cv); [assumption|].
+      clear H1.
+      red in H2; red; simpl in *.
+      disc_rule_conds_ex.
+      repeat split; try assumption.
+      eapply ImplMsgsCoh_other_enqMsgs; eauto.
+      solve_DisjList.
+    Qed.
+
+    Lemma SimState_spec_enqMsgs:
+      forall ist soss sorqs smsgs,
+        SimState ist {| bst_oss := soss; bst_orqs := sorqs; bst_msgs := smsgs |} ->
+        forall nmsgs,
+          SimState ist {| bst_oss := soss; bst_orqs := sorqs;
+                          bst_msgs := enqMsgs nmsgs smsgs |}.
+    Proof.
+      intros.
+      inv H.
+      econstructor; eauto.
+    Qed.
+
+    Lemma SimState_impl_deqMsgs:
+      forall ioss iorqs imsgs sst,
+        SimState {| bst_oss := ioss; bst_orqs := iorqs; bst_msgs := imsgs |} sst ->
+        forall minds,
+          SimState {| bst_oss := ioss; bst_orqs := iorqs;
+                      bst_msgs := deqMsgs minds imsgs |} sst.
+    Proof.
+      intros.
+      inv H.
+      apply SimStateIntro with (cv:= cv); [assumption|].
+      clear H0.
+      red in H1; red; simpl in *.
+      disc_rule_conds_ex.
+      repeat split; try assumption.
+      clear -H0.
+      red in H0; red; intros.
+      apply InMP_deqMsgs in H; auto.
+    Qed.
+
+    Lemma SimState_spec_deqMsgs:
+      forall ist soss sorqs smsgs,
+        SimState ist {| bst_oss := soss; bst_orqs := sorqs; bst_msgs := smsgs |} ->
+        forall minds,
+          SimState ist {| bst_oss := soss; bst_orqs := sorqs;
+                          bst_msgs := deqMsgs minds smsgs |}.
+    Proof.
+      intros.
+      inv H.
+      econstructor; eauto.
+    Qed.
+
+    Ltac spec_constr_step_get_FirstMPI :=
+      repeat constructor;
+      match goal with
+      | [H: SimExtMP _ _ _ |- _] => red in H; disc_rule_conds_const; dest
+      end;
+      eapply findQ_eq_FirstMPI; eauto.
+
+    Ltac spec_constr_step_get_ValidMsgs :=
+      clear; split;
+      [simpl; apply SubList_cons; [|apply SubList_nil];
+       simpl; tauto
+      |repeat constructor; intro; dest_in].
+
+    Ltac spec_constr_step_get ecmidx :=
+      match goal with
+      | [H: msg_id ?msg = Spec.getRq |- _] =>
+        eapply SmInt with (obj:= specObj 1) (ins:= [(ecmidx, msg)]);
+        try reflexivity;
+        [left; reflexivity (* object in *)
+        |simpl; tauto (* rule in *)
+        |eassumption
+        |eassumption
+        |spec_constr_step_get_FirstMPI
+        |spec_constr_step_get_ValidMsgs
+        |solve_rule_conds_ex (* rule_precond *)
+        |spec_constr_step_get_ValidMsgs
+        |solve_DisjList]
+      end.
+
+    Ltac spec_constr_step_set ecmidx :=
+      match goal with
+      | [H: msg_id ?msg = Spec.setRq |- _] =>
+        eapply SmInt with (obj:= specObj 1) (ins:= [(ecmidx, msg)]);
+        try reflexivity;
+        [left; reflexivity (* object in *)
+        |simpl; tauto (* rule in *)
+        |eassumption
+        |eassumption
+        |spec_constr_step_get_FirstMPI
+        |spec_constr_step_get_ValidMsgs
+        |solve_rule_conds_ex (* rule_precond *)
+        |spec_constr_step_get_ValidMsgs
+        |solve_DisjList]
+      end.
+
+    Ltac spec_case_get cidx ecmidx :=
+      eexists (RlblInt 0 (rule_idx (specGetRq cidx)) _ _); eexists;
+      repeat ssplit;
+      [reflexivity
+      |spec_constr_step_get ecmidx
+      |].
+
+    Ltac spec_case_set cidx ecmidx :=
+      eexists (RlblInt 0 (rule_idx (specSetRq cidx)) _ _); eexists;
+      repeat ssplit;
+      [reflexivity
+      |spec_constr_step_set ecmidx
+      |].
     
+    Ltac spec_case_silent cidx ecmidx :=
+      idtac; exists (RlblEmpty _); eexists;
+      repeat ssplit;
+      [reflexivity
+      |econstructor
+      |].
+
     Lemma simMsiSv_sim:
-      InvSim step_m step_m ImplInv SimMSI impl spec.
+      InvSim step_m step_m ImplStateExcl SimMSI impl spec.
     Proof.
       red; intros.
       inv H2.
@@ -306,9 +594,12 @@ Section Sim.
         repeat ssplit.
         + reflexivity.
         + eapply SmIns; eauto.
-        + split; [assumption|].
-          apply SimMP_enqMsgs; auto.
-          apply H5.
+        + split.
+          * apply SimState_spec_enqMsgs.
+            apply SimState_impl_ext_enqMsgs; [assumption|].
+            apply H5.
+          * apply SimExtMP_enqMsgs; auto.
+            apply H5.
 
       - destruct sst1 as [soss1 sorqs1 smsgs1]; simpl in *.
         destruct H0; simpl in *.
@@ -316,9 +607,12 @@ Section Sim.
         repeat ssplit.
         + reflexivity.
         + eapply SmOuts with (msgs0:= smsgs1); eauto.
-          eapply SimMP_ext_outs_FirstMPI; eauto.
-        + split; [assumption|].
-          apply SimMP_ext_outs_deqMsgs; auto.
+          eapply SimExtMP_ext_outs_FirstMPI; eauto.
+        + split.
+          * apply SimState_spec_deqMsgs.
+            apply SimState_impl_deqMsgs.
+            assumption.
+          * apply SimExtMP_ext_outs_deqMsgs; auto.
 
       - pose proof (footprints_ok
                       msiSv_impl_ORqsInit
@@ -326,120 +620,228 @@ Section Sim.
 
         destruct sst1 as [soss1 sorqs1 smsgs1].
         destruct H0; simpl in H0, H2; simpl.
-        red in H0; disc_rule_conds_const.
-        destruct H0 as [cv ?]; dest.
-        red in H15; disc_rule_conds_const.
+        inv H0.
+        red in H15; simpl in H15.
+        destruct (oss@[parentIdx]) as [post|] eqn:Hpost; simpl in *; [|exfalso; auto].
+        destruct (oss@[child1Idx]) as [cost1|] eqn:Hcost1; simpl in *; [|exfalso; auto].
+        destruct (oss@[child2Idx]) as [cost2|] eqn:Hcost2; simpl in *; [|exfalso; auto].
+        destruct (orqs@[child1Idx]) as [corq1|] eqn:Hcorq1; simpl in *; [|exfalso; auto].
+        destruct (orqs@[child2Idx]) as [corq2|] eqn:Hcorq2; simpl in *; [|exfalso; auto].
+        red in H6; simpl in H6.
+        destruct (soss1@[specIdx]) as [sost|] eqn:Hsost; simpl in *; [|exfalso; auto].
+        destruct (sorqs1@[specIdx]) as [sorq|] eqn:Hsorq; simpl in *; [|exfalso; auto].
+        dest; subst.
+        
         destruct H4 as [|[|[|]]];
           try (exfalso; auto; fail); subst; dest_in.
 
         + (** [childGetRqImm] *)
           disc_rule_conds_ex.
-          eexists (RlblInt 0 (rule_idx (specGetRq 0)) _ _); eexists.
-          repeat ssplit.
-          * reflexivity.
-          * eapply SmInt with (obj:= specObj 1);
-              try reflexivity; try eassumption.
-            { left; reflexivity. }
-            { simpl; tauto. }
-            { instantiate (1:= [(ec1, rmsg)]).
-              repeat constructor.
-              red in H2; disc_rule_conds_ex.
-              eapply findQ_eq_FirstMPI; eauto.
-            }
-            { split.
-              { simpl; apply SubList_cons; [|apply SubList_nil].
-                simpl; tauto.
+          spec_case_get 0 ec1.
+
+          red; simpl; split.
+          * eapply SimStateIntro with (cv:= fst sost).
+            { solve_rule_conds_ex. }
+            { red; simpl.
+              disc_rule_conds_ex.
+              split.
+              { solve_rule_conds_ex. }
+              { apply ImplMsgsCoh_other_enqMP;
+                  [|intro; dest_in; discriminate].
+                apply ImplMsgsCoh_deqMP.
+                assumption.
               }
-              { repeat constructor; intro Hx; dest_in. }
             }
-            { solve_rule_conds_ex. }
-            { clear; solve_rule_conds_ex.
-              { simpl; tauto. }
-              { repeat constructor; intro Hx; dest_in. }
-            }
-            { disc_rule_conds_ex. }
-          * red; simpl; split.
-            { solve_rule_conds_ex. }
-            { replace (orqs +[child1Idx <- norq]) with orqs by meq.
-              specialize (H0 eq_refl H15); rewrite H0.
-              apply SimMP_enqMP.
-              eapply SimMP_outs_deqMP_child_1; eauto.
-            }
+          * replace (orqs +[child1Idx <- norq]) with orqs by meq.
+            specialize (H5 eq_refl H19); rewrite H5.
+            apply SimExtMP_enqMP.
+            eapply SimExtMP_outs_deqMP_child_1; eauto.
 
         + (** [childGetRqS] *)
-          admit.
+          disc_rule_conds_ex.
+          spec_case_silent 0 ec1.
+                    
+          red; simpl; split.
+          * eapply SimStateIntro with (cv:= fst sost).
+            { solve_rule_conds_ex. }
+            { red; simpl.
+              disc_rule_conds_ex.
+              split.
+              { solve_rule_conds_ex. }
+              { admit. }
+            }
+          * admit.
 
         + (** [childGetRsS] *)
           disc_rule_conds_ex.
-          eexists (RlblInt 0 (rule_idx (specGetRq 0)) _ _); eexists.
-          repeat ssplit.
-          * reflexivity.
-          * eapply SmInt with (obj:= specObj 1);
-              try reflexivity; try eassumption.
-            { left; reflexivity. }
-            { simpl; tauto. }
-            { instantiate (1:= [(ec1, rqi_msg rqi)]).
-              repeat constructor.
-              red in H2.
-              disc_rule_conds_ex.
-              clear -H2.
-              unfold FirstMPI, FirstMP, firstMP; simpl.
-              unfold ec1.
-              rewrite <-H2.
-              reflexivity.
-            }
-            { split.
-              { simpl; apply SubList_cons; [|apply SubList_nil].
-                simpl; tauto.
-              }
-              { repeat constructor; intro Hx; dest_in. }
-            }
+          spec_case_get 0 ec1;
+            [unfold FirstMPI, FirstMP, firstMP;
+             simpl; change ec1 with (erq 0);
+             rewrite <-H2; reflexivity|].
+          
+          good_footprint_get child1Idx.
+          destruct H15 as [rqFrom [rqTo [rsFrom [rsbTo ?]]]]; dest.
+          disc_rule_conds_ex.
+          pose proof (parentIdxOf_child_indsOf _ _ H23).
+          dest_in; try discriminate; simpl in *.
+          inv H26; inv H27.
+
+          assert (n = fst sost).
+          { specialize (H4 _ (FirstMP_InMP H20)).
+            unfold sigOf, valOf, snd in H4.
+            rewrite H21, H22 in H4; simpl in H4.
+            congruence.
+          }
+          subst.
+
+          red; simpl; split.
+          * eapply SimStateIntro with (cv:= fst sost).
             { solve_rule_conds_ex. }
-            { clear; solve_rule_conds_ex.
-              { simpl; tauto. }
-              { repeat constructor; intro Hx; dest_in. }
-            }
-            { disc_rule_conds_ex.
-              (** TODO: develop [solve_sublist] and [solve_disjlist]. *)
-              red; intro e.
-              destruct (in_dec eq_nat_dec e [ec1]); [right|auto].
-              dest_in; intro; dest_in; discriminate.
-            }
-          * red; simpl; split.
-            { (** TODO: need to know the response message value is
-               *  coherent as well. This is part of predicate messages but
-               *  [ImplStateInv] does not contain it.
-               *)
-              admit.
-            }
-            { replace (fst ost1) with n by admit.
-              good_footprint_get child1Idx.
-              red in H9.
-              destruct H9 as [rqFrom [rqTo [rsFrom [rsbTo ?]]]]; dest.
+            { red; simpl.
               disc_rule_conds_ex.
-              pose proof (parentIdxOf_child_indsOf _ _ H19).
-              dest_in; try discriminate; simpl in *.
-              inv H22; inv H23.
-              apply SimMP_enqMP.
-              apply SimMP_impl_deqMP_indep; [intro Hx; dest_in; discriminate|].
-              eapply SimMP_spec_deqMP_unlocked_1; eauto.
-              { congruence. }
-              { mred. }
+              split.
+              { solve_rule_conds_ex. }
+              { admit. }
             }
+          * apply SimExtMP_enqMP.
+            apply SimExtMP_impl_deqMP_indep; [intro Hx; dest_in; discriminate|].
+            eapply SimExtMP_spec_deqMP_unlocked_1; eauto.
+            { congruence. }
+            { mred. }
 
         + (** [childDownRqS] *)
+          disc_rule_conds_ex.
+          spec_case_silent 0 ec1.
+                    
+          red; simpl; split.
+          * eapply SimStateIntro with (cv:= fst sost).
+            { solve_rule_conds_ex. }
+            { red; simpl.
+              disc_rule_conds_ex.
+              split.
+              { solve_rule_conds_ex.
+                apply H5; auto.
+              }
+              { admit. }
+            }
+          * admit.
 
+        + (** [childSetRqImm] *)
+          disc_rule_conds_ex.
+          spec_case_set 0 ec1.
+
+          (* discharging [ImplStateExcl] *)
+          red in H3; simpl in H3.
+          disc_rule_conds_ex.
+          specialize (H3 (conj eq_refl eq_refl)); dest.
+
+          red; simpl; split.
+          * eapply SimStateIntro with (cv:= n).
+            { rewrite Hmsg.
+              solve_rule_conds_ex.
+            }
+            { red; simpl.
+              disc_rule_conds_ex.
+              split.
+              { solve_rule_conds_ex.
+                { solve_msi. }
+                { destruct H12; [solve_msi|exfalso; auto]. }
+              }
+              { apply implNoCohMsgs_ImplMsgsCoh; assumption. }
+            }
+          * replace (orqs +[child1Idx <- norq]) with orqs by meq.
+            apply SimExtMP_enqMP.
+            eapply SimExtMP_outs_deqMP_child_1; eauto.
+          
+        + (** [childSetRqM] *)
+          disc_rule_conds_ex.
+          spec_case_silent 0 ec1.
+                    
+          red; simpl; split.
+          * eapply SimStateIntro with (cv:= fst sost).
+            { solve_rule_conds_ex. }
+            { red; simpl.
+              disc_rule_conds_ex.
+              split.
+              { solve_rule_conds_ex. }
+              { admit. }
+            }
+          * admit.
+          
+        + (** [childSetRsM] *)
+          disc_rule_conds_ex.
+          spec_case_set 0 ec1;
+            [unfold FirstMPI, FirstMP, firstMP;
+             simpl; change ec1 with (erq 0);
+             rewrite <-H2; reflexivity|].
+
+          (* discharging [ImplStateExcl] *)
+          red in H3; simpl in H3.
+          disc_rule_conds_ex.
+          specialize (H3 (conj eq_refl eq_refl)); dest.
+
+          red; simpl; split.
+          * eapply SimStateIntro with (cv:= n).
+            { rewrite Hmsg.
+              solve_rule_conds_ex.
+            }
+            { red; simpl.
+              disc_rule_conds_ex.
+              split.
+              { solve_rule_conds_ex.
+                { solve_msi. }
+                { destruct H18; [solve_msi|exfalso; auto]. }
+              }
+              { apply implNoCohMsgs_ImplMsgsCoh; assumption. }
+            }
+          * admit.
+
+        + (** [childDownRqI] *)
+          disc_rule_conds_ex.
+          spec_case_silent 0 ec1.
+                    
+          red; simpl; split.
+          * eapply SimStateIntro with (cv:= fst sost).
+            { solve_rule_conds_ex. }
+            { red; simpl.
+              disc_rule_conds_ex.
+              split.
+              { solve_rule_conds_ex.
+                apply H5; auto.
+              }
+              { admit. }
+            }
+          * admit.
+
+        + (** [childEvictRqI] *)
+          disc_rule_conds_ex.
+          spec_case_silent 0 ec1.
+
+          red; simpl; split.
+          * eapply SimStateIntro with (cv:= fst sost).
+            { solve_rule_conds_ex. }
+            { red; simpl.
+              disc_rule_conds_ex.
+              split.
+              { solve_rule_conds_ex. }
+              { admit. }
+            }
+          * admit.
+
+        + (** [childEvictRsI] *)
+          admit.
+          
     Admitted.
     
     Theorem MsiSv_ok:
       (steps step_m) # (steps step_m) |-- impl ⊑ spec.
     Proof.
-      apply invSim_implies_refinement with (ginv:= ImplInv) (sim:= SimMSI).
+      apply invSim_implies_refinement with (ginv:= ImplStateExcl) (sim:= SimMSI).
       - apply simMsiSv_sim.
-      - apply implInv_invStep.
+      - admit.
       - apply simMsiSv_init.
-      - apply implInv_init.
-    Qed.
+      - admit.
+    Admitted.
 
   End Facts.
   
