src/Ex/MsiSvInv.v
@@ -72,24 +72,6 @@ Ltac atomic_init_exfalso_rs_from_parent :=
 Ltac atomic_init_solve_AtomicMsgOutsInv :=
   simpl; repeat constructor.
 
-(* Ltac atomic_init_solve_AtomicLocksInv := *)
-(*   red; intros; dest_in; *)
-(*   repeat (simpl; mred); *)
-(*   unfold sigOf; simpl; *)
-(*   repeat *)
-(*     match goal with *)
-(*     | [H: msg_id ?msg = _ |- context [msg_id ?msg] ] => rewrite H *)
-(*     | [H1: msg_id ?msg = _, H2: context [msg_id ?msg] |- _] => *)
-(*       rewrite H1 in H2 *)
-(*     | [H: ?orq@[?i] = Some _ |- context [?orq@[?i]] ] => rewrite H *)
-(*     | [H1: ?orq@[?i] = Some _, H2: context [?orq@[?i]] |- _] => *)
-(*       rewrite H1 in H2 *)
-(*     | [H: ?orq@[?i] = None |- context [?orq@[?i]] ] => rewrite H *)
-(*     | [H1: ?orq@[?i] = None, H2: context [?orq@[?i]] |- _] => *)
-(*       rewrite H1 in H2 *)
-(*     end; *)
-(*   repeat (red; simpl; mred; auto). *)
-
 Ltac atomic_init_solve_AtomicInv :=
   atomic_init_solve_AtomicMsgOutsInv.
 
@@ -123,1850 +105,1843 @@ Ltac disc_msg_preds Hin :=
     disc_msg_preds_with Hl Hin
   end.
 
-Section Inv.
+(* Section Inv. *)
 
-  (** Basic predicates per an object *)
-  
-  Definition ImplOStateM (cv: nat) (ost: OState ImplOStateIfc): Prop :=
-    ost#[implStatusIdx] = msiM /\ ost#[implValueIdx] = cv.
+(*   (** Basic predicates per an object *) *)
 
-  Definition ImplOStateS (cv: nat) (ost: OState ImplOStateIfc): Prop :=
-    ost#[implStatusIdx] = msiS /\ ost#[implValueIdx] = cv.
+(*   Definition ImplOStateM (cv: nat) (ost: OState ImplOStateIfc): Prop := *)
+(*     ost#[implStatusIdx] = msiM /\ ost#[implValueIdx] = cv. *)
 
-  Definition ImplOStateI (ost: OState ImplOStateIfc): Prop :=
-    ost#[implStatusIdx] = msiI.
+(*   Definition ImplOStateS (cv: nat) (ost: OState ImplOStateIfc): Prop := *)
+(*     ost#[implStatusIdx] = msiS /\ ost#[implValueIdx] = cv. *)
 
-  Definition ImplOStateMSI (cv: nat) (ost: OState ImplOStateIfc): Prop :=
-    ost#[implStatusIdx] >= msiS -> ost#[implValueIdx] = cv.
+(*   Definition ImplOStateI (ost: OState ImplOStateIfc): Prop := *)
+(*     ost#[implStatusIdx] = msiI. *)
 
-  Definition ImplDirM (ost: OState ImplOStateIfc): Prop :=
-    (ost#[implDirIdx].(fst) = msiM /\ ost#[implDirIdx].(snd) = msiI) \/
-    (ost#[implDirIdx].(fst) = msiI /\ ost#[implDirIdx].(snd) = msiM).
+(*   Definition ImplOStateMSI (cv: nat) (ost: OState ImplOStateIfc): Prop := *)
+(*     ost#[implStatusIdx] >= msiS -> ost#[implValueIdx] = cv. *)
 
-  Definition ImplDirS (ost: OState ImplOStateIfc): Prop :=
-    ost#[implDirIdx].(fst) <= msiS /\
-    ost#[implDirIdx].(snd) <= msiS.
+(*   Definition ImplDirM (ost: OState ImplOStateIfc): Prop := *)
+(*     (ost#[implDirIdx].(fst) = msiM /\ ost#[implDirIdx].(snd) = msiI) \/ *)
+(*     (ost#[implDirIdx].(fst) = msiI /\ ost#[implDirIdx].(snd) = msiM). *)
 
-  Definition ImplDirI (ost: OState ImplOStateIfc): Prop :=
-    ost#[implDirIdx].(fst) = msiI /\
-    ost#[implDirIdx].(snd) = msiI.
+(*   Definition ImplDirS (ost: OState ImplOStateIfc): Prop := *)
+(*     ost#[implDirIdx].(fst) <= msiS /\ *)
+(*     ost#[implDirIdx].(snd) <= msiS. *)
 
-  Section GInv.
-    Variables (post cost1 cost2: OState ImplOStateIfc)
-              (porq corq1 corq2: ORq Msg).
+(*   Definition ImplDirI (ost: OState ImplOStateIfc): Prop := *)
+(*     ost#[implDirIdx].(fst) = msiI /\ *)
+(*     ost#[implDirIdx].(snd) = msiI. *)
 
-    (** The first invariant: the directory status is coherent to statuses of
-     * children. Note that an object is *not* required to keep the coherency
-     * when it is (properly) locked (the meaning of "properly" depends on the
-     * protocol).
-     *)
-    Definition ImplDirCoh: Prop :=
-      (!corq1@[upRq]; cost1#[implStatusIdx] <= post#[implDirIdx].(fst)) /\
-      (!corq2@[upRq]; cost2#[implStatusIdx] <= post#[implDirIdx].(snd)).
+(*   Section GInv. *)
+(*     Variables (post cost1 cost2: OState ImplOStateIfc) *)
+(*               (porq corq1 corq2: ORq Msg). *)
+
+(*     (** The first invariant: the directory status is coherent to statuses of *)
+(*      * children. Note that an object is *not* required to keep the coherency *)
+(*      * when it is (properly) locked (the meaning of "properly" depends on the *)
+(*      * protocol). *)
+(*      *) *)
+(*     Definition ImplDirCoh: Prop := *)
+(*       (!corq1@[upRq]; cost1#[implStatusIdx] <= post#[implDirIdx].(fst)) /\ *)
+(*       (!corq2@[upRq]; cost2#[implStatusIdx] <= post#[implDirIdx].(snd)). *)
     
-    (** The second invariant is only for parent, saying that the parent status
-     * and its directory status are coherent.
-     *)
-    Definition ImplParentCoh (cv: nat): Prop :=
-      (ImplOStateM cv post /\ ImplDirI post) \/
-      (ImplOStateS cv post /\ ImplDirS post) \/
-      (ImplOStateI post /\ ImplDirM post).
+(*     (** The second invariant is only for parent, saying that the parent status *)
+(*      * and its directory status are coherent. *)
+(*      *) *)
+(*     Definition ImplParentCoh (cv: nat): Prop := *)
+(*       (ImplOStateM cv post /\ ImplDirI post) \/ *)
+(*       (ImplOStateS cv post /\ ImplDirS post) \/ *)
+(*       (ImplOStateI post /\ ImplDirM post). *)
 
-    (** The last invariant is for children, in order for ensuring
-     * the local coherency. 
-     *)
-    Definition ImplChildCoh1 (cv: nat): Prop :=
-      !corq1@[upRq]; ImplOStateMSI cv cost1.
-    Definition ImplChildCoh2 (cv: nat): Prop :=
-      !corq2@[upRq]; ImplOStateMSI cv cost2.
+(*     (** The last invariant is for children, in order for ensuring *)
+(*      * the local coherency.  *)
+(*      *) *)
+(*     Definition ImplChildCoh1 (cv: nat): Prop := *)
+(*       !corq1@[upRq]; ImplOStateMSI cv cost1. *)
+(*     Definition ImplChildCoh2 (cv: nat): Prop := *)
+(*       !corq2@[upRq]; ImplOStateMSI cv cost2. *)
 
-    Definition ImplChildrenCoh: Prop :=
-      !corq1@[upRq]; !corq2@[upRq];
-        (cost1#[implStatusIdx] = msiM -> cost2#[implStatusIdx] = msiI) /\
-        (cost2#[implStatusIdx] = msiM -> cost1#[implStatusIdx] = msiI).
+(*     Definition ImplChildrenCoh: Prop := *)
+(*       !corq1@[upRq]; !corq2@[upRq]; *)
+(*         (cost1#[implStatusIdx] = msiM -> cost2#[implStatusIdx] = msiI) /\ *)
+(*         (cost2#[implStatusIdx] = msiM -> cost1#[implStatusIdx] = msiI). *)
   
-    Definition ImplStateCoh (cv: nat): Prop :=
-      ImplParentCoh cv /\ 
-      ImplChildCoh1 cv /\ ImplChildCoh2 cv /\
-      ImplChildrenCoh.
+(*     Definition ImplStateCoh (cv: nat): Prop := *)
+(*       ImplParentCoh cv /\  *)
+(*       ImplChildCoh1 cv /\ ImplChildCoh2 cv /\ *)
+(*       ImplChildrenCoh. *)
 
-    Definition ImplParentLockInv: Prop :=
-      rqid <+- porq@[downRq];
-        ((rqid.(rqi_minds_rss) = [c2pRs] /\ rqid.(rqi_midx_rsb) = pc1) \/
-         (rqid.(rqi_minds_rss) = [c1pRs] /\ rqid.(rqi_midx_rsb) = pc2)).
+(*     Definition ImplParentLockInv: Prop := *)
+(*       rqid <+- porq@[downRq]; *)
+(*         ((rqid.(rqi_minds_rss) = [c2pRs] /\ rqid.(rqi_midx_rsb) = pc1) \/ *)
+(*          (rqid.(rqi_minds_rss) = [c1pRs] /\ rqid.(rqi_midx_rsb) = pc2)). *)
     
-  End GInv.
+(*   End GInv. *)
 
-  Definition ImplStateInv (st: MState ImplOStateIfc): Prop :=
-    post <-- (bst_oss st)@[parentIdx];
-      cost1 <-- (bst_oss st)@[child1Idx];
-      cost2 <-- (bst_oss st)@[child2Idx];
-      corq1 <-- (bst_orqs st)@[child1Idx];
-      corq2 <-- (bst_orqs st)@[child2Idx];
-      (exists cv, ImplStateCoh post cost1 cost2 corq1 corq2 cv) /\
-      ImplDirCoh post cost1 cost2 corq1 corq2.
+(*   Definition ImplStateInv (st: MState ImplOStateIfc): Prop := *)
+(*     post <-- (bst_oss st)@[parentIdx]; *)
+(*       cost1 <-- (bst_oss st)@[child1Idx]; *)
+(*       cost2 <-- (bst_oss st)@[child2Idx]; *)
+(*       corq1 <-- (bst_orqs st)@[child1Idx]; *)
+(*       corq2 <-- (bst_orqs st)@[child2Idx]; *)
+(*       (exists cv, ImplStateCoh post cost1 cost2 corq1 corq2 cv) /\ *)
+(*       ImplDirCoh post cost1 cost2 corq1 corq2. *)
 
-  Definition ImplLockInv (st: MState ImplOStateIfc): Prop :=
-    porq <-- (bst_orqs st)@[parentIdx];
-      ImplParentLockInv porq.
+(*   Definition ImplLockInv (st: MState ImplOStateIfc): Prop := *)
+(*     porq <-- (bst_orqs st)@[parentIdx]; *)
+(*       ImplParentLockInv porq. *)
 
-  Definition ImplInv (st: MState ImplOStateIfc): Prop :=
-    ImplStateInv st /\ ImplLockInv st.
+(*   Definition ImplInv (st: MState ImplOStateIfc): Prop := *)
+(*     ImplStateInv st /\ ImplLockInv st. *)
 
-  Hint Unfold ImplOStateM ImplOStateS ImplOStateI ImplOStateMSI
-       ImplDirM ImplDirS ImplDirI
-       ImplDirCoh ImplParentCoh ImplChildCoh1 ImplChildCoh2 ImplChildrenCoh
-       ImplStateCoh: RuleConds.
+(*   Hint Unfold ImplOStateM ImplOStateS ImplOStateI ImplOStateMSI *)
+(*        ImplDirM ImplDirS ImplDirI *)
+(*        ImplDirCoh ImplParentCoh ImplChildCoh1 ImplChildCoh2 ImplChildrenCoh *)
+(*        ImplStateCoh: RuleConds. *)
 
-  Ltac disc_msi :=
-    try
-      match goal with
-      | [H: ?t = ?t -> _ |- _] => specialize (H eq_refl)
-      | [H: ?p -> _, Hp: ?p |- _] => specialize (H Hp)
-      | [H: VNat ?v = VNat _ |- _] => is_var v; inv H
-      | [H: VNat _ = VNat ?v |- _] => is_var v; inv H
-      | [H: ?oss@[parentIdx] = Some ?ost |- _] =>
-        match type of ost with
-        | OState _ =>
-          let val := fresh "val" in
-          let stt := fresh "stt" in
-          let dir := fresh "dir" in
-          destruct ost as [val [stt [dir ?]]]
-        end
-      | [H: ?oss@[child1Idx] = Some ?ost |- _] =>
-        match type of ost with
-        | OState _ =>
-          let val := fresh "val" in
-          let stt := fresh "stt" in
-          destruct ost as [val [stt ?]]
-        end
-      | [H: ?oss@[child2Idx] = Some ?ost |- _] =>
-        match type of ost with
-        | OState _ =>
-          let val := fresh "val" in
-          let stt := fresh "stt" in
-          destruct ost as [val [stt ?]]
-        end
-      | [H: msiM = _ |- _] => apply eq_sym in H
-      | [H: msiS = _ |- _] => apply eq_sym in H
-      | [H: msiI = _ |- _] => apply eq_sym in H
-      | [H1: ?t = msiM, H2: ?t = msiS |- _] => rewrite H1 in H2; discriminate
-      | [H1: ?t = msiM, H2: ?t = msiI |- _] => rewrite H1 in H2; discriminate
-      | [H1: ?t = msiS, H2: ?t = msiI |- _] => rewrite H1 in H2; discriminate
-      | [H1: ?t = msiM, H2: ?t <= msiS |- _] =>
-        rewrite H1 in H2; unfold msiM, msiS in H2; lia
-      | [H1: ?t = msiI, H2: ?t >= msiS |- _] =>
-        rewrite H1 in H2; unfold msiS, msiI in H2; lia
-      end.
+(*   Ltac disc_msi := *)
+(*     try *)
+(*       match goal with *)
+(*       | [H: ?t = ?t -> _ |- _] => specialize (H eq_refl) *)
+(*       | [H: ?p -> _, Hp: ?p |- _] => specialize (H Hp) *)
+(*       | [H: VNat ?v = VNat _ |- _] => is_var v; inv H *)
+(*       | [H: VNat _ = VNat ?v |- _] => is_var v; inv H *)
+(*       | [H: ?oss@[parentIdx] = Some ?ost |- _] => *)
+(*         match type of ost with *)
+(*         | OState _ => *)
+(*           let val := fresh "val" in *)
+(*           let stt := fresh "stt" in *)
+(*           let dir := fresh "dir" in *)
+(*           destruct ost as [val [stt [dir ?]]] *)
+(*         end *)
+(*       | [H: ?oss@[child1Idx] = Some ?ost |- _] => *)
+(*         match type of ost with *)
+(*         | OState _ => *)
+(*           let val := fresh "val" in *)
+(*           let stt := fresh "stt" in *)
+(*           destruct ost as [val [stt ?]] *)
+(*         end *)
+(*       | [H: ?oss@[child2Idx] = Some ?ost |- _] => *)
+(*         match type of ost with *)
+(*         | OState _ => *)
+(*           let val := fresh "val" in *)
+(*           let stt := fresh "stt" in *)
+(*           destruct ost as [val [stt ?]] *)
+(*         end *)
+(*       | [H: msiM = _ |- _] => apply eq_sym in H *)
+(*       | [H: msiS = _ |- _] => apply eq_sym in H *)
+(*       | [H: msiI = _ |- _] => apply eq_sym in H *)
+(*       | [H1: ?t = msiM, H2: ?t = msiS |- _] => rewrite H1 in H2; discriminate *)
+(*       | [H1: ?t = msiM, H2: ?t = msiI |- _] => rewrite H1 in H2; discriminate *)
+(*       | [H1: ?t = msiS, H2: ?t = msiI |- _] => rewrite H1 in H2; discriminate *)
+(*       | [H1: ?t = msiM, H2: ?t <= msiS |- _] => *)
+(*         rewrite H1 in H2; unfold msiM, msiS in H2; lia *)
+(*       | [H1: ?t = msiI, H2: ?t >= msiS |- _] => *)
+(*         rewrite H1 in H2; unfold msiS, msiI in H2; lia *)
+(*       end. *)
 
-  Ltac solve_msi :=
-    unfold msiM, msiS, msiI in *; lia.
+(*   Ltac solve_msi := *)
+(*     unfold msiM, msiS, msiI in *; lia. *)
   
-  Ltac disc_rule_custom ::=
-    try disc_msi.
+(*   Ltac disc_rule_custom ::= *)
+(*     try disc_msi. *)
   
-  Section Facts.
+(*   Section Facts. *)
 
-    Lemma msiSv_impl_ORqsInit: GoodORqsInit (initsOf impl).
-    Proof.
-      red; intros.
-      cbn; unfold implORqsInit.
-      mred.
-    Qed.
+(*     Lemma implInv_orqs_weakened: *)
+(*       forall st oidx orq norq rqt rqi nmsgs, *)
+(*         ImplInv st -> *)
+(*         (oidx = child1Idx \/ oidx = child2Idx) -> *)
+(*         (bst_orqs st)@[oidx] = Some orq -> *)
+(*         norq = orq +[rqt <- rqi] -> *)
+(*         ImplInv {| bst_oss := bst_oss st; *)
+(*                    bst_orqs := (bst_orqs st) +[oidx <- norq]; *)
+(*                    bst_msgs := nmsgs |}. *)
+(*     Proof. *)
+(*       unfold ImplInv, ImplStateInv, ImplLockInv; simpl; intros; dest. *)
+(*       split. *)
+(*       - disc_rule_conds_const. *)
+(*         destruct H as [[cv ?] ?]. *)
+(*         destruct H0; subst. *)
+(*         + solve_rule_conds_ex. *)
+(*         + solve_rule_conds_ex. *)
+(*       - disc_rule_conds_const. *)
+(*         destruct H0; subst; mred. *)
+(*     Qed. *)
 
-    Lemma implInv_orqs_weakened:
-      forall st oidx orq norq rqt rqi nmsgs,
-        ImplInv st ->
-        (oidx = child1Idx \/ oidx = child2Idx) ->
-        (bst_orqs st)@[oidx] = Some orq ->
-        norq = orq +[rqt <- rqi] ->
-        ImplInv {| bst_oss := bst_oss st;
-                   bst_orqs := (bst_orqs st) +[oidx <- norq];
-                   bst_msgs := nmsgs |}.
-    Proof.
-      unfold ImplInv, ImplStateInv, ImplLockInv; simpl; intros; dest.
-      split.
-      - disc_rule_conds_const.
-        destruct H as [[cv ?] ?].
-        destruct H0; subst.
-        + solve_rule_conds_ex.
-        + solve_rule_conds_ex.
-      - disc_rule_conds_const.
-        destruct H0; subst; mred.
-    Qed.
+(*     Lemma implInv_M_value_changed: *)
+(*       forall st, *)
+(*         ImplInv st -> *)
+(*         forall oidx ost orq, *)
+(*           (oidx = child1Idx \/ oidx = child2Idx) -> *)
+(*           (bst_oss st)@[oidx] = Some ost -> *)
+(*           ost#[implStatusIdx] = msiM -> *)
+(*           (bst_orqs st)@[oidx] = Some orq -> *)
+(*           orq@[upRq] = None -> *)
+(*           forall n (uv: DirT * unit) nmsgs, *)
+(*             ImplInv *)
+(*               (Build_MState *)
+(*                  (oifc:= ImplOStateIfc) *)
+(*                  ((bst_oss st) +[oidx <- (n, (msiM, uv))]) *)
+(*                  (bst_orqs st) nmsgs). *)
+(*     Proof. *)
+(*       unfold ImplInv, ImplStateInv, ImplLockInv; simpl; intros; dest. *)
+(*       split. *)
+(*       - disc_rule_conds_const. *)
+(*         destruct H as [[cv ?] ?]. *)
+(*         disc_rule_conds_ex. *)
+(*         + destruct H0; discriminate. *)
+(*         + split. *)
+(*           * exists n; repeat split. *)
+(*             { disc_rule_conds_ex. *)
+(*               destruct H as [|[|]]; *)
+(*                 try (exfalso; solve_rule_conds_ex; solve_msi; fail). *)
+(*               right; right. *)
+(*               solve_rule_conds_ex. *)
+(*             } *)
+(*             { solve_rule_conds_ex; solve_msi. } *)
+(*             { solve_rule_conds_ex. } *)
+(*             { solve_rule_conds_ex. } *)
+(*           * solve_rule_conds_ex. *)
+(*         + split. *)
+(*           * exists n; repeat split. *)
+(*             { disc_rule_conds_ex. *)
+(*               destruct H as [|[|]]; *)
+(*                 try (exfalso; solve_rule_conds_ex; solve_msi; fail). *)
+(*               right; right. *)
+(*               solve_rule_conds_ex. *)
+(*             } *)
+(*             { solve_rule_conds_ex; solve_msi. } *)
+(*             { solve_rule_conds_ex. } *)
+(*             { solve_rule_conds_ex. } *)
+(*           * solve_rule_conds_ex. *)
+(*         + eauto 7. *)
+(*       - assumption. *)
+(*     Qed. *)
 
-    Lemma implInv_M_value_changed:
-      forall st,
-        ImplInv st ->
-        forall oidx ost orq,
-          (oidx = child1Idx \/ oidx = child2Idx) ->
-          (bst_oss st)@[oidx] = Some ost ->
-          ost#[implStatusIdx] = msiM ->
-          (bst_orqs st)@[oidx] = Some orq ->
-          orq@[upRq] = None ->
-          forall n (uv: DirT * unit) nmsgs,
-            ImplInv
-              (Build_MState
-                 (oifc:= ImplOStateIfc)
-                 ((bst_oss st) +[oidx <- (n, (msiM, uv))])
-                 (bst_orqs st) nmsgs).
-    Proof.
-      unfold ImplInv, ImplStateInv, ImplLockInv; simpl; intros; dest.
-      split.
-      - disc_rule_conds_const.
-        destruct H as [[cv ?] ?].
-        disc_rule_conds_ex.
-        + destruct H0; discriminate.
-        + split.
-          * exists n; repeat split.
-            { disc_rule_conds_ex.
-              destruct H as [|[|]];
-                try (exfalso; solve_rule_conds_ex; solve_msi; fail).
-              right; right.
-              solve_rule_conds_ex.
-            }
-            { solve_rule_conds_ex; solve_msi. }
-            { solve_rule_conds_ex. }
-            { solve_rule_conds_ex. }
-          * solve_rule_conds_ex.
-        + split.
-          * exists n; repeat split.
-            { disc_rule_conds_ex.
-              destruct H as [|[|]];
-                try (exfalso; solve_rule_conds_ex; solve_msi; fail).
-              right; right.
-              solve_rule_conds_ex.
-            }
-            { solve_rule_conds_ex; solve_msi. }
-            { solve_rule_conds_ex. }
-            { solve_rule_conds_ex. }
-          * solve_rule_conds_ex.
-        + eauto 7.
-      - assumption.
-    Qed.
+(*     Lemma msiSv_impl_InvTrs_ext_in: *)
+(*       forall st1 eins st2, *)
+(*         ImplInv st1 -> *)
+(*         step_m impl st1 (RlblIns eins) st2 -> *)
+(*         ImplInv st2. *)
+(*     Proof. *)
+(*       intros; inv_step; assumption. *)
+(*     Qed. *)
 
-    Lemma msiSv_impl_InvTrs_ext_in:
-      forall st1 eins st2,
-        ImplInv st1 ->
-        step_m impl st1 (RlblIns eins) st2 ->
-        ImplInv st2.
-    Proof.
-      intros; inv_step; assumption.
-    Qed.
+(*     Lemma msiSv_impl_InvTrs_ext_out: *)
+(*       forall st1 eouts st2, *)
+(*         ImplInv st1 -> *)
+(*         step_m impl st1 (RlblOuts eouts) st2 -> *)
+(*         ImplInv st2. *)
+(*     Proof. *)
+(*       intros; inv_step; assumption. *)
+(*     Qed. *)
 
-    Lemma msiSv_impl_InvTrs_ext_out:
-      forall st1 eouts st2,
-        ImplInv st1 ->
-        step_m impl st1 (RlblOuts eouts) st2 ->
-        ImplInv st2.
-    Proof.
-      intros; inv_step; assumption.
-    Qed.
+(*     Definition MsiSvMsgOutPred: MsgOutPred ImplOStateIfc := *)
+(*       fun eout oss orqs => *)
+(*         match case (sigOf eout) on sig_dec default True with *)
+(*         | (ec1, (MRq, Spec.getRq)): False *)
+(*         | (ec1, (MRq, Spec.setRq)): False *)
+(*         | (ec1, (MRq, Spec.evictRq)): False *)
+(*         | (ec2, (MRq, Spec.getRq)): False *)
+(*         | (ec2, (MRq, Spec.setRq)): False *)
+(*         | (ec2, (MRq, Spec.evictRq)): False *)
 
-    Definition MsiSvMsgOutPred: MsgOutPred ImplOStateIfc :=
-      fun eout oss orqs =>
-        match case (sigOf eout) on sig_dec default True with
-        | (ec1, (MRq, Spec.getRq)): False
-        | (ec1, (MRq, Spec.setRq)): False
-        | (ec1, (MRq, Spec.evictRq)): False
-        | (ec2, (MRq, Spec.getRq)): False
-        | (ec2, (MRq, Spec.setRq)): False
-        | (ec2, (MRq, Spec.evictRq)): False
+(*         | (pc1, (MRs, msiRsS)):  *)
+(*             post <-- oss@[parentIdx]; *)
+(*             porq <-- orqs@[parentIdx]; *)
+(*             post#[implStatusIdx] = msiS /\ *)
+(*             post#[implDirIdx].(fst) = msiS /\ *)
+(*             porq@[downRq] = None /\ *)
+(*             msg_value (valOf eout) = VNat post#[implValueIdx] *)
+(*         | (pc2, (MRs, msiRsS)): *)
+(*             post <-- oss@[parentIdx]; *)
+(*             porq <-- orqs@[parentIdx]; *)
+(*             post#[implStatusIdx] = msiS /\ *)
+(*             post#[implDirIdx].(snd) = msiS /\ *)
+(*             porq@[downRq] = None /\ *)
+(*             msg_value (valOf eout) = VNat post#[implValueIdx] *)
 
-        | (pc1, (MRs, msiRsS)): 
-            post <-- oss@[parentIdx];
-            porq <-- orqs@[parentIdx];
-            post#[implStatusIdx] = msiS /\
-            post#[implDirIdx].(fst) = msiS /\
-            porq@[downRq] = None /\
-            msg_value (valOf eout) = VNat post#[implValueIdx]
-        | (pc2, (MRs, msiRsS)):
-            post <-- oss@[parentIdx];
-            porq <-- orqs@[parentIdx];
-            post#[implStatusIdx] = msiS /\
-            post#[implDirIdx].(snd) = msiS /\
-            porq@[downRq] = None /\
-            msg_value (valOf eout) = VNat post#[implValueIdx]
+(*         | (pc1, (MRs, msiRsM)): *)
+(*             post <-- oss@[parentIdx]; *)
+(*             porq <-- orqs@[parentIdx]; *)
+(*             post#[implStatusIdx] = msiI /\ *)
+(*             post#[implDirIdx].(fst) = msiM /\ *)
+(*             porq@[downRq] = None *)
+(*         | (pc2, (MRs, msiRsM)): *)
+(*             post <-- oss@[parentIdx]; *)
+(*             porq <-- orqs@[parentIdx]; *)
+(*             post#[implStatusIdx] = msiI /\ *)
+(*             post#[implDirIdx].(snd) = msiM /\ *)
+(*             porq@[downRq] = None *)
 
-        | (pc1, (MRs, msiRsM)):
-            post <-- oss@[parentIdx];
-            porq <-- orqs@[parentIdx];
-            post#[implStatusIdx] = msiI /\
-            post#[implDirIdx].(fst) = msiM /\
-            porq@[downRq] = None
-        | (pc2, (MRs, msiRsM)):
-            post <-- oss@[parentIdx];
-            porq <-- orqs@[parentIdx];
-            post#[implStatusIdx] = msiI /\
-            post#[implDirIdx].(snd) = msiM /\
-            porq@[downRq] = None
+(*         | (pc1, (MRs, msiRsI)): *)
+(*             post <-- oss@[parentIdx]; *)
+(*             post#[implDirIdx].(fst) = msiI *)
+(*         | (pc2, (MRs, msiRsI)): *)
+(*             post <-- oss@[parentIdx]; *)
+(*             post#[implDirIdx].(snd) = msiI *)
 
-        | (pc1, (MRs, msiRsI)):
-            post <-- oss@[parentIdx];
-            post#[implDirIdx].(fst) = msiI
-        | (pc2, (MRs, msiRsI)):
-            post <-- oss@[parentIdx];
-            post#[implDirIdx].(snd) = msiI
+(*         | (c1pRs, (MRs, msiDownRsS)): *)
+(*             cost1 <-- oss@[child1Idx]; *)
+(*             cost1#[implStatusIdx] = msiS /\              *)
+(*             msg_value (valOf eout) = VNat cost1#[implValueIdx] *)
+(*         | (c2pRs, (MRs, msiDownRsS)): *)
+(*             cost2 <-- oss@[child2Idx]; *)
+(*             cost2#[implStatusIdx] = msiS /\ *)
+(*             msg_value (valOf eout) = VNat cost2#[implValueIdx] *)
 
-        | (c1pRs, (MRs, msiDownRsS)):
-            cost1 <-- oss@[child1Idx];
-            cost1#[implStatusIdx] = msiS /\             
-            msg_value (valOf eout) = VNat cost1#[implValueIdx]
-        | (c2pRs, (MRs, msiDownRsS)):
-            cost2 <-- oss@[child2Idx];
-            cost2#[implStatusIdx] = msiS /\
-            msg_value (valOf eout) = VNat cost2#[implValueIdx]
+(*         | (c1pRs, (MRs, msiDownRsM)): *)
+(*             cost1 <-- oss@[child1Idx]; *)
+(*             cost1#[implStatusIdx] = msiI *)
+(*         | (c2pRs, (MRs, msiDownRsM)): *)
+(*             cost2 <-- oss@[child2Idx]; *)
+(*             cost2#[implStatusIdx] = msiI *)
+(*         end. *)
 
-        | (c1pRs, (MRs, msiDownRsM)):
-            cost1 <-- oss@[child1Idx];
-            cost1#[implStatusIdx] = msiI
-        | (c2pRs, (MRs, msiDownRsM)):
-            cost2 <-- oss@[child2Idx];
-            cost2#[implStatusIdx] = msiI
-        end.
+(*     Lemma msiSvMsgOutPred_good: *)
+(*       GoodMsgOutPred topo impl MsiSvMsgOutPred. *)
+(*     Proof. *)
+(*       red; intros; repeat split. *)
 
-    Lemma msiSvMsgOutPred_good:
-      GoodMsgOutPred topo impl MsiSvMsgOutPred.
-    Proof.
-      red; intros; repeat split.
+(*       - do 2 (red; intros). *)
+(*         red in H0; unfold caseDec in H0. *)
+(*         repeat find_if_inside; *)
+(*           try (exfalso; auto; fail); *)
+(*           disc_GoodMsgOutPred. *)
 
-      - do 2 (red; intros).
-        red in H0; unfold caseDec in H0.
-        repeat find_if_inside;
-          try (exfalso; auto; fail);
-          disc_GoodMsgOutPred.
+(*         + red; unfold sigOf, valOf, snd; rewrite H4, H5; simpl. *)
+(*           assert (In child1Idx (subtreeIndsOf topo child1Idx)). *)
+(*           { simpl; tauto. } *)
+(*           specialize (H1 _ H). *)
+(*           destruct H1; rewrite <-H1. *)
+(*           assumption. *)
 
-        + red; unfold sigOf, valOf, snd; rewrite H4, H5; simpl.
-          assert (In child1Idx (subtreeIndsOf topo child1Idx)).
-          { simpl; tauto. }
-          specialize (H1 _ H).
-          destruct H1; rewrite <-H1.
-          assumption.
+(*         + red; unfold sigOf, valOf, snd; rewrite H4, H5; simpl. *)
+(*           assert (In child2Idx (subtreeIndsOf topo child2Idx)). *)
+(*           { simpl; tauto. } *)
+(*           specialize (H1 _ H). *)
+(*           destruct H1; rewrite <-H1. *)
+(*           assumption. *)
 
-        + red; unfold sigOf, valOf, snd; rewrite H4, H5; simpl.
-          assert (In child2Idx (subtreeIndsOf topo child2Idx)).
-          { simpl; tauto. }
-          specialize (H1 _ H).
-          destruct H1; rewrite <-H1.
-          assumption.
+(*         + red; unfold sigOf, valOf, snd; rewrite H4, H5; simpl. *)
+(*           assert (In child1Idx (subtreeIndsOf topo child1Idx)). *)
+(*           { simpl; tauto. } *)
+(*           specialize (H1 _ H). *)
+(*           destruct H1; rewrite <-H1. *)
+(*           assumption. *)
 
-        + red; unfold sigOf, valOf, snd; rewrite H4, H5; simpl.
-          assert (In child1Idx (subtreeIndsOf topo child1Idx)).
-          { simpl; tauto. }
-          specialize (H1 _ H).
-          destruct H1; rewrite <-H1.
-          assumption.
+(*         + red; unfold sigOf, valOf, snd; rewrite H4, H5; simpl. *)
+(*           assert (In child2Idx (subtreeIndsOf topo child2Idx)). *)
+(*           { simpl; tauto. } *)
+(*           specialize (H1 _ H). *)
+(*           destruct H1; rewrite <-H1. *)
+(*           assumption. *)
 
-        + red; unfold sigOf, valOf, snd; rewrite H4, H5; simpl.
-          assert (In child2Idx (subtreeIndsOf topo child2Idx)).
-          { simpl; tauto. }
-          specialize (H1 _ H).
-          destruct H1; rewrite <-H1.
-          assumption.
+(*         + red; unfold caseDec. *)
+(*           repeat find_if_inside; congruence. *)
 
-        + red; unfold caseDec.
-          repeat find_if_inside; congruence.
+(*       - do 2 (red; intros). *)
+(*         red in H0; unfold caseDec in H0. *)
+(*         repeat find_if_inside; *)
+(*           try (exfalso; auto; fail); *)
+(*           disc_GoodMsgOutPred. *)
 
-      - do 2 (red; intros).
-        red in H0; unfold caseDec in H0.
-        repeat find_if_inside;
-          try (exfalso; auto; fail);
-          disc_GoodMsgOutPred.
+(*         + red; unfold sigOf, valOf, snd; rewrite H4, H5; simpl. *)
+(*           assert (~ In parentIdx (subtreeIndsOf topo child1Idx)). *)
+(*           { intro Hx; dest_in; discriminate. } *)
+(*           specialize (H1 _ H). *)
+(*           destruct H1; rewrite <-H1, <-H6. *)
+(*           assumption. *)
 
-        + red; unfold sigOf, valOf, snd; rewrite H4, H5; simpl.
-          assert (~ In parentIdx (subtreeIndsOf topo child1Idx)).
-          { intro Hx; dest_in; discriminate. }
-          specialize (H1 _ H).
-          destruct H1; rewrite <-H1, <-H6.
-          assumption.
+(*         + red; unfold sigOf, valOf, snd; rewrite H4, H5; simpl. *)
+(*           assert (~ In parentIdx (subtreeIndsOf topo child2Idx)). *)
+(*           { intro Hx; dest_in; discriminate. } *)
+(*           specialize (H1 _ H). *)
+(*           destruct H1; rewrite <-H1, <-H6. *)
+(*           assumption. *)
 
-        + red; unfold sigOf, valOf, snd; rewrite H4, H5; simpl.
-          assert (~ In parentIdx (subtreeIndsOf topo child2Idx)).
-          { intro Hx; dest_in; discriminate. }
-          specialize (H1 _ H).
-          destruct H1; rewrite <-H1, <-H6.
-          assumption.
+(*         + red; unfold sigOf, valOf, snd; rewrite H4, H5; simpl. *)
+(*           assert (~ In parentIdx (subtreeIndsOf topo child1Idx)). *)
+(*           { intro Hx; dest_in; discriminate. } *)
+(*           specialize (H1 _ H). *)
+(*           destruct H1; rewrite <-H1, <-H6. *)
+(*           assumption. *)
 
-        + red; unfold sigOf, valOf, snd; rewrite H4, H5; simpl.
-          assert (~ In parentIdx (subtreeIndsOf topo child1Idx)).
-          { intro Hx; dest_in; discriminate. }
-          specialize (H1 _ H).
-          destruct H1; rewrite <-H1, <-H6.
-          assumption.
+(*         + red; unfold sigOf, valOf, snd; rewrite H4, H5; simpl. *)
+(*           assert (~ In parentIdx (subtreeIndsOf topo child2Idx)). *)
+(*           { intro Hx; dest_in; discriminate. } *)
+(*           specialize (H1 _ H). *)
+(*           destruct H1; rewrite <-H1, <-H6. *)
+(*           assumption. *)
 
-        + red; unfold sigOf, valOf, snd; rewrite H4, H5; simpl.
-          assert (~ In parentIdx (subtreeIndsOf topo child2Idx)).
-          { intro Hx; dest_in; discriminate. }
-          specialize (H1 _ H).
-          destruct H1; rewrite <-H1, <-H6.
-          assumption.
+(*         + red; unfold sigOf, valOf, snd; rewrite H4, H5; simpl. *)
+(*           assert (~ In parentIdx (subtreeIndsOf topo child1Idx)). *)
+(*           { intro Hx; dest_in; discriminate. } *)
+(*           specialize (H1 _ H). *)
+(*           destruct H1; rewrite <-H1. *)
+(*           assumption. *)
 
-        + red; unfold sigOf, valOf, snd; rewrite H4, H5; simpl.
-          assert (~ In parentIdx (subtreeIndsOf topo child1Idx)).
-          { intro Hx; dest_in; discriminate. }
-          specialize (H1 _ H).
-          destruct H1; rewrite <-H1.
-          assumption.
+(*         + red; unfold sigOf, valOf, snd; rewrite H4, H5; simpl. *)
+(*           assert (~ In parentIdx (subtreeIndsOf topo child2Idx)). *)
+(*           { intro Hx; dest_in; discriminate. } *)
+(*           specialize (H1 _ H). *)
+(*           destruct H1; rewrite <-H1. *)
+(*           assumption. *)
 
-        + red; unfold sigOf, valOf, snd; rewrite H4, H5; simpl.
-          assert (~ In parentIdx (subtreeIndsOf topo child2Idx)).
-          { intro Hx; dest_in; discriminate. }
-          specialize (H1 _ H).
-          destruct H1; rewrite <-H1.
-          assumption.
-
-        + red; unfold caseDec.
-          repeat find_if_inside; congruence.
+(*         + red; unfold caseDec. *)
+(*           repeat find_if_inside; congruence. *)
           
-      - red; intros.
-        destruct (in_dec eq_nat_dec (idOf eout) (sys_merqs impl)); auto.
-        right; intros.
-        red; unfold caseDec.
-        repeat find_if_inside; disc_GoodMsgOutPred.
-        auto.
+(*       - red; intros. *)
+(*         destruct (in_dec eq_nat_dec (idOf eout) (sys_merqs impl)); auto. *)
+(*         right; intros. *)
+(*         red; unfold caseDec. *)
+(*         repeat find_if_inside; disc_GoodMsgOutPred. *)
+(*         auto. *)
 
-      - red; intros.
-        red; unfold caseDec.
-        repeat find_if_inside; disc_GoodMsgOutPred.
-        auto.
-    Qed.
+(*       - red; intros. *)
+(*         red; unfold caseDec. *)
+(*         repeat find_if_inside; disc_GoodMsgOutPred. *)
+(*         auto. *)
+(*     Qed. *)
 
-    Ltac disc_rule_custom ::=
-      try disc_footprints_ok;
-      try disc_AtomicInv.
+(*     Ltac disc_rule_custom ::= *)
+(*       try disc_footprints_ok; *)
+(*       try disc_AtomicInv. *)
 
-    Lemma msiSv_impl_InvTrs_init:
-      forall st1,
-        Reachable (steps step_m) impl st1 ->
-        ImplInv st1 ->
-        forall oidx ridx ins outs st2,
-          SubList (idsOf ins) (sys_merqs impl) ->
-          step_m impl st1 (RlblInt oidx ridx ins outs) st2 ->
-          AtomicInv
-            MsiSvMsgOutPred
-            ins st1 [RlblInt oidx ridx ins outs] outs st2 /\
-          ImplInv st2.
-    Proof.
-      intros.
-      inv_step.
-      pose proof (upLockInv_ok
-                    msiSv_impl_ORqsInit
-                    msiSv_impl_GoodRqRsSys
-                    msiSv_impl_RqRsDTree H) as Hulinv.
-      pose proof (downLockInv_ok
-                    msiSv_impl_ORqsInit
-                    msiSv_impl_GoodRqRsSys
-                    msiSv_impl_RqRsDTree
-                    msiSv_impl_GoodExtRssSys H) as Hdlinv.
-      good_locking_get obj.
-      dest_in.
+(*     Lemma msiSv_impl_InvTrs_init: *)
+(*       forall st1, *)
+(*         Reachable (steps step_m) impl st1 -> *)
+(*         ImplInv st1 -> *)
+(*         forall oidx ridx ins outs st2, *)
+(*           SubList (idsOf ins) (sys_merqs impl) -> *)
+(*           step_m impl st1 (RlblInt oidx ridx ins outs) st2 -> *)
+(*           AtomicInv *)
+(*             MsiSvMsgOutPred *)
+(*             ins st1 [RlblInt oidx ridx ins outs] outs st2 /\ *)
+(*           ImplInv st2. *)
+(*     Proof. *)
+(*       intros. *)
+(*       inv_step. *)
+(*       pose proof (upLockInv_ok *)
+(*                     msiSv_impl_ORqsInit *)
+(*                     msiSv_impl_GoodRqRsSys *)
+(*                     msiSv_impl_RqRsDTree H) as Hulinv. *)
+(*       pose proof (downLockInv_ok *)
+(*                     msiSv_impl_ORqsInit *)
+(*                     msiSv_impl_GoodRqRsSys *)
+(*                     msiSv_impl_RqRsDTree *)
+(*                     msiSv_impl_GoodExtRssSys H) as Hdlinv. *)
+(*       good_locking_get obj. *)
+(*       dest_in. *)
 
-      (** List of [Rule]s:
-       * [childGetRqImm; childGetRqS; childGetRsS; childDownRqS; 
-       *  childSetRqImm; childSetRqM; childSetRsM; childDownRqM;
-       *  childEvictRqI; childEvictRsI] for [child1Idx] +
-       * [childGetRqImm; childGetRqS; childGetRsS; childDownRqS; 
-       *  childSetRqImm; childSetRqM; childSetRsM; childDownRqM;
-       *  childEvictRqI; childEvictRsI] for [child2Idx] +
-       * [parentGetRqImm; parentGetDownRqS; parentSetRqImm; parentSetDownRqM;
-       *  parentGetDownRsS; parentSetDownRsM;
-       *  parentEvictRqImmI; parentEvictRqImmS; parentEvictRqImmLastS; parentEvictRqImmM]
-       *  * {child1Idx, child2Idx}
-       *)
+(*       (** List of [Rule]s: *)
+(*        * [childGetRqImm; childGetRqS; childGetRsS; childDownRqS;  *)
+(*        *  childSetRqImm; childSetRqM; childSetRsM; childDownRqM; *)
+(*        *  childEvictRqI; childEvictRsI] for [child1Idx] + *)
+(*        * [childGetRqImm; childGetRqS; childGetRsS; childDownRqS;  *)
+(*        *  childSetRqImm; childSetRqM; childSetRsM; childDownRqM; *)
+(*        *  childEvictRqI; childEvictRsI] for [child2Idx] + *)
+(*        * [parentGetRqImm; parentGetDownRqS; parentSetRqImm; parentSetDownRqM; *)
+(*        *  parentGetDownRsS; parentSetDownRsM; *)
+(*        *  parentEvictRqImmI; parentEvictRqImmS; parentEvictRqImmLastS; parentEvictRqImmM] *)
+(*        *  * {child1Idx, child2Idx} *)
+(*        *) *)
 
-      3, 7, 10, 13, 17, 20: atomic_init_exfalso_rs_from_parent.
-      all: try (atomic_init_exfalso_rq; fail).
+(*       3, 7, 10, 13, 17, 20: atomic_init_exfalso_rs_from_parent. *)
+(*       all: try (atomic_init_exfalso_rq; fail). *)
 
-      - (** [childGetRqImm] *)
-        disc_rule_conds_ex.
-        simpl; split; [atomic_init_solve_AtomicInv|].
-        replace (oss +[child1Idx <- pos]) with oss by meq.
-        replace (orqs +[child1Idx <- norq]) with orqs by meq.
-        assumption.
+(*       - (** [childGetRqImm] *) *)
+(*         disc_rule_conds_ex. *)
+(*         simpl; split; [atomic_init_solve_AtomicInv|]. *)
+(*         replace (oss +[child1Idx <- pos]) with oss by meq. *)
+(*         replace (orqs +[child1Idx <- norq]) with orqs by meq. *)
+(*         assumption. *)
 
-      - (** [childGetRqS] *)
-        disc_rule_conds_ex.
-        simpl; split; [atomic_init_solve_AtomicInv|].
-        replace (oss +[child1Idx <- pos]) with oss by meq.
-        eapply implInv_orqs_weakened in H0; eauto.
+(*       - (** [childGetRqS] *) *)
+(*         disc_rule_conds_ex. *)
+(*         simpl; split; [atomic_init_solve_AtomicInv|]. *)
+(*         replace (oss +[child1Idx <- pos]) with oss by meq. *)
+(*         eapply implInv_orqs_weakened in H0; eauto. *)
 
-      - (** [childSetRqImm] *)
-        disc_rule_conds_ex.
-        simpl; split; [atomic_init_solve_AtomicInv|].
-        replace (orqs +[child1Idx <- norq]) with orqs by meq.
-        eapply implInv_M_value_changed in H0; eauto.
+(*       - (** [childSetRqImm] *) *)
+(*         disc_rule_conds_ex. *)
+(*         simpl; split; [atomic_init_solve_AtomicInv|]. *)
+(*         replace (orqs +[child1Idx <- norq]) with orqs by meq. *)
+(*         eapply implInv_M_value_changed in H0; eauto. *)
 
-      - (** [childSetRqM] *)
-        disc_rule_conds_ex.
-        simpl; split; [atomic_init_solve_AtomicInv|].
-        replace (oss +[child1Idx <- pos]) with oss by meq.
-        eapply implInv_orqs_weakened in H0; eauto.
+(*       - (** [childSetRqM] *) *)
+(*         disc_rule_conds_ex. *)
+(*         simpl; split; [atomic_init_solve_AtomicInv|]. *)
+(*         replace (oss +[child1Idx <- pos]) with oss by meq. *)
+(*         eapply implInv_orqs_weakened in H0; eauto. *)
 
-      - (** [childEvictRqI] *)
-        disc_rule_conds_ex.
-        simpl; split; [atomic_init_solve_AtomicInv|].
-        replace (oss +[child1Idx <- pos]) with oss by meq.
-        eapply implInv_orqs_weakened in H0; eauto.
+(*       - (** [childEvictRqI] *) *)
+(*         disc_rule_conds_ex. *)
+(*         simpl; split; [atomic_init_solve_AtomicInv|]. *)
+(*         replace (oss +[child1Idx <- pos]) with oss by meq. *)
+(*         eapply implInv_orqs_weakened in H0; eauto. *)
 
-      - (** [childGetRqImm] *)
-        disc_rule_conds_ex.
-        simpl; split; [atomic_init_solve_AtomicInv|].
-        replace (oss +[child2Idx <- pos]) with oss by meq.
-        replace (orqs +[child2Idx <- norq]) with orqs by meq.
-        assumption.
+(*       - (** [childGetRqImm] *) *)
+(*         disc_rule_conds_ex. *)
+(*         simpl; split; [atomic_init_solve_AtomicInv|]. *)
+(*         replace (oss +[child2Idx <- pos]) with oss by meq. *)
+(*         replace (orqs +[child2Idx <- norq]) with orqs by meq. *)
+(*         assumption. *)
 
-      - (** [childGetRqS] *)
-        disc_rule_conds_ex.
-        simpl; split; [atomic_init_solve_AtomicInv|].
-        replace (oss +[child2Idx <- pos]) with oss by meq.
-        eapply implInv_orqs_weakened in H0; eauto.
+(*       - (** [childGetRqS] *) *)
+(*         disc_rule_conds_ex. *)
+(*         simpl; split; [atomic_init_solve_AtomicInv|]. *)
+(*         replace (oss +[child2Idx <- pos]) with oss by meq. *)
+(*         eapply implInv_orqs_weakened in H0; eauto. *)
 
-      - (** [childSetRqImm] *)
-        disc_rule_conds_ex.
-        simpl; split; [atomic_init_solve_AtomicInv|].
-        replace (orqs +[child2Idx <- norq]) with orqs by meq.
-        eapply implInv_M_value_changed in H0; eauto.
+(*       - (** [childSetRqImm] *) *)
+(*         disc_rule_conds_ex. *)
+(*         simpl; split; [atomic_init_solve_AtomicInv|]. *)
+(*         replace (orqs +[child2Idx <- norq]) with orqs by meq. *)
+(*         eapply implInv_M_value_changed in H0; eauto. *)
 
-      - (** [childSetRqM] *)
-        disc_rule_conds_ex.
-        simpl; split; [atomic_init_solve_AtomicInv|].
-        replace (oss +[child2Idx <- pos]) with oss by meq.
-        eapply implInv_orqs_weakened in H0; eauto.
+(*       - (** [childSetRqM] *) *)
+(*         disc_rule_conds_ex. *)
+(*         simpl; split; [atomic_init_solve_AtomicInv|]. *)
+(*         replace (oss +[child2Idx <- pos]) with oss by meq. *)
+(*         eapply implInv_orqs_weakened in H0; eauto. *)
 
-      - (** [childEvictRqI] *)
-        disc_rule_conds_ex.
-        simpl; split; [atomic_init_solve_AtomicInv|].
-        replace (oss +[child2Idx <- pos]) with oss by meq.
-        eapply implInv_orqs_weakened in H0; eauto.
-    Qed.
+(*       - (** [childEvictRqI] *) *)
+(*         disc_rule_conds_ex. *)
+(*         simpl; split; [atomic_init_solve_AtomicInv|]. *)
+(*         replace (oss +[child2Idx <- pos]) with oss by meq. *)
+(*         eapply implInv_orqs_weakened in H0; eauto. *)
+(*     Qed. *)
 
-    Ltac disc_rule_custom ::=
-      try disc_footprints_ok;
-      try disc_msg_case;
-      try disc_AtomicInv;
-      try disc_msi;
-      try disc_minds_const.
+(*     Ltac disc_rule_custom ::= *)
+(*       try disc_footprints_ok; *)
+(*       try disc_msg_case; *)
+(*       try disc_AtomicInv; *)
+(*       try disc_msi; *)
+(*       try disc_minds_const. *)
 
-    Lemma msiSv_impl_InvTrs: InvTrs impl ImplInv.
-    Proof.
-      eapply inv_atomic_InvTrs;
-        [red; intros; eapply msiSv_impl_InvTrs_ext_in; eauto
-        |red; intros; eapply msiSv_impl_InvTrs_ext_out; eauto
-        |].
-      instantiate (1:= AtomicInv MsiSvMsgOutPred).
-      red; intros.
-      destruct H1.
-      generalize dependent ist2.
-      induction H3; simpl; intros; subst;
-        [inv_steps; apply msiSv_impl_InvTrs_init; auto|].
+(*     Lemma msiSv_impl_InvTrs: InvTrs impl ImplInv. *)
+(*     Proof. *)
+(*       eapply inv_atomic_InvTrs; *)
+(*         [red; intros; eapply msiSv_impl_InvTrs_ext_in; eauto *)
+(*         |red; intros; eapply msiSv_impl_InvTrs_ext_out; eauto *)
+(*         |]. *)
+(*       instantiate (1:= AtomicInv MsiSvMsgOutPred). *)
+(*       red; intros. *)
+(*       destruct H1. *)
+(*       generalize dependent ist2. *)
+(*       induction H3; simpl; intros; subst; *)
+(*         [inv_steps; apply msiSv_impl_InvTrs_init; auto|]. *)
 
-      inv_steps.
-      pose proof (footprints_ok
-                    msiSv_impl_ORqsInit
-                    msiSv_impl_GoodRqRsSys
-                    (reachable_steps H H9))
-        as Hftinv.
-      specialize (IHAtomic H1 _ H9); dest.
-      pose proof (upLockInv_ok
-                    msiSv_impl_ORqsInit
-                    msiSv_impl_GoodRqRsSys
-                    msiSv_impl_RqRsDTree (reachable_steps H H9)) as Hulinv.
-      pose proof (downLockInv_ok
-                    msiSv_impl_ORqsInit
-                    msiSv_impl_GoodRqRsSys
-                    msiSv_impl_RqRsDTree
-                    msiSv_impl_GoodExtRssSys (reachable_steps H H9)) as Hdlinv.
-      inv_step; dest_in.
+(*       inv_steps. *)
+(*       pose proof (footprints_ok *)
+(*                     msiSv_impl_ORqsInit *)
+(*                     msiSv_impl_GoodRqRsSys *)
+(*                     (reachable_steps H H9)) *)
+(*         as Hftinv. *)
+(*       specialize (IHAtomic H1 _ H9); dest. *)
+(*       pose proof (upLockInv_ok *)
+(*                     msiSv_impl_ORqsInit *)
+(*                     msiSv_impl_GoodRqRsSys *)
+(*                     msiSv_impl_RqRsDTree (reachable_steps H H9)) as Hulinv. *)
+(*       pose proof (downLockInv_ok *)
+(*                     msiSv_impl_ORqsInit *)
+(*                     msiSv_impl_GoodRqRsSys *)
+(*                     msiSv_impl_RqRsDTree *)
+(*                     msiSv_impl_GoodExtRssSys (reachable_steps H H9)) as Hdlinv. *)
+(*       inv_step; dest_in. *)
 
-      (** child1 *)
+(*       (** child1 *) *)
 
-      - atomic_cont_exfalso_bound MsiSvMsgOutPred.
-      - atomic_cont_exfalso_bound MsiSvMsgOutPred.
+(*       - atomic_cont_exfalso_bound MsiSvMsgOutPred. *)
+(*       - atomic_cont_exfalso_bound MsiSvMsgOutPred. *)
 
-      - (** [childGetRsS] *)
-        disc_rule_conds_ex.
-        good_footprint_get child1Idx.
-        disc_rule_conds_ex.
+(*       - (** [childGetRsS] *) *)
+(*         disc_rule_conds_ex. *)
+(*         good_footprint_get child1Idx. *)
+(*         disc_rule_conds_ex. *)
 
-        (* discharge message predicates *)
-        disc_msg_preds H4.
-        disc_rule_conds_ex.
+(*         (* discharge message predicates *) *)
+(*         disc_msg_preds H4. *)
+(*         disc_rule_conds_ex. *)
 
-        (* generate hints for leaves (L1 caches) *)
-        pose proof (parentIdxOf_child_indsOf _ _ H7).
-        dest_in; try discriminate; simpl in *.
-        cbn in H26; inv H26.
+(*         (* generate hints for leaves (L1 caches) *) *)
+(*         pose proof (parentIdxOf_child_indsOf _ _ H7). *)
+(*         dest_in; try discriminate; simpl in *. *)
+(*         cbn in H26; inv H26. *)
 
-        (* construction *)
-        split.
-        + apply Forall_app.
-          * apply forall_removeOnce.
-            eapply atomic_rsDown_preserves_msg_out_preds; eauto;
-              [exact msiSv_impl_ORqsInit
-              |exact msiSv_impl_RqRsSys
-              |red; auto
-              |exact msiSvMsgOutPred_good].
-          * repeat (constructor; simpl).
-        + destruct H6; split.
-          * red in H6; red; simpl in *; mred; simpl.
-            destruct (oss@[child2Idx]) as [cost2|]; simpl in *; [|auto].
-            destruct (orqs@[child2Idx]) as [corq2|]; simpl in *; [|auto].
-            destruct H6 as [[cv ?] ?].
-            red in H6; dest.
-            split.
-            { exists val0.
-              red; repeat ssplit.
-              { solve_rule_conds_ex; solve_msi. }
-              { solve_rule_conds_ex. }
-              { solve_rule_conds_ex; solve_msi. }
-              { solve_rule_conds_ex; solve_msi. }
-            }
-            { solve_rule_conds_ex; solve_msi. }
-          * red in H22; red; simpl in *; mred.
+(*         (* construction *) *)
+(*         split. *)
+(*         + apply Forall_app. *)
+(*           * apply forall_removeOnce. *)
+(*             eapply atomic_rsDown_preserves_msg_out_preds; eauto; *)
+(*               [exact msiSv_impl_ORqsInit *)
+(*               |exact msiSv_impl_RqRsSys *)
+(*               |red; auto *)
+(*               |exact msiSvMsgOutPred_good]. *)
+(*           * repeat (constructor; simpl). *)
+(*         + destruct H6; split. *)
+(*           * red in H6; red; simpl in *; mred; simpl. *)
+(*             destruct (oss@[child2Idx]) as [cost2|]; simpl in *; [|auto]. *)
+(*             destruct (orqs@[child2Idx]) as [corq2|]; simpl in *; [|auto]. *)
+(*             destruct H6 as [[cv ?] ?]. *)
+(*             red in H6; dest. *)
+(*             split. *)
+(*             { exists val0. *)
+(*               red; repeat ssplit. *)
+(*               { solve_rule_conds_ex; solve_msi. } *)
+(*               { solve_rule_conds_ex. } *)
+(*               { solve_rule_conds_ex; solve_msi. } *)
+(*               { solve_rule_conds_ex; solve_msi. } *)
+(*             } *)
+(*             { solve_rule_conds_ex; solve_msi. } *)
+(*           * red in H22; red; simpl in *; mred. *)
             
-      - (** [childDownRqS] *)
-        disc_rule_conds_ex.
+(*       - (** [childDownRqS] *) *)
+(*         disc_rule_conds_ex. *)
 
-        (* construction *)
-        split.
-        + apply Forall_app.
-          * apply forall_removeOnce.
-            eapply atomic_rqDown_preserves_msg_out_preds; eauto;
-              [exact msiSv_impl_ORqsInit
-              |exact msiSv_impl_RqRsSys
-              |red; auto
-              |exact msiSvMsgOutPred_good].
-          * repeat (constructor; simpl).
-            red; simpl.
-            mred; simpl; auto.
-        + destruct H6; split.
-          * red in H6; red; simpl in *; mred; simpl.
-            destruct (oss@[parentIdx]) as [post|] eqn:Hpost; simpl in *; [|auto].
-            destruct (oss@[child2Idx]) as [cost2|] eqn:Hcost2; simpl in *; [|auto].
-            destruct (orqs@[child2Idx]) as [corq2|] eqn:Hcorq2; simpl in *; [|auto].
-            destruct H6 as [[cv ?] ?].
-            red in H6; dest.
-            split.
-            { exists cv.
-              red; repeat ssplit.
-              { solve_rule_conds_ex. }
-              { solve_rule_conds_ex. }
-              { solve_rule_conds_ex. }
-              { solve_rule_conds_ex; solve_msi. }
-            }
-            { solve_rule_conds_ex; solve_msi. }
-          * red in H7; red; simpl in *; mred.
+(*         (* construction *) *)
+(*         split. *)
+(*         + apply Forall_app. *)
+(*           * apply forall_removeOnce. *)
+(*             eapply atomic_rqDown_preserves_msg_out_preds; eauto; *)
+(*               [exact msiSv_impl_ORqsInit *)
+(*               |exact msiSv_impl_RqRsSys *)
+(*               |red; auto *)
+(*               |exact msiSvMsgOutPred_good]. *)
+(*           * repeat (constructor; simpl). *)
+(*             red; simpl. *)
+(*             mred; simpl; auto. *)
+(*         + destruct H6; split. *)
+(*           * red in H6; red; simpl in *; mred; simpl. *)
+(*             destruct (oss@[parentIdx]) as [post|] eqn:Hpost; simpl in *; [|auto]. *)
+(*             destruct (oss@[child2Idx]) as [cost2|] eqn:Hcost2; simpl in *; [|auto]. *)
+(*             destruct (orqs@[child2Idx]) as [corq2|] eqn:Hcorq2; simpl in *; [|auto]. *)
+(*             destruct H6 as [[cv ?] ?]. *)
+(*             red in H6; dest. *)
+(*             split. *)
+(*             { exists cv. *)
+(*               red; repeat ssplit. *)
+(*               { solve_rule_conds_ex. } *)
+(*               { solve_rule_conds_ex. } *)
+(*               { solve_rule_conds_ex. } *)
+(*               { solve_rule_conds_ex; solve_msi. } *)
+(*             } *)
+(*             { solve_rule_conds_ex; solve_msi. } *)
+(*           * red in H7; red; simpl in *; mred. *)
 
-      - atomic_cont_exfalso_bound MsiSvMsgOutPred.
-      - atomic_cont_exfalso_bound MsiSvMsgOutPred.
-      - (** [childSetRsM] *)
-        disc_rule_conds_ex.
-        good_footprint_get child1Idx.
-        disc_rule_conds_ex.
+(*       - atomic_cont_exfalso_bound MsiSvMsgOutPred. *)
+(*       - atomic_cont_exfalso_bound MsiSvMsgOutPred. *)
+(*       - (** [childSetRsM] *) *)
+(*         disc_rule_conds_ex. *)
+(*         good_footprint_get child1Idx. *)
+(*         disc_rule_conds_ex. *)
 
-        (* discharge message predicates *)
-        disc_msg_preds H4.
-        disc_rule_conds_ex.
+(*         (* discharge message predicates *) *)
+(*         disc_msg_preds H4. *)
+(*         disc_rule_conds_ex. *)
 
-        (* generate hints for leaves (L1 caches) *)
-        pose proof (parentIdxOf_child_indsOf _ _ H7).
-        dest_in; try discriminate; simpl in *.
-        cbn in H26; inv H26.
+(*         (* generate hints for leaves (L1 caches) *) *)
+(*         pose proof (parentIdxOf_child_indsOf _ _ H7). *)
+(*         dest_in; try discriminate; simpl in *. *)
+(*         cbn in H26; inv H26. *)
 
-        (* construction *)
-        split.
-        + apply Forall_app.
-          * apply forall_removeOnce.
-            eapply atomic_rsDown_preserves_msg_out_preds; eauto;
-              [exact msiSv_impl_ORqsInit
-              |exact msiSv_impl_RqRsSys
-              |red; auto
-              |exact msiSvMsgOutPred_good].
-          * repeat (constructor; simpl).
-        + destruct H6; split.
-          * red in H6; red; simpl in *; mred; simpl.
-            destruct (oss@[child2Idx]) as [cost2|]; simpl in *; [|auto].
-            destruct (orqs@[child2Idx]) as [corq2|]; simpl in *; [|auto].
-            destruct H6 as [[cv ?] ?].
-            red in H6; dest.
-            split.
-            { exists n.
-              red; repeat ssplit.
-              { solve_rule_conds_ex.
-                destruct H6 as [|[|]]; try (exfalso; dest; discriminate).
-                right; right; solve_rule_conds_ex.
-              }
-              { solve_rule_conds_ex. }
-              { solve_rule_conds_ex; solve_msi. }
-              { solve_rule_conds_ex; solve_msi. }
-            }
-            { solve_rule_conds_ex; solve_msi. }
-          * red in H22; red; simpl in *; mred.
+(*         (* construction *) *)
+(*         split. *)
+(*         + apply Forall_app. *)
+(*           * apply forall_removeOnce. *)
+(*             eapply atomic_rsDown_preserves_msg_out_preds; eauto; *)
+(*               [exact msiSv_impl_ORqsInit *)
+(*               |exact msiSv_impl_RqRsSys *)
+(*               |red; auto *)
+(*               |exact msiSvMsgOutPred_good]. *)
+(*           * repeat (constructor; simpl). *)
+(*         + destruct H6; split. *)
+(*           * red in H6; red; simpl in *; mred; simpl. *)
+(*             destruct (oss@[child2Idx]) as [cost2|]; simpl in *; [|auto]. *)
+(*             destruct (orqs@[child2Idx]) as [corq2|]; simpl in *; [|auto]. *)
+(*             destruct H6 as [[cv ?] ?]. *)
+(*             red in H6; dest. *)
+(*             split. *)
+(*             { exists n. *)
+(*               red; repeat ssplit. *)
+(*               { solve_rule_conds_ex. *)
+(*                 destruct H6 as [|[|]]; try (exfalso; dest; discriminate). *)
+(*                 right; right; solve_rule_conds_ex. *)
+(*               } *)
+(*               { solve_rule_conds_ex. } *)
+(*               { solve_rule_conds_ex; solve_msi. } *)
+(*               { solve_rule_conds_ex; solve_msi. } *)
+(*             } *)
+(*             { solve_rule_conds_ex; solve_msi. } *)
+(*           * red in H22; red; simpl in *; mred. *)
 
-      - (** [childDownRqM] *)
-        disc_rule_conds_ex.
+(*       - (** [childDownRqM] *) *)
+(*         disc_rule_conds_ex. *)
 
-        (* construction *)
-        split.
-        + apply Forall_app.
-          * apply forall_removeOnce.
-            eapply atomic_rqDown_preserves_msg_out_preds; eauto;
-              [exact msiSv_impl_ORqsInit
-              |exact msiSv_impl_RqRsSys
-              |red; auto
-              |exact msiSvMsgOutPred_good].
-          * repeat (constructor; simpl).
-            red; simpl.
-            mred; simpl; auto.
-        + destruct H6; split.
-          * red in H6; red; simpl in *; mred; simpl.
-            destruct (oss@[parentIdx]) as [post|] eqn:Hpost; simpl in *; [|auto].
-            destruct (oss@[child2Idx]) as [cost2|] eqn:Hcost2; simpl in *; [|auto].
-            destruct (orqs@[child2Idx]) as [corq2|] eqn:Hcorq2; simpl in *; [|auto].
-            destruct H6 as [[cv ?] ?].
-            red in H6; dest.
-            split.
-            { exists cv.
-              red; repeat ssplit.
-              { solve_rule_conds_ex. }
-              { solve_rule_conds_ex. }
-              { solve_rule_conds_ex. }
-              { solve_rule_conds_ex. }
-            }
-            { solve_rule_conds_ex; solve_msi. }
-          * red in H7; red; simpl in *; mred.
+(*         (* construction *) *)
+(*         split. *)
+(*         + apply Forall_app. *)
+(*           * apply forall_removeOnce. *)
+(*             eapply atomic_rqDown_preserves_msg_out_preds; eauto; *)
+(*               [exact msiSv_impl_ORqsInit *)
+(*               |exact msiSv_impl_RqRsSys *)
+(*               |red; auto *)
+(*               |exact msiSvMsgOutPred_good]. *)
+(*           * repeat (constructor; simpl). *)
+(*             red; simpl. *)
+(*             mred; simpl; auto. *)
+(*         + destruct H6; split. *)
+(*           * red in H6; red; simpl in *; mred; simpl. *)
+(*             destruct (oss@[parentIdx]) as [post|] eqn:Hpost; simpl in *; [|auto]. *)
+(*             destruct (oss@[child2Idx]) as [cost2|] eqn:Hcost2; simpl in *; [|auto]. *)
+(*             destruct (orqs@[child2Idx]) as [corq2|] eqn:Hcorq2; simpl in *; [|auto]. *)
+(*             destruct H6 as [[cv ?] ?]. *)
+(*             red in H6; dest. *)
+(*             split. *)
+(*             { exists cv. *)
+(*               red; repeat ssplit. *)
+(*               { solve_rule_conds_ex. } *)
+(*               { solve_rule_conds_ex. } *)
+(*               { solve_rule_conds_ex. } *)
+(*               { solve_rule_conds_ex. } *)
+(*             } *)
+(*             { solve_rule_conds_ex; solve_msi. } *)
+(*           * red in H7; red; simpl in *; mred. *)
 
-      - atomic_cont_exfalso_bound MsiSvMsgOutPred.
-      - (** [childEvictRsI] *)
-        disc_rule_conds_ex.
-        good_footprint_get child1Idx.
-        disc_rule_conds_ex.
+(*       - atomic_cont_exfalso_bound MsiSvMsgOutPred. *)
+(*       - (** [childEvictRsI] *) *)
+(*         disc_rule_conds_ex. *)
+(*         good_footprint_get child1Idx. *)
+(*         disc_rule_conds_ex. *)
 
-        (* discharge message predicates *)
-        disc_msg_preds H4.
-        disc_rule_conds_ex.
+(*         (* discharge message predicates *) *)
+(*         disc_msg_preds H4. *)
+(*         disc_rule_conds_ex. *)
 
-        (* generate hints for leaves (L1 caches) *)
-        pose proof (parentIdxOf_child_indsOf _ _ H7).
-        dest_in; try discriminate; simpl in *.
-        cbn in H21; inv H21.
+(*         (* generate hints for leaves (L1 caches) *) *)
+(*         pose proof (parentIdxOf_child_indsOf _ _ H7). *)
+(*         dest_in; try discriminate; simpl in *. *)
+(*         cbn in H21; inv H21. *)
 
-        (* construction *)
-        split.
-        + apply Forall_app.
-          * apply forall_removeOnce.
-            eapply atomic_rsDown_preserves_msg_out_preds; eauto;
-              [exact msiSv_impl_ORqsInit
-              |exact msiSv_impl_RqRsSys
-              |red; auto
-              |exact msiSvMsgOutPred_good].
-          * repeat (constructor; simpl).
-        + destruct H6; split.
-          * red in H6; red; simpl in *; mred; simpl.
-            rename porq into orq.
-            destruct (oss@[child2Idx]) as [cost2|]; simpl in *; [|auto].
-            destruct (orqs@[child2Idx]) as [corq2|]; simpl in *; [|auto].
-            destruct H6 as [[cv ?] ?].
-            red in H6; dest.
-            split.
-            { exists cv.
-              red; repeat ssplit.
-              { solve_rule_conds_ex. }
-              { solve_rule_conds_ex; solve_msi. }
-              { solve_rule_conds_ex. }
-              { solve_rule_conds_ex. }
-            }
-            { solve_rule_conds_ex; solve_msi. }
-          * red in H20; red; simpl in *; mred.
+(*         (* construction *) *)
+(*         split. *)
+(*         + apply Forall_app. *)
+(*           * apply forall_removeOnce. *)
+(*             eapply atomic_rsDown_preserves_msg_out_preds; eauto; *)
+(*               [exact msiSv_impl_ORqsInit *)
+(*               |exact msiSv_impl_RqRsSys *)
+(*               |red; auto *)
+(*               |exact msiSvMsgOutPred_good]. *)
+(*           * repeat (constructor; simpl). *)
+(*         + destruct H6; split. *)
+(*           * red in H6; red; simpl in *; mred; simpl. *)
+(*             rename porq into orq. *)
+(*             destruct (oss@[child2Idx]) as [cost2|]; simpl in *; [|auto]. *)
+(*             destruct (orqs@[child2Idx]) as [corq2|]; simpl in *; [|auto]. *)
+(*             destruct H6 as [[cv ?] ?]. *)
+(*             red in H6; dest. *)
+(*             split. *)
+(*             { exists cv. *)
+(*               red; repeat ssplit. *)
+(*               { solve_rule_conds_ex. } *)
+(*               { solve_rule_conds_ex; solve_msi. } *)
+(*               { solve_rule_conds_ex. } *)
+(*               { solve_rule_conds_ex. } *)
+(*             } *)
+(*             { solve_rule_conds_ex; solve_msi. } *)
+(*           * red in H20; red; simpl in *; mred. *)
 
-      (** child2 *)
-      - atomic_cont_exfalso_bound MsiSvMsgOutPred.
-      - atomic_cont_exfalso_bound MsiSvMsgOutPred.
+(*       (** child2 *) *)
+(*       - atomic_cont_exfalso_bound MsiSvMsgOutPred. *)
+(*       - atomic_cont_exfalso_bound MsiSvMsgOutPred. *)
 
-      - (** [childGetRsS] *)
-        disc_rule_conds_ex.
-        good_footprint_get child2Idx.
-        disc_rule_conds_ex.
+(*       - (** [childGetRsS] *) *)
+(*         disc_rule_conds_ex. *)
+(*         good_footprint_get child2Idx. *)
+(*         disc_rule_conds_ex. *)
 
-        (* discharge message predicates *)
-        disc_msg_preds H4.
-        disc_rule_conds_ex.
+(*         (* discharge message predicates *) *)
+(*         disc_msg_preds H4. *)
+(*         disc_rule_conds_ex. *)
 
-        (* generate hints for leaves (L1 caches) *)
-        pose proof (parentIdxOf_child_indsOf _ _ H7).
-        dest_in; try discriminate; simpl in *.
-        cbn in H26; inv H26.
+(*         (* generate hints for leaves (L1 caches) *) *)
+(*         pose proof (parentIdxOf_child_indsOf _ _ H7). *)
+(*         dest_in; try discriminate; simpl in *. *)
+(*         cbn in H26; inv H26. *)
 
-        (* construction *)
-        split.
-        + apply Forall_app.
-          * apply forall_removeOnce.
-            eapply atomic_rsDown_preserves_msg_out_preds; eauto;
-              [exact msiSv_impl_ORqsInit
-              |exact msiSv_impl_RqRsSys
-              |red; auto
-              |exact msiSvMsgOutPred_good].
-          * repeat (constructor; simpl).
-        + destruct H6; split.
-          * red in H6; red; simpl in *; mred; simpl.
-            destruct (oss@[child1Idx]) as [cost1|]; simpl in *; [|auto].
-            destruct (orqs@[child1Idx]) as [corq1|]; simpl in *; [|auto].
-            destruct H6 as [[cv ?] ?].
-            red in H6; dest.
-            split.
-            { exists val0.
-              red; repeat ssplit.
-              { solve_rule_conds_ex; solve_msi. }
-              { solve_rule_conds_ex; solve_msi. }
-              { solve_rule_conds_ex. }
-              { solve_rule_conds_ex; solve_msi. }
-            }
-            { solve_rule_conds_ex; solve_msi. }
-          * red in H22; red; simpl in *; mred.
+(*         (* construction *) *)
+(*         split. *)
+(*         + apply Forall_app. *)
+(*           * apply forall_removeOnce. *)
+(*             eapply atomic_rsDown_preserves_msg_out_preds; eauto; *)
+(*               [exact msiSv_impl_ORqsInit *)
+(*               |exact msiSv_impl_RqRsSys *)
+(*               |red; auto *)
+(*               |exact msiSvMsgOutPred_good]. *)
+(*           * repeat (constructor; simpl). *)
+(*         + destruct H6; split. *)
+(*           * red in H6; red; simpl in *; mred; simpl. *)
+(*             destruct (oss@[child1Idx]) as [cost1|]; simpl in *; [|auto]. *)
+(*             destruct (orqs@[child1Idx]) as [corq1|]; simpl in *; [|auto]. *)
+(*             destruct H6 as [[cv ?] ?]. *)
+(*             red in H6; dest. *)
+(*             split. *)
+(*             { exists val0. *)
+(*               red; repeat ssplit. *)
+(*               { solve_rule_conds_ex; solve_msi. } *)
+(*               { solve_rule_conds_ex; solve_msi. } *)
+(*               { solve_rule_conds_ex. } *)
+(*               { solve_rule_conds_ex; solve_msi. } *)
+(*             } *)
+(*             { solve_rule_conds_ex; solve_msi. } *)
+(*           * red in H22; red; simpl in *; mred. *)
 
-      - (** [childDownRqS] *)
-        disc_rule_conds_ex.
+(*       - (** [childDownRqS] *) *)
+(*         disc_rule_conds_ex. *)
 
-        (* construction *)
-        split.
-        + apply Forall_app.
-          * apply forall_removeOnce.
-            eapply atomic_rqDown_preserves_msg_out_preds; eauto;
-              [exact msiSv_impl_ORqsInit
-              |exact msiSv_impl_RqRsSys
-              |red; auto
-              |exact msiSvMsgOutPred_good].
-          * repeat (constructor; simpl).
-            red; simpl.
-            mred; simpl; auto.
-        + destruct H6; split.
-          * red in H6; red; simpl in *; mred; simpl.
-            destruct (oss@[parentIdx]) as [post|] eqn:Hpost; simpl in *; [|auto].
-            destruct (oss@[child1Idx]) as [cost1|] eqn:Hcost1; simpl in *; [|auto].
-            destruct (orqs@[child1Idx]) as [corq1|] eqn:Hcorq1; simpl in *; [|auto].
-            destruct H6 as [[cv ?] [? ?]].
-            red in H6; dest.
-            split.
-            { exists cv.
-              red; repeat ssplit.
-              { solve_rule_conds_ex. }
-              { solve_rule_conds_ex. }
-              { solve_rule_conds_ex. }
-              { solve_rule_conds_ex; solve_msi. }
-            }
-            { solve_rule_conds_ex; solve_msi. }
-          * red in H7; red; simpl in *; mred.
+(*         (* construction *) *)
+(*         split. *)
+(*         + apply Forall_app. *)
+(*           * apply forall_removeOnce. *)
+(*             eapply atomic_rqDown_preserves_msg_out_preds; eauto; *)
+(*               [exact msiSv_impl_ORqsInit *)
+(*               |exact msiSv_impl_RqRsSys *)
+(*               |red; auto *)
+(*               |exact msiSvMsgOutPred_good]. *)
+(*           * repeat (constructor; simpl). *)
+(*             red; simpl. *)
+(*             mred; simpl; auto. *)
+(*         + destruct H6; split. *)
+(*           * red in H6; red; simpl in *; mred; simpl. *)
+(*             destruct (oss@[parentIdx]) as [post|] eqn:Hpost; simpl in *; [|auto]. *)
+(*             destruct (oss@[child1Idx]) as [cost1|] eqn:Hcost1; simpl in *; [|auto]. *)
+(*             destruct (orqs@[child1Idx]) as [corq1|] eqn:Hcorq1; simpl in *; [|auto]. *)
+(*             destruct H6 as [[cv ?] [? ?]]. *)
+(*             red in H6; dest. *)
+(*             split. *)
+(*             { exists cv. *)
+(*               red; repeat ssplit. *)
+(*               { solve_rule_conds_ex. } *)
+(*               { solve_rule_conds_ex. } *)
+(*               { solve_rule_conds_ex. } *)
+(*               { solve_rule_conds_ex; solve_msi. } *)
+(*             } *)
+(*             { solve_rule_conds_ex; solve_msi. } *)
+(*           * red in H7; red; simpl in *; mred. *)
         
-      - atomic_cont_exfalso_bound MsiSvMsgOutPred.
-      - atomic_cont_exfalso_bound MsiSvMsgOutPred.
-      - (** [childSetRsM] *)
-        disc_rule_conds_ex.
-        good_footprint_get child2Idx.
-        disc_rule_conds_ex.
+(*       - atomic_cont_exfalso_bound MsiSvMsgOutPred. *)
+(*       - atomic_cont_exfalso_bound MsiSvMsgOutPred. *)
+(*       - (** [childSetRsM] *) *)
+(*         disc_rule_conds_ex. *)
+(*         good_footprint_get child2Idx. *)
+(*         disc_rule_conds_ex. *)
 
-        (* discharge message predicates *)
-        disc_msg_preds H4.
-        disc_rule_conds_ex.
+(*         (* discharge message predicates *) *)
+(*         disc_msg_preds H4. *)
+(*         disc_rule_conds_ex. *)
 
-        (* generate hints for leaves (L1 caches) *)
-        pose proof (parentIdxOf_child_indsOf _ _ H7).
-        dest_in; try discriminate; simpl in *.
-        cbn in H26; inv H26.
+(*         (* generate hints for leaves (L1 caches) *) *)
+(*         pose proof (parentIdxOf_child_indsOf _ _ H7). *)
+(*         dest_in; try discriminate; simpl in *. *)
+(*         cbn in H26; inv H26. *)
 
-        (* construction *)
-        split.
-        + apply Forall_app.
-          * apply forall_removeOnce.
-            eapply atomic_rsDown_preserves_msg_out_preds; eauto;
-              [exact msiSv_impl_ORqsInit
-              |exact msiSv_impl_RqRsSys
-              |red; auto
-              |exact msiSvMsgOutPred_good].
-          * repeat (constructor; simpl).
-        + destruct H6; split.
-          * red in H6; red; simpl in *; mred; simpl.
-            destruct (oss@[child1Idx]) as [cost1|]; simpl in *; [|auto].
-            destruct (orqs@[child1Idx]) as [corq1|]; simpl in *; [|auto].
-            destruct H6 as [[cv ?] ?].
-            red in H6; dest.
-            split.
-            { exists n.
-              red; repeat ssplit.
-              { solve_rule_conds_ex.
-                destruct H6 as [|[|]]; try (exfalso; dest; discriminate).
-                right; right; solve_rule_conds_ex.
-              }
-              { solve_rule_conds_ex; solve_msi. }
-              { solve_rule_conds_ex. }
-              { solve_rule_conds_ex; solve_msi. }
-            }
-            { solve_rule_conds_ex; solve_msi. }
-          * red in H22; red; simpl in *; mred.
+(*         (* construction *) *)
+(*         split. *)
+(*         + apply Forall_app. *)
+(*           * apply forall_removeOnce. *)
+(*             eapply atomic_rsDown_preserves_msg_out_preds; eauto; *)
+(*               [exact msiSv_impl_ORqsInit *)
+(*               |exact msiSv_impl_RqRsSys *)
+(*               |red; auto *)
+(*               |exact msiSvMsgOutPred_good]. *)
+(*           * repeat (constructor; simpl). *)
+(*         + destruct H6; split. *)
+(*           * red in H6; red; simpl in *; mred; simpl. *)
+(*             destruct (oss@[child1Idx]) as [cost1|]; simpl in *; [|auto]. *)
+(*             destruct (orqs@[child1Idx]) as [corq1|]; simpl in *; [|auto]. *)
+(*             destruct H6 as [[cv ?] ?]. *)
+(*             red in H6; dest. *)
+(*             split. *)
+(*             { exists n. *)
+(*               red; repeat ssplit. *)
+(*               { solve_rule_conds_ex. *)
+(*                 destruct H6 as [|[|]]; try (exfalso; dest; discriminate). *)
+(*                 right; right; solve_rule_conds_ex. *)
+(*               } *)
+(*               { solve_rule_conds_ex; solve_msi. } *)
+(*               { solve_rule_conds_ex. } *)
+(*               { solve_rule_conds_ex; solve_msi. } *)
+(*             } *)
+(*             { solve_rule_conds_ex; solve_msi. } *)
+(*           * red in H22; red; simpl in *; mred. *)
           
-      - (** [childDownRqM] *)
-        disc_rule_conds_ex.
+(*       - (** [childDownRqM] *) *)
+(*         disc_rule_conds_ex. *)
 
-        (* construction *)
-        split.
-        + apply Forall_app.
-          * apply forall_removeOnce.
-            eapply atomic_rqDown_preserves_msg_out_preds; eauto;
-              [exact msiSv_impl_ORqsInit
-              |exact msiSv_impl_RqRsSys
-              |red; auto
-              |exact msiSvMsgOutPred_good].
-          * repeat (constructor; simpl).
-            red; simpl.
-            mred; simpl; auto.
-        + destruct H6; split.
-          * red in H6; red; simpl in *; mred; simpl.
-            destruct (oss@[parentIdx]) as [post|] eqn:Hpost; simpl in *; [|auto].
-            destruct (oss@[child1Idx]) as [cost1|] eqn:Hcost1; simpl in *; [|auto].
-            destruct (orqs@[child1Idx]) as [corq1|] eqn:Hcorq1; simpl in *; [|auto].
-            destruct H6 as [[cv ?] [? ?]].
-            red in H6; dest.
-            split.
-            { exists cv.
-              red; repeat ssplit.
-              { solve_rule_conds_ex. }
-              { solve_rule_conds_ex. }
-              { solve_rule_conds_ex. }
-              { solve_rule_conds_ex. }
-            }
-            { solve_rule_conds_ex; solve_msi. }
-          * red in H7; red; simpl in *; mred.
+(*         (* construction *) *)
+(*         split. *)
+(*         + apply Forall_app. *)
+(*           * apply forall_removeOnce. *)
+(*             eapply atomic_rqDown_preserves_msg_out_preds; eauto; *)
+(*               [exact msiSv_impl_ORqsInit *)
+(*               |exact msiSv_impl_RqRsSys *)
+(*               |red; auto *)
+(*               |exact msiSvMsgOutPred_good]. *)
+(*           * repeat (constructor; simpl). *)
+(*             red; simpl. *)
+(*             mred; simpl; auto. *)
+(*         + destruct H6; split. *)
+(*           * red in H6; red; simpl in *; mred; simpl. *)
+(*             destruct (oss@[parentIdx]) as [post|] eqn:Hpost; simpl in *; [|auto]. *)
+(*             destruct (oss@[child1Idx]) as [cost1|] eqn:Hcost1; simpl in *; [|auto]. *)
+(*             destruct (orqs@[child1Idx]) as [corq1|] eqn:Hcorq1; simpl in *; [|auto]. *)
+(*             destruct H6 as [[cv ?] [? ?]]. *)
+(*             red in H6; dest. *)
+(*             split. *)
+(*             { exists cv. *)
+(*               red; repeat ssplit. *)
+(*               { solve_rule_conds_ex. } *)
+(*               { solve_rule_conds_ex. } *)
+(*               { solve_rule_conds_ex. } *)
+(*               { solve_rule_conds_ex. } *)
+(*             } *)
+(*             { solve_rule_conds_ex; solve_msi. } *)
+(*           * red in H7; red; simpl in *; mred. *)
 
-      - atomic_cont_exfalso_bound MsiSvMsgOutPred.
-      - (** [childEvictRsI] *)
-        disc_rule_conds_ex.
-        good_footprint_get child2Idx.
-        disc_rule_conds_ex.
+(*       - atomic_cont_exfalso_bound MsiSvMsgOutPred. *)
+(*       - (** [childEvictRsI] *) *)
+(*         disc_rule_conds_ex. *)
+(*         good_footprint_get child2Idx. *)
+(*         disc_rule_conds_ex. *)
 
-        (* discharge message predicates *)
-        disc_msg_preds H4.
-        disc_rule_conds_ex.
+(*         (* discharge message predicates *) *)
+(*         disc_msg_preds H4. *)
+(*         disc_rule_conds_ex. *)
 
-        (* generate hints for leaves (L1 caches) *)
-        pose proof (parentIdxOf_child_indsOf _ _ H7).
-        dest_in; try discriminate; simpl in *.
-        cbn in H21; inv H21.
+(*         (* generate hints for leaves (L1 caches) *) *)
+(*         pose proof (parentIdxOf_child_indsOf _ _ H7). *)
+(*         dest_in; try discriminate; simpl in *. *)
+(*         cbn in H21; inv H21. *)
 
-        (* construction *)
-        split.
-        + apply Forall_app.
-          * apply forall_removeOnce.
-            eapply atomic_rsDown_preserves_msg_out_preds; eauto;
-              [exact msiSv_impl_ORqsInit
-              |exact msiSv_impl_RqRsSys
-              |red; auto
-              |exact msiSvMsgOutPred_good].
-          * repeat (constructor; simpl).
-        + destruct H6; split.
-          * red in H6; red; simpl in *; mred; simpl.
-            rename porq into orq.
-            destruct (oss@[child1Idx]) as [cost1|]; simpl in *; [|auto].
-            destruct (orqs@[child1Idx]) as [corq1|]; simpl in *; [|auto].
-            destruct H6 as [[cv ?] ?].
-            red in H6; dest.
-            split.
-            { exists cv.
-              red; repeat ssplit.
-              { solve_rule_conds_ex. }
-              { solve_rule_conds_ex. }
-              { solve_rule_conds_ex; solve_msi. }
-              { solve_rule_conds_ex. }
-            }
-            { solve_rule_conds_ex; solve_msi. }
-          * red in H20; red; simpl in *; mred.
+(*         (* construction *) *)
+(*         split. *)
+(*         + apply Forall_app. *)
+(*           * apply forall_removeOnce. *)
+(*             eapply atomic_rsDown_preserves_msg_out_preds; eauto; *)
+(*               [exact msiSv_impl_ORqsInit *)
+(*               |exact msiSv_impl_RqRsSys *)
+(*               |red; auto *)
+(*               |exact msiSvMsgOutPred_good]. *)
+(*           * repeat (constructor; simpl). *)
+(*         + destruct H6; split. *)
+(*           * red in H6; red; simpl in *; mred; simpl. *)
+(*             rename porq into orq. *)
+(*             destruct (oss@[child1Idx]) as [cost1|]; simpl in *; [|auto]. *)
+(*             destruct (orqs@[child1Idx]) as [corq1|]; simpl in *; [|auto]. *)
+(*             destruct H6 as [[cv ?] ?]. *)
+(*             red in H6; dest. *)
+(*             split. *)
+(*             { exists cv. *)
+(*               red; repeat ssplit. *)
+(*               { solve_rule_conds_ex. } *)
+(*               { solve_rule_conds_ex. } *)
+(*               { solve_rule_conds_ex; solve_msi. } *)
+(*               { solve_rule_conds_ex. } *)
+(*             } *)
+(*             { solve_rule_conds_ex; solve_msi. } *)
+(*           * red in H20; red; simpl in *; mred. *)
 
-      (** parent(child1) *)
+(*       (** parent(child1) *) *)
 
-      - (** [parentGetRqImm] *)
-        disc_rule_conds_ex.
+(*       - (** [parentGetRqImm] *) *)
+(*         disc_rule_conds_ex. *)
 
-        split.
-        + apply Forall_app.
-          * apply forall_removeOnce.
-            eapply atomic_rqUp_preserves_msg_out_preds with (oidx:= child1Idx);
-              [exact msiSv_impl_ORqsInit
-              |exact msiSv_impl_RqRsSys|..]; eauto.
-            { intro; dest_in; discriminate. }
-            { red; auto. }
-            { exact msiSvMsgOutPred_good. }
-          * repeat (constructor; simpl).
-            red; repeat (simpl; mred).
-        + destruct H6; split.
-          * red in H6; red; simpl in *; mred; simpl.
-            destruct (oss@[child1Idx]) as [cost1|] eqn:Hcost1; simpl in *; [|auto].
-            destruct (oss@[child2Idx]) as [cost2|] eqn:Hcost2; simpl in *; [|auto].
-            destruct (orqs@[child1Idx]) as [corq1|] eqn:Hcorq1; simpl in *; [|auto].
-            destruct (orqs@[child2Idx]) as [corq2|] eqn:Hcorq2; simpl in *; [|auto].
-            destruct H6 as [[cv ?] ?].
-            red in H6; dest.
-            split.
-            { exists cv.
-              red; repeat ssplit.
-              { solve_rule_conds_ex.
-                right; left.
-                destruct H6 as [|[|]].
-                { solve_rule_conds_ex; solve_msi. }
-                { solve_rule_conds_ex. }
-                { solve_msi. }
-              }
-              { solve_rule_conds_ex. }
-              { solve_rule_conds_ex. }
-              { solve_rule_conds_ex. }
-            }
-            { disc_rule_conds_ex.
-              assert (In (child child1Idx ec1 ce1 c1pRq c1pRs pc1) (sys_objs impl))
-                by (simpl; tauto).
-              good_locking_get (child child1Idx ec1 ce1 c1pRq c1pRs pc1).
-              clear H24.
-              eapply upLockInvORq_rqUp_length_one_locked in H26; try reflexivity;
-                [|eapply findQ_length_ge_one; apply FirstMP_InMP; eassumption].
-              solve_rule_conds_ex.
-            }
-          * red in H7; red; simpl in *; mred.
+(*         split. *)
+(*         + apply Forall_app. *)
+(*           * apply forall_removeOnce. *)
+(*             eapply atomic_rqUp_preserves_msg_out_preds with (oidx:= child1Idx); *)
+(*               [exact msiSv_impl_ORqsInit *)
+(*               |exact msiSv_impl_RqRsSys|..]; eauto. *)
+(*             { intro; dest_in; discriminate. } *)
+(*             { red; auto. } *)
+(*             { exact msiSvMsgOutPred_good. } *)
+(*           * repeat (constructor; simpl). *)
+(*             red; repeat (simpl; mred). *)
+(*         + destruct H6; split. *)
+(*           * red in H6; red; simpl in *; mred; simpl. *)
+(*             destruct (oss@[child1Idx]) as [cost1|] eqn:Hcost1; simpl in *; [|auto]. *)
+(*             destruct (oss@[child2Idx]) as [cost2|] eqn:Hcost2; simpl in *; [|auto]. *)
+(*             destruct (orqs@[child1Idx]) as [corq1|] eqn:Hcorq1; simpl in *; [|auto]. *)
+(*             destruct (orqs@[child2Idx]) as [corq2|] eqn:Hcorq2; simpl in *; [|auto]. *)
+(*             destruct H6 as [[cv ?] ?]. *)
+(*             red in H6; dest. *)
+(*             split. *)
+(*             { exists cv. *)
+(*               red; repeat ssplit. *)
+(*               { solve_rule_conds_ex. *)
+(*                 right; left. *)
+(*                 destruct H6 as [|[|]]. *)
+(*                 { solve_rule_conds_ex; solve_msi. } *)
+(*                 { solve_rule_conds_ex. } *)
+(*                 { solve_msi. } *)
+(*               } *)
+(*               { solve_rule_conds_ex. } *)
+(*               { solve_rule_conds_ex. } *)
+(*               { solve_rule_conds_ex. } *)
+(*             } *)
+(*             { disc_rule_conds_ex. *)
+(*               assert (In (child child1Idx ec1 ce1 c1pRq c1pRs pc1) (sys_objs impl)) *)
+(*                 by (simpl; tauto). *)
+(*               good_locking_get (child child1Idx ec1 ce1 c1pRq c1pRs pc1). *)
+(*               clear H24. *)
+(*               eapply upLockInvORq_rqUp_length_one_locked in H26; try reflexivity; *)
+(*                 [|eapply findQ_length_ge_one; apply FirstMP_InMP; eassumption]. *)
+(*               solve_rule_conds_ex. *)
+(*             } *)
+(*           * red in H7; red; simpl in *; mred. *)
 
-      - (** [parentGetDownRqS] *)
-        disc_rule_conds_ex.
+(*       - (** [parentGetDownRqS] *) *)
+(*         disc_rule_conds_ex. *)
 
-        split.
-        + apply Forall_app.
-          * apply forall_removeOnce.
-            eapply atomic_rqUp_preserves_msg_out_preds with (oidx:= child1Idx);
-              [exact msiSv_impl_ORqsInit
-              |exact msiSv_impl_RqRsSys|..]; eauto.
-            { intro; dest_in; discriminate. }
-            { red; auto. }
-            { exact msiSvMsgOutPred_good. }
-          * repeat (constructor; simpl).
-        + destruct H6; split.
-          * red in H6; red; simpl in *; mred.
-          * solve_rule_conds_ex.
+(*         split. *)
+(*         + apply Forall_app. *)
+(*           * apply forall_removeOnce. *)
+(*             eapply atomic_rqUp_preserves_msg_out_preds with (oidx:= child1Idx); *)
+(*               [exact msiSv_impl_ORqsInit *)
+(*               |exact msiSv_impl_RqRsSys|..]; eauto. *)
+(*             { intro; dest_in; discriminate. } *)
+(*             { red; auto. } *)
+(*             { exact msiSvMsgOutPred_good. } *)
+(*           * repeat (constructor; simpl). *)
+(*         + destruct H6; split. *)
+(*           * red in H6; red; simpl in *; mred. *)
+(*           * solve_rule_conds_ex. *)
 
-      - (** [parentSetRqImm] *)
-        disc_rule_conds_ex.
+(*       - (** [parentSetRqImm] *) *)
+(*         disc_rule_conds_ex. *)
 
-        split.
-        + apply Forall_app.
-          * apply forall_removeOnce.
-            eapply atomic_rqUp_preserves_msg_out_preds with (oidx:= child1Idx);
-              [exact msiSv_impl_ORqsInit
-              |exact msiSv_impl_RqRsSys|..]; eauto.
-            { intro; dest_in; discriminate. }
-            { red; auto. }
-            { exact msiSvMsgOutPred_good. }
-          * repeat (constructor; simpl).
-            red; repeat (simpl; mred).
-        + destruct H6; split.
-          * red in H6; red; simpl in *; mred; simpl.
-            destruct (oss@[child1Idx]) as [cost1|] eqn:Hcost1; simpl in *; [|auto].
-            destruct (oss@[child2Idx]) as [cost2|] eqn:Hcost2; simpl in *; [|auto].
-            destruct (orqs@[child1Idx]) as [corq1|] eqn:Hcorq1; simpl in *; [|auto].
-            destruct (orqs@[child2Idx]) as [corq2|] eqn:Hcorq2; simpl in *; [|auto].
-            destruct H6 as [[cv ?] ?].
-            red in H6; dest.
-            unfold getDir in H13; simpl in H13.
+(*         split. *)
+(*         + apply Forall_app. *)
+(*           * apply forall_removeOnce. *)
+(*             eapply atomic_rqUp_preserves_msg_out_preds with (oidx:= child1Idx); *)
+(*               [exact msiSv_impl_ORqsInit *)
+(*               |exact msiSv_impl_RqRsSys|..]; eauto. *)
+(*             { intro; dest_in; discriminate. } *)
+(*             { red; auto. } *)
+(*             { exact msiSvMsgOutPred_good. } *)
+(*           * repeat (constructor; simpl). *)
+(*             red; repeat (simpl; mred). *)
+(*         + destruct H6; split. *)
+(*           * red in H6; red; simpl in *; mred; simpl. *)
+(*             destruct (oss@[child1Idx]) as [cost1|] eqn:Hcost1; simpl in *; [|auto]. *)
+(*             destruct (oss@[child2Idx]) as [cost2|] eqn:Hcost2; simpl in *; [|auto]. *)
+(*             destruct (orqs@[child1Idx]) as [corq1|] eqn:Hcorq1; simpl in *; [|auto]. *)
+(*             destruct (orqs@[child2Idx]) as [corq2|] eqn:Hcorq2; simpl in *; [|auto]. *)
+(*             destruct H6 as [[cv ?] ?]. *)
+(*             red in H6; dest. *)
+(*             unfold getDir in H13; simpl in H13. *)
 
-            split.
-            { exists cv.
-              red; repeat ssplit.
-              { solve_rule_conds_ex.
-                right; right; auto.
-              }
-              { solve_rule_conds_ex. }
-              { solve_rule_conds_ex. }
-              { solve_rule_conds_ex. }
-            }
-            { disc_rule_conds_ex.
-              assert (In (child child1Idx ec1 ce1 c1pRq c1pRs pc1) (sys_objs impl))
-                by (simpl; tauto).
-              good_locking_get (child child1Idx ec1 ce1 c1pRq c1pRs pc1).
-              clear H24.
-              eapply upLockInvORq_rqUp_length_one_locked in H26; try reflexivity;
-                [|eapply findQ_length_ge_one; apply FirstMP_InMP; eassumption].
-              solve_rule_conds_ex.
-            }
-          * red in H7; red; simpl in *; mred.
+(*             split. *)
+(*             { exists cv. *)
+(*               red; repeat ssplit. *)
+(*               { solve_rule_conds_ex. *)
+(*                 right; right; auto. *)
+(*               } *)
+(*               { solve_rule_conds_ex. } *)
+(*               { solve_rule_conds_ex. } *)
+(*               { solve_rule_conds_ex. } *)
+(*             } *)
+(*             { disc_rule_conds_ex. *)
+(*               assert (In (child child1Idx ec1 ce1 c1pRq c1pRs pc1) (sys_objs impl)) *)
+(*                 by (simpl; tauto). *)
+(*               good_locking_get (child child1Idx ec1 ce1 c1pRq c1pRs pc1). *)
+(*               clear H24. *)
+(*               eapply upLockInvORq_rqUp_length_one_locked in H26; try reflexivity; *)
+(*                 [|eapply findQ_length_ge_one; apply FirstMP_InMP; eassumption]. *)
+(*               solve_rule_conds_ex. *)
+(*             } *)
+(*           * red in H7; red; simpl in *; mred. *)
 
-      - (** [parentSetDownRqM] *)
-        disc_rule_conds_ex.
+(*       - (** [parentSetDownRqM] *) *)
+(*         disc_rule_conds_ex. *)
 
-        split.
-        + apply Forall_app.
-          * apply forall_removeOnce.
-            eapply atomic_rqUp_preserves_msg_out_preds with (oidx:= child1Idx);
-              [exact msiSv_impl_ORqsInit
-              |exact msiSv_impl_RqRsSys|..]; eauto.
-            { intro; dest_in; discriminate. }
-            { red; auto. }
-            { exact msiSvMsgOutPred_good. }
-          * repeat (constructor; simpl).
-        + destruct H6; split.
-          * red in H6; red; simpl in *; mred.
-          * solve_rule_conds_ex.
+(*         split. *)
+(*         + apply Forall_app. *)
+(*           * apply forall_removeOnce. *)
+(*             eapply atomic_rqUp_preserves_msg_out_preds with (oidx:= child1Idx); *)
+(*               [exact msiSv_impl_ORqsInit *)
+(*               |exact msiSv_impl_RqRsSys|..]; eauto. *)
+(*             { intro; dest_in; discriminate. } *)
+(*             { red; auto. } *)
+(*             { exact msiSvMsgOutPred_good. } *)
+(*           * repeat (constructor; simpl). *)
+(*         + destruct H6; split. *)
+(*           * red in H6; red; simpl in *; mred. *)
+(*           * solve_rule_conds_ex. *)
 
-      - (** [parentGetDownRsS] *)
-        disc_rule_conds_ex.
+(*       - (** [parentGetDownRsS] *) *)
+(*         disc_rule_conds_ex. *)
 
-        (* discharge the lock invariant *)
-        destruct H6.
-        red in H8; simpl in H8.
-        disc_rule_conds_const.
-        red in H8.
-        disc_rule_conds_const.
-        destruct H8; dest; [|discriminate].
-        rewrite H10 in *.
+(*         (* discharge the lock invariant *) *)
+(*         destruct H6. *)
+(*         red in H8; simpl in H8. *)
+(*         disc_rule_conds_const. *)
+(*         red in H8. *)
+(*         disc_rule_conds_const. *)
+(*         destruct H8; dest; [|discriminate]. *)
+(*         rewrite H10 in *. *)
 
-        (* discharge message predicates *)
-        disc_msg_preds H4.
-        disc_rule_conds_ex.
+(*         (* discharge message predicates *) *)
+(*         disc_msg_preds H4. *)
+(*         disc_rule_conds_ex. *)
         
-        split.
-        + apply Forall_app.
-          * apply forall_removeOnce.
-            eapply atomic_rsUps_preserves_msg_out_preds
-              with (rsUps:= [(c2pRs, rmsg)]); eauto.
-            { exact msiSv_impl_ORqsInit. }
-            { exact msiSv_impl_RqRsSys. }
-            { repeat constructor; intro; dest_in. }
-            { apply SubList_cons; [|apply SubList_nil].
-              assumption.
-            }
-            { instantiate (1:= fun _ => True).
-              instantiate (1:= [pc2]).
-              repeat split.
-              { discriminate. }
-              { repeat constructor.
-                simpl; exists child2Idx.
-                repeat split.
-              }
-            }
-            { exact msiSvMsgOutPred_good. }
-          * repeat (constructor; simpl).
-            red; simpl.
-            solve_rule_conds_ex.
-        + split.
-          * red in H6; red; simpl in *; mred; simpl.
-            destruct (oss@[child1Idx]) as [cost1|] eqn:Hcost1; simpl in *; [|auto].
-            destruct (orqs@[child1Idx]) as [corq1|] eqn:Hcorq1; simpl in *; [|auto].
-            destruct (orqs@[child2Idx]) as [corq2|] eqn:Hcorq2; simpl in *; [|auto].
-            destruct H6 as [[cv ?] ?].
-            red in H6; dest.
+(*         split. *)
+(*         + apply Forall_app. *)
+(*           * apply forall_removeOnce. *)
+(*             eapply atomic_rsUps_preserves_msg_out_preds *)
+(*               with (rsUps:= [(c2pRs, rmsg)]); eauto. *)
+(*             { exact msiSv_impl_ORqsInit. } *)
+(*             { exact msiSv_impl_RqRsSys. } *)
+(*             { repeat constructor; intro; dest_in. } *)
+(*             { apply SubList_cons; [|apply SubList_nil]. *)
+(*               assumption. *)
+(*             } *)
+(*             { instantiate (1:= fun _ => True). *)
+(*               instantiate (1:= [pc2]). *)
+(*               repeat split. *)
+(*               { discriminate. } *)
+(*               { repeat constructor. *)
+(*                 simpl; exists child2Idx. *)
+(*                 repeat split. *)
+(*               } *)
+(*             } *)
+(*             { exact msiSvMsgOutPred_good. } *)
+(*           * repeat (constructor; simpl). *)
+(*             red; simpl. *)
+(*             solve_rule_conds_ex. *)
+(*         + split. *)
+(*           * red in H6; red; simpl in *; mred; simpl. *)
+(*             destruct (oss@[child1Idx]) as [cost1|] eqn:Hcost1; simpl in *; [|auto]. *)
+(*             destruct (orqs@[child1Idx]) as [corq1|] eqn:Hcorq1; simpl in *; [|auto]. *)
+(*             destruct (orqs@[child2Idx]) as [corq2|] eqn:Hcorq2; simpl in *; [|auto]. *)
+(*             destruct H6 as [[cv ?] ?]. *)
+(*             red in H6; dest. *)
 
-            assert (In (child child1Idx ec1 ce1 c1pRq c1pRs pc1) (sys_objs impl))
-              by (simpl; tauto).
-            good_locking_get (child child1Idx ec1 ce1 c1pRq c1pRs pc1).
-            clear H21.
-            eapply upLockInvORq_parent_locked_locked in H22; try reflexivity;
-              [|red; repeat (simpl; mred); eauto]; dest.
+(*             assert (In (child child1Idx ec1 ce1 c1pRq c1pRs pc1) (sys_objs impl)) *)
+(*               by (simpl; tauto). *)
+(*             good_locking_get (child child1Idx ec1 ce1 c1pRq c1pRs pc1). *)
+(*             clear H21. *)
+(*             eapply upLockInvORq_parent_locked_locked in H22; try reflexivity; *)
+(*               [|red; repeat (simpl; mred); eauto]; dest. *)
           
-            split.
-            { exists val0.
-              red; repeat ssplit.
-              { solve_rule_conds_ex.
-                right; left; auto.
-              }
-              { solve_rule_conds_ex. }
-              { solve_rule_conds_ex. }
-              { solve_rule_conds_ex. }
-            }
-            { solve_rule_conds_ex. }
-          * solve_rule_conds_ex.
+(*             split. *)
+(*             { exists val0. *)
+(*               red; repeat ssplit. *)
+(*               { solve_rule_conds_ex. *)
+(*                 right; left; auto. *)
+(*               } *)
+(*               { solve_rule_conds_ex. } *)
+(*               { solve_rule_conds_ex. } *)
+(*               { solve_rule_conds_ex. } *)
+(*             } *)
+(*             { solve_rule_conds_ex. } *)
+(*           * solve_rule_conds_ex. *)
 
-      - (** [parentSetDownRsM] *)
-        disc_rule_conds_ex.
+(*       - (** [parentSetDownRsM] *) *)
+(*         disc_rule_conds_ex. *)
 
-        (* discharge the lock invariant *)
-        destruct H6.
-        red in H8; simpl in H8.
-        disc_rule_conds_const.
-        red in H8.
-        disc_rule_conds_const.
-        destruct H8; dest; [|discriminate].
-        rewrite H10 in *.
+(*         (* discharge the lock invariant *) *)
+(*         destruct H6. *)
+(*         red in H8; simpl in H8. *)
+(*         disc_rule_conds_const. *)
+(*         red in H8. *)
+(*         disc_rule_conds_const. *)
+(*         destruct H8; dest; [|discriminate]. *)
+(*         rewrite H10 in *. *)
 
-        (* discharge message predicates *)
-        disc_msg_preds H4.
-        disc_rule_conds_ex.
+(*         (* discharge message predicates *) *)
+(*         disc_msg_preds H4. *)
+(*         disc_rule_conds_ex. *)
         
-        split.
-        + apply Forall_app.
-          * apply forall_removeOnce.
-            eapply atomic_rsUps_preserves_msg_out_preds
-              with (rsUps:= [(c2pRs, rmsg)]); eauto.
-            { exact msiSv_impl_ORqsInit. }
-            { exact msiSv_impl_RqRsSys. }
-            { repeat constructor; intro; dest_in. }
-            { apply SubList_cons; [|apply SubList_nil].
-              assumption.
-            }
-            { instantiate (1:= fun _ => True).
-              instantiate (1:= [pc2]).
-              repeat split.
-              { discriminate. }
-              { repeat constructor.
-                simpl; exists child2Idx.
-                repeat split.
-              }
-            }
-            { exact msiSvMsgOutPred_good. }
-          * repeat (constructor; simpl).
-            red; simpl.
-            solve_rule_conds_ex.
-        + split.
-          * red in H6; red; simpl in *; mred; simpl.
-            destruct (oss@[child1Idx]) as [cost1|] eqn:Hcost1; simpl in *; [|auto].
-            destruct (orqs@[child1Idx]) as [corq1|] eqn:Hcorq1; simpl in *; [|auto].
-            destruct (orqs@[child2Idx]) as [corq2|] eqn:Hcorq2; simpl in *; [|auto].
-            destruct H6 as [[cv ?] ?].
-            red in H6; dest.
+(*         split. *)
+(*         + apply Forall_app. *)
+(*           * apply forall_removeOnce. *)
+(*             eapply atomic_rsUps_preserves_msg_out_preds *)
+(*               with (rsUps:= [(c2pRs, rmsg)]); eauto. *)
+(*             { exact msiSv_impl_ORqsInit. } *)
+(*             { exact msiSv_impl_RqRsSys. } *)
+(*             { repeat constructor; intro; dest_in. } *)
+(*             { apply SubList_cons; [|apply SubList_nil]. *)
+(*               assumption. *)
+(*             } *)
+(*             { instantiate (1:= fun _ => True). *)
+(*               instantiate (1:= [pc2]). *)
+(*               repeat split. *)
+(*               { discriminate. } *)
+(*               { repeat constructor. *)
+(*                 simpl; exists child2Idx. *)
+(*                 repeat split. *)
+(*               } *)
+(*             } *)
+(*             { exact msiSvMsgOutPred_good. } *)
+(*           * repeat (constructor; simpl). *)
+(*             red; simpl. *)
+(*             solve_rule_conds_ex. *)
+(*         + split. *)
+(*           * red in H6; red; simpl in *; mred; simpl. *)
+(*             destruct (oss@[child1Idx]) as [cost1|] eqn:Hcost1; simpl in *; [|auto]. *)
+(*             destruct (orqs@[child1Idx]) as [corq1|] eqn:Hcorq1; simpl in *; [|auto]. *)
+(*             destruct (orqs@[child2Idx]) as [corq2|] eqn:Hcorq2; simpl in *; [|auto]. *)
+(*             destruct H6 as [[cv ?] ?]. *)
+(*             red in H6; dest. *)
 
-            assert (In (child child1Idx ec1 ce1 c1pRq c1pRs pc1) (sys_objs impl))
-              by (simpl; tauto).
-            good_locking_get (child child1Idx ec1 ce1 c1pRq c1pRs pc1).
-            clear H21.
-            eapply upLockInvORq_parent_locked_locked in H22; try reflexivity;
-              [|red; repeat (simpl; mred); eauto]; dest.
+(*             assert (In (child child1Idx ec1 ce1 c1pRq c1pRs pc1) (sys_objs impl)) *)
+(*               by (simpl; tauto). *)
+(*             good_locking_get (child child1Idx ec1 ce1 c1pRq c1pRs pc1). *)
+(*             clear H21. *)
+(*             eapply upLockInvORq_parent_locked_locked in H22; try reflexivity; *)
+(*               [|red; repeat (simpl; mred); eauto]; dest. *)
 
-            split.
-            { exists val0.
-              red; repeat ssplit.
-              { solve_rule_conds_ex.
-                right; right; auto.
-              }
-              { solve_rule_conds_ex. }
-              { solve_rule_conds_ex. }
-              { solve_rule_conds_ex. }
-            }
-            { solve_rule_conds_ex. }
-          * solve_rule_conds_ex.
+(*             split. *)
+(*             { exists val0. *)
+(*               red; repeat ssplit. *)
+(*               { solve_rule_conds_ex. *)
+(*                 right; right; auto. *)
+(*               } *)
+(*               { solve_rule_conds_ex. } *)
+(*               { solve_rule_conds_ex. } *)
+(*               { solve_rule_conds_ex. } *)
+(*             } *)
+(*             { solve_rule_conds_ex. } *)
+(*           * solve_rule_conds_ex. *)
 
-      - (** [parentEvictRqImmI] *)
-        disc_rule_conds_ex.
+(*       - (** [parentEvictRqImmI] *) *)
+(*         disc_rule_conds_ex. *)
 
-        split.
-        + apply Forall_app.
-          * apply forall_removeOnce.
-            eapply atomic_rqUp_preserves_msg_out_preds with (oidx:= child1Idx);
-              [exact msiSv_impl_ORqsInit
-              |exact msiSv_impl_RqRsSys|..]; eauto.
-            { intro; dest_in; discriminate. }
-            { red; auto. }
-            { exact msiSvMsgOutPred_good. }
-          * repeat (constructor; simpl).
-            red; repeat (simpl; mred).
-        + destruct H6; split.
-          * red in H6; red; simpl in *; mred.
-          * red in H7; red; simpl in *; mred.
+(*         split. *)
+(*         + apply Forall_app. *)
+(*           * apply forall_removeOnce. *)
+(*             eapply atomic_rqUp_preserves_msg_out_preds with (oidx:= child1Idx); *)
+(*               [exact msiSv_impl_ORqsInit *)
+(*               |exact msiSv_impl_RqRsSys|..]; eauto. *)
+(*             { intro; dest_in; discriminate. } *)
+(*             { red; auto. } *)
+(*             { exact msiSvMsgOutPred_good. } *)
+(*           * repeat (constructor; simpl). *)
+(*             red; repeat (simpl; mred). *)
+(*         + destruct H6; split. *)
+(*           * red in H6; red; simpl in *; mred. *)
+(*           * red in H7; red; simpl in *; mred. *)
         
-      - (** [parentEvictRqImmS] *)
-        disc_rule_conds_ex.
+(*       - (** [parentEvictRqImmS] *) *)
+(*         disc_rule_conds_ex. *)
 
-        split.
-        + apply Forall_app.
-          * apply forall_removeOnce.
-            eapply atomic_rqUp_preserves_msg_out_preds with (oidx:= child1Idx);
-              [exact msiSv_impl_ORqsInit
-              |exact msiSv_impl_RqRsSys|..]; eauto.
-            { intro; dest_in; discriminate. }
-            { red; auto. }
-            { exact msiSvMsgOutPred_good. }
-          * repeat (constructor; simpl).
-            red; repeat (simpl; mred).
-        + destruct H6; split.
-          * red in H6; red; simpl in *; mred; simpl.
-            destruct (oss@[child1Idx]) as [cost1|] eqn:Hcost1; simpl in *; [|auto].
-            destruct (oss@[child2Idx]) as [cost2|] eqn:Hcost2; simpl in *; [|auto].
-            destruct (orqs@[child1Idx]) as [corq1|] eqn:Hcorq1; simpl in *; [|auto].
-            destruct (orqs@[child2Idx]) as [corq2|] eqn:Hcorq2; simpl in *; [|auto].
-            destruct H6 as [[cv ?] ?].
-            red in H6; dest.
-            unfold getDir in *; simpl in *.
-            disc_rule_conds_ex.
-            destruct H6 as [|[|]];
-              [exfalso; solve_rule_conds_ex
-              | |exfalso; destruct H6 as [? [|]]; solve_rule_conds_ex].
-            split.
-            { exists cv.
-              repeat ssplit.
-              { solve_rule_conds_ex.
-                right; left; solve_msi.
-              }
-              { solve_rule_conds_ex. }
-              { solve_rule_conds_ex. }
-              { solve_rule_conds_ex. }
-            }
-            { disc_rule_conds_ex.
-              assert (In (child child1Idx ec1 ce1 c1pRq c1pRs pc1) (sys_objs impl))
-                by (simpl; tauto).
-              good_locking_get (child child1Idx ec1 ce1 c1pRq c1pRs pc1).
-              clear H6.
-              eapply upLockInvORq_rqUp_length_one_locked in H28; try reflexivity;
-                [|eapply findQ_length_ge_one; apply FirstMP_InMP; eassumption].
-              solve_rule_conds_ex.
-            }
-          * red in H7; red; simpl in *; mred.
+(*         split. *)
+(*         + apply Forall_app. *)
+(*           * apply forall_removeOnce. *)
+(*             eapply atomic_rqUp_preserves_msg_out_preds with (oidx:= child1Idx); *)
+(*               [exact msiSv_impl_ORqsInit *)
+(*               |exact msiSv_impl_RqRsSys|..]; eauto. *)
+(*             { intro; dest_in; discriminate. } *)
+(*             { red; auto. } *)
+(*             { exact msiSvMsgOutPred_good. } *)
+(*           * repeat (constructor; simpl). *)
+(*             red; repeat (simpl; mred). *)
+(*         + destruct H6; split. *)
+(*           * red in H6; red; simpl in *; mred; simpl. *)
+(*             destruct (oss@[child1Idx]) as [cost1|] eqn:Hcost1; simpl in *; [|auto]. *)
+(*             destruct (oss@[child2Idx]) as [cost2|] eqn:Hcost2; simpl in *; [|auto]. *)
+(*             destruct (orqs@[child1Idx]) as [corq1|] eqn:Hcorq1; simpl in *; [|auto]. *)
+(*             destruct (orqs@[child2Idx]) as [corq2|] eqn:Hcorq2; simpl in *; [|auto]. *)
+(*             destruct H6 as [[cv ?] ?]. *)
+(*             red in H6; dest. *)
+(*             unfold getDir in *; simpl in *. *)
+(*             disc_rule_conds_ex. *)
+(*             destruct H6 as [|[|]]; *)
+(*               [exfalso; solve_rule_conds_ex *)
+(*               | |exfalso; destruct H6 as [? [|]]; solve_rule_conds_ex]. *)
+(*             split. *)
+(*             { exists cv. *)
+(*               repeat ssplit. *)
+(*               { solve_rule_conds_ex. *)
+(*                 right; left; solve_msi. *)
+(*               } *)
+(*               { solve_rule_conds_ex. } *)
+(*               { solve_rule_conds_ex. } *)
+(*               { solve_rule_conds_ex. } *)
+(*             } *)
+(*             { disc_rule_conds_ex. *)
+(*               assert (In (child child1Idx ec1 ce1 c1pRq c1pRs pc1) (sys_objs impl)) *)
+(*                 by (simpl; tauto). *)
+(*               good_locking_get (child child1Idx ec1 ce1 c1pRq c1pRs pc1). *)
+(*               clear H6. *)
+(*               eapply upLockInvORq_rqUp_length_one_locked in H28; try reflexivity; *)
+(*                 [|eapply findQ_length_ge_one; apply FirstMP_InMP; eassumption]. *)
+(*               solve_rule_conds_ex. *)
+(*             } *)
+(*           * red in H7; red; simpl in *; mred. *)
 
-      - (** [parentEvictRqImmLastS] *)
-        disc_rule_conds_ex.
+(*       - (** [parentEvictRqImmLastS] *) *)
+(*         disc_rule_conds_ex. *)
 
-        split.
-        + apply Forall_app.
-          * apply forall_removeOnce.
-            eapply atomic_rqUp_preserves_msg_out_preds with (oidx:= child1Idx);
-              [exact msiSv_impl_ORqsInit
-              |exact msiSv_impl_RqRsSys|..]; eauto.
-            { intro; dest_in; discriminate. }
-            { red; auto. }
-            { exact msiSvMsgOutPred_good. }
-          * repeat (constructor; simpl).
-            red; repeat (simpl; mred).
-        + destruct H6; split.
-          * red in H6; red; simpl in *; mred; simpl.
-            destruct (oss@[child1Idx]) as [cost1|] eqn:Hcost1; simpl in *; [|auto].
-            destruct (oss@[child2Idx]) as [cost2|] eqn:Hcost2; simpl in *; [|auto].
-            destruct (orqs@[child1Idx]) as [corq1|] eqn:Hcorq1; simpl in *; [|auto].
-            destruct (orqs@[child2Idx]) as [corq2|] eqn:Hcorq2; simpl in *; [|auto].
-            destruct H6 as [[cv ?] ?].
-            red in H6; dest.
-            unfold getDir in *; simpl in *.
-            disc_rule_conds_ex.
-            destruct H6 as [|[|]];
-              [exfalso; solve_rule_conds_ex
-              | |exfalso; destruct H6 as [? [|]]; solve_rule_conds_ex].
-            split.
-            { exists cv.
-              repeat ssplit.
-              { solve_rule_conds_ex.
-                left; auto.
-              }
-              { solve_rule_conds_ex. }
-              { solve_rule_conds_ex. }
-              { solve_rule_conds_ex. }
-            }
-            { disc_rule_conds_ex.
-              assert (In (child child1Idx ec1 ce1 c1pRq c1pRs pc1) (sys_objs impl))
-                by (simpl; tauto).
-              good_locking_get (child child1Idx ec1 ce1 c1pRq c1pRs pc1).
-              clear H6.
-              eapply upLockInvORq_rqUp_length_one_locked in H28; try reflexivity;
-                [|eapply findQ_length_ge_one; apply FirstMP_InMP; eassumption].
-              solve_rule_conds_ex.
-            }
-          * red in H7; red; simpl in *; mred.
+(*         split. *)
+(*         + apply Forall_app. *)
+(*           * apply forall_removeOnce. *)
+(*             eapply atomic_rqUp_preserves_msg_out_preds with (oidx:= child1Idx); *)
+(*               [exact msiSv_impl_ORqsInit *)
+(*               |exact msiSv_impl_RqRsSys|..]; eauto. *)
+(*             { intro; dest_in; discriminate. } *)
+(*             { red; auto. } *)
+(*             { exact msiSvMsgOutPred_good. } *)
+(*           * repeat (constructor; simpl). *)
+(*             red; repeat (simpl; mred). *)
+(*         + destruct H6; split. *)
+(*           * red in H6; red; simpl in *; mred; simpl. *)
+(*             destruct (oss@[child1Idx]) as [cost1|] eqn:Hcost1; simpl in *; [|auto]. *)
+(*             destruct (oss@[child2Idx]) as [cost2|] eqn:Hcost2; simpl in *; [|auto]. *)
+(*             destruct (orqs@[child1Idx]) as [corq1|] eqn:Hcorq1; simpl in *; [|auto]. *)
+(*             destruct (orqs@[child2Idx]) as [corq2|] eqn:Hcorq2; simpl in *; [|auto]. *)
+(*             destruct H6 as [[cv ?] ?]. *)
+(*             red in H6; dest. *)
+(*             unfold getDir in *; simpl in *. *)
+(*             disc_rule_conds_ex. *)
+(*             destruct H6 as [|[|]]; *)
+(*               [exfalso; solve_rule_conds_ex *)
+(*               | |exfalso; destruct H6 as [? [|]]; solve_rule_conds_ex]. *)
+(*             split. *)
+(*             { exists cv. *)
+(*               repeat ssplit. *)
+(*               { solve_rule_conds_ex. *)
+(*                 left; auto. *)
+(*               } *)
+(*               { solve_rule_conds_ex. } *)
+(*               { solve_rule_conds_ex. } *)
+(*               { solve_rule_conds_ex. } *)
+(*             } *)
+(*             { disc_rule_conds_ex. *)
+(*               assert (In (child child1Idx ec1 ce1 c1pRq c1pRs pc1) (sys_objs impl)) *)
+(*                 by (simpl; tauto). *)
+(*               good_locking_get (child child1Idx ec1 ce1 c1pRq c1pRs pc1). *)
+(*               clear H6. *)
+(*               eapply upLockInvORq_rqUp_length_one_locked in H28; try reflexivity; *)
+(*                 [|eapply findQ_length_ge_one; apply FirstMP_InMP; eassumption]. *)
+(*               solve_rule_conds_ex. *)
+(*             } *)
+(*           * red in H7; red; simpl in *; mred. *)
 
-      - (** [parentEvictRqImmM] *)
-        disc_rule_conds_ex.
+(*       - (** [parentEvictRqImmM] *) *)
+(*         disc_rule_conds_ex. *)
 
-        split.
-        + apply Forall_app.
-          * apply forall_removeOnce.
-            eapply atomic_rqUp_preserves_msg_out_preds with (oidx:= child1Idx);
-              [exact msiSv_impl_ORqsInit
-              |exact msiSv_impl_RqRsSys|..]; eauto.
-            { intro; dest_in; discriminate. }
-            { red; auto. }
-            { exact msiSvMsgOutPred_good. }
-          * repeat (constructor; simpl).
-            red; repeat (simpl; mred).
-        + destruct H6; split.
-          * red in H6; red; simpl in *; mred; simpl.
-            destruct (oss@[child1Idx]) as [cost1|] eqn:Hcost1; simpl in *; [|auto].
-            destruct (oss@[child2Idx]) as [cost2|] eqn:Hcost2; simpl in *; [|auto].
-            destruct (orqs@[child1Idx]) as [corq1|] eqn:Hcorq1; simpl in *; [|auto].
-            destruct (orqs@[child2Idx]) as [corq2|] eqn:Hcorq2; simpl in *; [|auto].
-            destruct H6 as [[cv ?] ?].
-            red in H6; dest.
-            unfold getDir in *; simpl in *.
-            disc_rule_conds_ex.
-            destruct H6 as [|[|]]; try (exfalso; solve_rule_conds_ex; fail).
+(*         split. *)
+(*         + apply Forall_app. *)
+(*           * apply forall_removeOnce. *)
+(*             eapply atomic_rqUp_preserves_msg_out_preds with (oidx:= child1Idx); *)
+(*               [exact msiSv_impl_ORqsInit *)
+(*               |exact msiSv_impl_RqRsSys|..]; eauto. *)
+(*             { intro; dest_in; discriminate. } *)
+(*             { red; auto. } *)
+(*             { exact msiSvMsgOutPred_good. } *)
+(*           * repeat (constructor; simpl). *)
+(*             red; repeat (simpl; mred). *)
+(*         + destruct H6; split. *)
+(*           * red in H6; red; simpl in *; mred; simpl. *)
+(*             destruct (oss@[child1Idx]) as [cost1|] eqn:Hcost1; simpl in *; [|auto]. *)
+(*             destruct (oss@[child2Idx]) as [cost2|] eqn:Hcost2; simpl in *; [|auto]. *)
+(*             destruct (orqs@[child1Idx]) as [corq1|] eqn:Hcorq1; simpl in *; [|auto]. *)
+(*             destruct (orqs@[child2Idx]) as [corq2|] eqn:Hcorq2; simpl in *; [|auto]. *)
+(*             destruct H6 as [[cv ?] ?]. *)
+(*             red in H6; dest. *)
+(*             unfold getDir in *; simpl in *. *)
+(*             disc_rule_conds_ex. *)
+(*             destruct H6 as [|[|]]; try (exfalso; solve_rule_conds_ex; fail). *)
 
-            assert (In (child child1Idx ec1 ce1 c1pRq c1pRs pc1) (sys_objs impl))
-              by (simpl; tauto).
-            good_locking_get (child child1Idx ec1 ce1 c1pRq c1pRs pc1).
-            clear H26.
-            eapply upLockInvORq_rqUp_length_one_locked in H27; try reflexivity;
-              [|eapply findQ_length_ge_one; apply FirstMP_InMP; eassumption].
-            disc_rule_conds_ex.
+(*             assert (In (child child1Idx ec1 ce1 c1pRq c1pRs pc1) (sys_objs impl)) *)
+(*               by (simpl; tauto). *)
+(*             good_locking_get (child child1Idx ec1 ce1 c1pRq c1pRs pc1). *)
+(*             clear H26. *)
+(*             eapply upLockInvORq_rqUp_length_one_locked in H27; try reflexivity; *)
+(*               [|eapply findQ_length_ge_one; apply FirstMP_InMP; eassumption]. *)
+(*             disc_rule_conds_ex. *)
           
-            split.
-            { exists n.
-              repeat ssplit.
-              { solve_rule_conds_ex.
-                left; solve_msi.
-              }
-              { solve_rule_conds_ex. }
-              { solve_rule_conds_ex; solve_msi. }
-              { solve_rule_conds_ex. }
-            }
-            { solve_rule_conds_ex. }
-          * red in H7; red; simpl in *; mred.
+(*             split. *)
+(*             { exists n. *)
+(*               repeat ssplit. *)
+(*               { solve_rule_conds_ex. *)
+(*                 left; solve_msi. *)
+(*               } *)
+(*               { solve_rule_conds_ex. } *)
+(*               { solve_rule_conds_ex; solve_msi. } *)
+(*               { solve_rule_conds_ex. } *)
+(*             } *)
+(*             { solve_rule_conds_ex. } *)
+(*           * red in H7; red; simpl in *; mred. *)
 
-      (** parent(child2) *)
+(*       (** parent(child2) *) *)
 
-      - (** [parentGetRqImm] *)
-        disc_rule_conds_ex.
+(*       - (** [parentGetRqImm] *) *)
+(*         disc_rule_conds_ex. *)
 
-        split.
-        + apply Forall_app.
-          * apply forall_removeOnce.
-            eapply atomic_rqUp_preserves_msg_out_preds with (oidx:= child2Idx);
-              [exact msiSv_impl_ORqsInit
-              |exact msiSv_impl_RqRsSys|..]; eauto.
-            { intro; dest_in; discriminate. }
-            { red; auto. }
-            { exact msiSvMsgOutPred_good. }
-          * repeat (constructor; simpl).
-            red; repeat (simpl; mred).
-        + destruct H6; split.
-          * red in H6; red; simpl in *; mred; simpl.
-            destruct (oss@[child1Idx]) as [cost1|] eqn:Hcost1; simpl in *; [|auto].
-            destruct (oss@[child2Idx]) as [cost2|] eqn:Hcost2; simpl in *; [|auto].
-            destruct (orqs@[child1Idx]) as [corq1|] eqn:Hcorq1; simpl in *; [|auto].
-            destruct (orqs@[child2Idx]) as [corq2|] eqn:Hcorq2; simpl in *; [|auto].
-            destruct H6 as [[cv ?] ?].
-            red in H6; dest.
-            split.
-            { exists cv.
-              red; repeat ssplit.
-              { solve_rule_conds_ex.
-                right; left.
-                destruct H6 as [|[|]].
-                { solve_rule_conds_ex; solve_msi. }
-                { solve_rule_conds_ex. }
-                { solve_msi. }
-              }
-              { solve_rule_conds_ex. }
-              { solve_rule_conds_ex. }
-              { solve_rule_conds_ex. }
-            }
-            { disc_rule_conds_ex.
-              assert (In (child child2Idx ec2 ce2 c2pRq c2pRs pc2) (sys_objs impl))
-                by (simpl; tauto).
-              good_locking_get (child child2Idx ec2 ce2 c2pRq c2pRs pc2).
-              clear H24.
-              eapply upLockInvORq_rqUp_length_one_locked in H26; try reflexivity;
-                [|eapply findQ_length_ge_one; apply FirstMP_InMP; eassumption].
-              solve_rule_conds_ex.
-            }
-          * red in H7; red; simpl in *; mred.
+(*         split. *)
+(*         + apply Forall_app. *)
+(*           * apply forall_removeOnce. *)
+(*             eapply atomic_rqUp_preserves_msg_out_preds with (oidx:= child2Idx); *)
+(*               [exact msiSv_impl_ORqsInit *)
+(*               |exact msiSv_impl_RqRsSys|..]; eauto. *)
+(*             { intro; dest_in; discriminate. } *)
+(*             { red; auto. } *)
+(*             { exact msiSvMsgOutPred_good. } *)
+(*           * repeat (constructor; simpl). *)
+(*             red; repeat (simpl; mred). *)
+(*         + destruct H6; split. *)
+(*           * red in H6; red; simpl in *; mred; simpl. *)
+(*             destruct (oss@[child1Idx]) as [cost1|] eqn:Hcost1; simpl in *; [|auto]. *)
+(*             destruct (oss@[child2Idx]) as [cost2|] eqn:Hcost2; simpl in *; [|auto]. *)
+(*             destruct (orqs@[child1Idx]) as [corq1|] eqn:Hcorq1; simpl in *; [|auto]. *)
+(*             destruct (orqs@[child2Idx]) as [corq2|] eqn:Hcorq2; simpl in *; [|auto]. *)
+(*             destruct H6 as [[cv ?] ?]. *)
+(*             red in H6; dest. *)
+(*             split. *)
+(*             { exists cv. *)
+(*               red; repeat ssplit. *)
+(*               { solve_rule_conds_ex. *)
+(*                 right; left. *)
+(*                 destruct H6 as [|[|]]. *)
+(*                 { solve_rule_conds_ex; solve_msi. } *)
+(*                 { solve_rule_conds_ex. } *)
+(*                 { solve_msi. } *)
+(*               } *)
+(*               { solve_rule_conds_ex. } *)
+(*               { solve_rule_conds_ex. } *)
+(*               { solve_rule_conds_ex. } *)
+(*             } *)
+(*             { disc_rule_conds_ex. *)
+(*               assert (In (child child2Idx ec2 ce2 c2pRq c2pRs pc2) (sys_objs impl)) *)
+(*                 by (simpl; tauto). *)
+(*               good_locking_get (child child2Idx ec2 ce2 c2pRq c2pRs pc2). *)
+(*               clear H24. *)
+(*               eapply upLockInvORq_rqUp_length_one_locked in H26; try reflexivity; *)
+(*                 [|eapply findQ_length_ge_one; apply FirstMP_InMP; eassumption]. *)
+(*               solve_rule_conds_ex. *)
+(*             } *)
+(*           * red in H7; red; simpl in *; mred. *)
 
-      - (** [parentGetDownRqS] *)
-        disc_rule_conds_ex.
+(*       - (** [parentGetDownRqS] *) *)
+(*         disc_rule_conds_ex. *)
 
-        split.
-        + apply Forall_app.
-          * apply forall_removeOnce.
-            eapply atomic_rqUp_preserves_msg_out_preds with (oidx:= child2Idx);
-              [exact msiSv_impl_ORqsInit
-              |exact msiSv_impl_RqRsSys|..]; eauto.
-            { intro; dest_in; discriminate. }
-            { red; auto. }
-            { exact msiSvMsgOutPred_good. }
-          * repeat (constructor; simpl).
-        + destruct H6; split.
-          * red in H6; red; simpl in *; mred.
-          * solve_rule_conds_ex.
+(*         split. *)
+(*         + apply Forall_app. *)
+(*           * apply forall_removeOnce. *)
+(*             eapply atomic_rqUp_preserves_msg_out_preds with (oidx:= child2Idx); *)
+(*               [exact msiSv_impl_ORqsInit *)
+(*               |exact msiSv_impl_RqRsSys|..]; eauto. *)
+(*             { intro; dest_in; discriminate. } *)
+(*             { red; auto. } *)
+(*             { exact msiSvMsgOutPred_good. } *)
+(*           * repeat (constructor; simpl). *)
+(*         + destruct H6; split. *)
+(*           * red in H6; red; simpl in *; mred. *)
+(*           * solve_rule_conds_ex. *)
 
-      - (** [parentSetRqImm] *)
-        disc_rule_conds_ex.
+(*       - (** [parentSetRqImm] *) *)
+(*         disc_rule_conds_ex. *)
 
-        split.
-        + apply Forall_app.
-          * apply forall_removeOnce.
-            eapply atomic_rqUp_preserves_msg_out_preds with (oidx:= child2Idx);
-              [exact msiSv_impl_ORqsInit
-              |exact msiSv_impl_RqRsSys|..]; eauto.
-            { intro; dest_in; discriminate. }
-            { red; auto. }
-            { exact msiSvMsgOutPred_good. }
-          * repeat (constructor; simpl).
-            red; repeat (simpl; mred).
-        + destruct H6; split.
-          * red in H6; red; simpl in *; mred; simpl.
-            destruct (oss@[child1Idx]) as [cost1|] eqn:Hcost1; simpl in *; [|auto].
-            destruct (oss@[child2Idx]) as [cost2|] eqn:Hcost2; simpl in *; [|auto].
-            destruct (orqs@[child1Idx]) as [corq1|] eqn:Hcorq1; simpl in *; [|auto].
-            destruct (orqs@[child2Idx]) as [corq2|] eqn:Hcorq2; simpl in *; [|auto].
-            destruct H6 as [[cv ?] ?].
-            red in H6; dest.
-            unfold getDir in H14; simpl in H14.
-            split.
-            { exists cv.
-              red; repeat ssplit.
-              { solve_rule_conds_ex.
-                right; right; auto.
-              }
-              { solve_rule_conds_ex. }
-              { solve_rule_conds_ex. }
-              { solve_rule_conds_ex. }
-            }
-            { disc_rule_conds_ex.
-              assert (In (child child2Idx ec2 ce2 c2pRq c2pRs pc2) (sys_objs impl))
-                by (simpl; tauto).
-              good_locking_get (child child2Idx ec2 ce2 c2pRq c2pRs pc2).
-              clear H24.
-              eapply upLockInvORq_rqUp_length_one_locked in H26; try reflexivity;
-                [|eapply findQ_length_ge_one; apply FirstMP_InMP; eassumption].
-              solve_rule_conds_ex.
-            }
-          * red in H7; red; simpl in *; mred.
+(*         split. *)
+(*         + apply Forall_app. *)
+(*           * apply forall_removeOnce. *)
+(*             eapply atomic_rqUp_preserves_msg_out_preds with (oidx:= child2Idx); *)
+(*               [exact msiSv_impl_ORqsInit *)
+(*               |exact msiSv_impl_RqRsSys|..]; eauto. *)
+(*             { intro; dest_in; discriminate. } *)
+(*             { red; auto. } *)
+(*             { exact msiSvMsgOutPred_good. } *)
+(*           * repeat (constructor; simpl). *)
+(*             red; repeat (simpl; mred). *)
+(*         + destruct H6; split. *)
+(*           * red in H6; red; simpl in *; mred; simpl. *)
+(*             destruct (oss@[child1Idx]) as [cost1|] eqn:Hcost1; simpl in *; [|auto]. *)
+(*             destruct (oss@[child2Idx]) as [cost2|] eqn:Hcost2; simpl in *; [|auto]. *)
+(*             destruct (orqs@[child1Idx]) as [corq1|] eqn:Hcorq1; simpl in *; [|auto]. *)
+(*             destruct (orqs@[child2Idx]) as [corq2|] eqn:Hcorq2; simpl in *; [|auto]. *)
+(*             destruct H6 as [[cv ?] ?]. *)
+(*             red in H6; dest. *)
+(*             unfold getDir in H14; simpl in H14. *)
+(*             split. *)
+(*             { exists cv. *)
+(*               red; repeat ssplit. *)
+(*               { solve_rule_conds_ex. *)
+(*                 right; right; auto. *)
+(*               } *)
+(*               { solve_rule_conds_ex. } *)
+(*               { solve_rule_conds_ex. } *)
+(*               { solve_rule_conds_ex. } *)
+(*             } *)
+(*             { disc_rule_conds_ex. *)
+(*               assert (In (child child2Idx ec2 ce2 c2pRq c2pRs pc2) (sys_objs impl)) *)
+(*                 by (simpl; tauto). *)
+(*               good_locking_get (child child2Idx ec2 ce2 c2pRq c2pRs pc2). *)
+(*               clear H24. *)
+(*               eapply upLockInvORq_rqUp_length_one_locked in H26; try reflexivity; *)
+(*                 [|eapply findQ_length_ge_one; apply FirstMP_InMP; eassumption]. *)
+(*               solve_rule_conds_ex. *)
+(*             } *)
+(*           * red in H7; red; simpl in *; mred. *)
 
-      - (** [parentSetDownRqM] *)
-        disc_rule_conds_ex.
+(*       - (** [parentSetDownRqM] *) *)
+(*         disc_rule_conds_ex. *)
 
-        split.
-        + apply Forall_app.
-          * apply forall_removeOnce.
-            eapply atomic_rqUp_preserves_msg_out_preds with (oidx:= child2Idx);
-              [exact msiSv_impl_ORqsInit
-              |exact msiSv_impl_RqRsSys|..]; eauto.
-            { intro; dest_in; discriminate. }
-            { red; auto. }
-            { exact msiSvMsgOutPred_good. }
-          * repeat (constructor; simpl).
-        + destruct H6; split.
-          * red in H6; red; simpl in *; mred.
-          * solve_rule_conds_ex.
+(*         split. *)
+(*         + apply Forall_app. *)
+(*           * apply forall_removeOnce. *)
+(*             eapply atomic_rqUp_preserves_msg_out_preds with (oidx:= child2Idx); *)
+(*               [exact msiSv_impl_ORqsInit *)
+(*               |exact msiSv_impl_RqRsSys|..]; eauto. *)
+(*             { intro; dest_in; discriminate. } *)
+(*             { red; auto. } *)
+(*             { exact msiSvMsgOutPred_good. } *)
+(*           * repeat (constructor; simpl). *)
+(*         + destruct H6; split. *)
+(*           * red in H6; red; simpl in *; mred. *)
+(*           * solve_rule_conds_ex. *)
 
-      - (** [parentGetDownRsS] *)
-        disc_rule_conds_ex.
+(*       - (** [parentGetDownRsS] *) *)
+(*         disc_rule_conds_ex. *)
 
-        (* discharge the lock invariant *)
-        destruct H6.
-        red in H8; simpl in H8.
-        disc_rule_conds_const.
-        red in H8.
-        disc_rule_conds_const.
-        destruct H8; dest; [discriminate|].
-        rewrite H10 in *.
+(*         (* discharge the lock invariant *) *)
+(*         destruct H6. *)
+(*         red in H8; simpl in H8. *)
+(*         disc_rule_conds_const. *)
+(*         red in H8. *)
+(*         disc_rule_conds_const. *)
+(*         destruct H8; dest; [discriminate|]. *)
+(*         rewrite H10 in *. *)
 
-        (* discharge message predicates *)
-        disc_msg_preds H4.
-        disc_rule_conds_ex.
+(*         (* discharge message predicates *) *)
+(*         disc_msg_preds H4. *)
+(*         disc_rule_conds_ex. *)
         
-        split.
-        + apply Forall_app.
-          * apply forall_removeOnce.
-            eapply atomic_rsUps_preserves_msg_out_preds
-              with (rsUps:= [(c1pRs, rmsg)]); eauto.
-            { exact msiSv_impl_ORqsInit. }
-            { exact msiSv_impl_RqRsSys. }
-            { repeat constructor; intro; dest_in. }
-            { apply SubList_cons; [|apply SubList_nil].
-              assumption.
-            }
-            { instantiate (1:= fun _ => True).
-              instantiate (1:= [pc1]).
-              repeat split.
-              { discriminate. }
-              { repeat constructor.
-                simpl; exists child1Idx.
-                repeat split.
-              }
-            }
-            { exact msiSvMsgOutPred_good. }
-          * repeat (constructor; simpl).
-            red; simpl.
-            solve_rule_conds_ex.
-        + split.
-          * red in H6; red; simpl in *; mred; simpl.
-            destruct (oss@[child2Idx]) as [cost2|] eqn:Hcost2; simpl in *; [|auto].
-            destruct (orqs@[child1Idx]) as [corq1|] eqn:Hcorq1; simpl in *; [|auto].
-            destruct (orqs@[child2Idx]) as [corq2|] eqn:Hcorq2; simpl in *; [|auto].
-            destruct H6 as [[cv ?] ?].
-            red in H6; dest.
+(*         split. *)
+(*         + apply Forall_app. *)
+(*           * apply forall_removeOnce. *)
+(*             eapply atomic_rsUps_preserves_msg_out_preds *)
+(*               with (rsUps:= [(c1pRs, rmsg)]); eauto. *)
+(*             { exact msiSv_impl_ORqsInit. } *)
+(*             { exact msiSv_impl_RqRsSys. } *)
+(*             { repeat constructor; intro; dest_in. } *)
+(*             { apply SubList_cons; [|apply SubList_nil]. *)
+(*               assumption. *)
+(*             } *)
+(*             { instantiate (1:= fun _ => True). *)
+(*               instantiate (1:= [pc1]). *)
+(*               repeat split. *)
+(*               { discriminate. } *)
+(*               { repeat constructor. *)
+(*                 simpl; exists child1Idx. *)
+(*                 repeat split. *)
+(*               } *)
+(*             } *)
+(*             { exact msiSvMsgOutPred_good. } *)
+(*           * repeat (constructor; simpl). *)
+(*             red; simpl. *)
+(*             solve_rule_conds_ex. *)
+(*         + split. *)
+(*           * red in H6; red; simpl in *; mred; simpl. *)
+(*             destruct (oss@[child2Idx]) as [cost2|] eqn:Hcost2; simpl in *; [|auto]. *)
+(*             destruct (orqs@[child1Idx]) as [corq1|] eqn:Hcorq1; simpl in *; [|auto]. *)
+(*             destruct (orqs@[child2Idx]) as [corq2|] eqn:Hcorq2; simpl in *; [|auto]. *)
+(*             destruct H6 as [[cv ?] ?]. *)
+(*             red in H6; dest. *)
 
-            assert (In (child child2Idx ec2 ce2 c2pRq c2pRs pc2) (sys_objs impl))
-              by (simpl; tauto).
-            good_locking_get (child child2Idx ec2 ce2 c2pRq c2pRs pc2).
-            clear H21.
-            eapply upLockInvORq_parent_locked_locked in H22; try reflexivity;
-              [|red; repeat (simpl; mred); eauto]; dest.
+(*             assert (In (child child2Idx ec2 ce2 c2pRq c2pRs pc2) (sys_objs impl)) *)
+(*               by (simpl; tauto). *)
+(*             good_locking_get (child child2Idx ec2 ce2 c2pRq c2pRs pc2). *)
+(*             clear H21. *)
+(*             eapply upLockInvORq_parent_locked_locked in H22; try reflexivity; *)
+(*               [|red; repeat (simpl; mred); eauto]; dest. *)
           
-            split.
-            { exists val0.
-              red; repeat ssplit.
-              { solve_rule_conds_ex.
-                right; left; auto.
-              }
-              { solve_rule_conds_ex. }
-              { solve_rule_conds_ex. }
-              { solve_rule_conds_ex. }
-            }
-            { solve_rule_conds_ex. }
-          * solve_rule_conds_ex.
+(*             split. *)
+(*             { exists val0. *)
+(*               red; repeat ssplit. *)
+(*               { solve_rule_conds_ex. *)
+(*                 right; left; auto. *)
+(*               } *)
+(*               { solve_rule_conds_ex. } *)
+(*               { solve_rule_conds_ex. } *)
+(*               { solve_rule_conds_ex. } *)
+(*             } *)
+(*             { solve_rule_conds_ex. } *)
+(*           * solve_rule_conds_ex. *)
 
-      - (** [parentSetDownRsM] *)
-        disc_rule_conds_ex.
+(*       - (** [parentSetDownRsM] *) *)
+(*         disc_rule_conds_ex. *)
 
-        (* discharge the lock invariant *)
-        destruct H6.
-        red in H8; simpl in H8.
-        disc_rule_conds_const.
-        red in H8.
-        disc_rule_conds_const.
-        destruct H8; dest; [discriminate|].
-        rewrite H10 in *.
+(*         (* discharge the lock invariant *) *)
+(*         destruct H6. *)
+(*         red in H8; simpl in H8. *)
+(*         disc_rule_conds_const. *)
+(*         red in H8. *)
+(*         disc_rule_conds_const. *)
+(*         destruct H8; dest; [discriminate|]. *)
+(*         rewrite H10 in *. *)
 
-        (* discharge message predicates *)
-        disc_msg_preds H4.
-        disc_rule_conds_ex.
+(*         (* discharge message predicates *) *)
+(*         disc_msg_preds H4. *)
+(*         disc_rule_conds_ex. *)
         
-        split.
-        + apply Forall_app.
-          * apply forall_removeOnce.
-            eapply atomic_rsUps_preserves_msg_out_preds
-              with (rsUps:= [(c1pRs, rmsg)]); eauto.
-            { exact msiSv_impl_ORqsInit. }
-            { exact msiSv_impl_RqRsSys. }
-            { repeat constructor; intro; dest_in. }
-            { apply SubList_cons; [|apply SubList_nil].
-              assumption.
-            }
-            { instantiate (1:= fun _ => True).
-              instantiate (1:= [pc1]).
-              repeat split.
-              { discriminate. }
-              { repeat constructor.
-                simpl; exists child1Idx.
-                repeat split.
-              }
-            }
-            { exact msiSvMsgOutPred_good. }
-          * repeat (constructor; simpl).
-            red; simpl.
-            solve_rule_conds_ex.
-        + split.
-          * red in H6; red; simpl in *; mred; simpl.
-            destruct (oss@[child2Idx]) as [cost2|] eqn:Hcost2; simpl in *; [|auto].
-            destruct (orqs@[child1Idx]) as [corq1|] eqn:Hcorq1; simpl in *; [|auto].
-            destruct (orqs@[child2Idx]) as [corq2|] eqn:Hcorq2; simpl in *; [|auto].
-            destruct H6 as [[cv ?] ?].
-            red in H6; dest.
+(*         split. *)
+(*         + apply Forall_app. *)
+(*           * apply forall_removeOnce. *)
+(*             eapply atomic_rsUps_preserves_msg_out_preds *)
+(*               with (rsUps:= [(c1pRs, rmsg)]); eauto. *)
+(*             { exact msiSv_impl_ORqsInit. } *)
+(*             { exact msiSv_impl_RqRsSys. } *)
+(*             { repeat constructor; intro; dest_in. } *)
+(*             { apply SubList_cons; [|apply SubList_nil]. *)
+(*               assumption. *)
+(*             } *)
+(*             { instantiate (1:= fun _ => True). *)
+(*               instantiate (1:= [pc1]). *)
+(*               repeat split. *)
+(*               { discriminate. } *)
+(*               { repeat constructor. *)
+(*                 simpl; exists child1Idx. *)
+(*                 repeat split. *)
+(*               } *)
+(*             } *)
+(*             { exact msiSvMsgOutPred_good. } *)
+(*           * repeat (constructor; simpl). *)
+(*             red; simpl. *)
+(*             solve_rule_conds_ex. *)
+(*         + split. *)
+(*           * red in H6; red; simpl in *; mred; simpl. *)
+(*             destruct (oss@[child2Idx]) as [cost2|] eqn:Hcost2; simpl in *; [|auto]. *)
+(*             destruct (orqs@[child1Idx]) as [corq1|] eqn:Hcorq1; simpl in *; [|auto]. *)
+(*             destruct (orqs@[child2Idx]) as [corq2|] eqn:Hcorq2; simpl in *; [|auto]. *)
+(*             destruct H6 as [[cv ?] ?]. *)
+(*             red in H6; dest. *)
 
-            assert (In (child child2Idx ec2 ce2 c2pRq c2pRs pc2) (sys_objs impl))
-              by (simpl; tauto).
-            good_locking_get (child child2Idx ec2 ce2 c2pRq c2pRs pc2).
-            clear H21.
-            eapply upLockInvORq_parent_locked_locked in H22; try reflexivity;
-              [|red; repeat (simpl; mred); eauto]; dest.
+(*             assert (In (child child2Idx ec2 ce2 c2pRq c2pRs pc2) (sys_objs impl)) *)
+(*               by (simpl; tauto). *)
+(*             good_locking_get (child child2Idx ec2 ce2 c2pRq c2pRs pc2). *)
+(*             clear H21. *)
+(*             eapply upLockInvORq_parent_locked_locked in H22; try reflexivity; *)
+(*               [|red; repeat (simpl; mred); eauto]; dest. *)
 
-            split.
-            { exists val0.
-              red; repeat ssplit.
-              { solve_rule_conds_ex.
-                right; right; auto.
-              }
-              { solve_rule_conds_ex. }
-              { solve_rule_conds_ex. }
-              { solve_rule_conds_ex. }
-            }
-            { solve_rule_conds_ex. }
-          * solve_rule_conds_ex.
+(*             split. *)
+(*             { exists val0. *)
+(*               red; repeat ssplit. *)
+(*               { solve_rule_conds_ex. *)
+(*                 right; right; auto. *)
+(*               } *)
+(*               { solve_rule_conds_ex. } *)
+(*               { solve_rule_conds_ex. } *)
+(*               { solve_rule_conds_ex. } *)
+(*             } *)
+(*             { solve_rule_conds_ex. } *)
+(*           * solve_rule_conds_ex. *)
 
-      - (** [parentEvictRqImmI] *)
-        disc_rule_conds_ex.
+(*       - (** [parentEvictRqImmI] *) *)
+(*         disc_rule_conds_ex. *)
 
-        split.
-        + apply Forall_app.
-          * apply forall_removeOnce.
-            eapply atomic_rqUp_preserves_msg_out_preds with (oidx:= child2Idx);
-              [exact msiSv_impl_ORqsInit
-              |exact msiSv_impl_RqRsSys|..]; eauto.
-            { intro; dest_in; discriminate. }
-            { red; auto. }
-            { exact msiSvMsgOutPred_good. }
-          * repeat (constructor; simpl).
-            red; repeat (simpl; mred).
-        + destruct H6; split.
-          * red in H6; red; simpl in *; mred.
-          * red in H7; red; simpl in *; mred.
+(*         split. *)
+(*         + apply Forall_app. *)
+(*           * apply forall_removeOnce. *)
+(*             eapply atomic_rqUp_preserves_msg_out_preds with (oidx:= child2Idx); *)
+(*               [exact msiSv_impl_ORqsInit *)
+(*               |exact msiSv_impl_RqRsSys|..]; eauto. *)
+(*             { intro; dest_in; discriminate. } *)
+(*             { red; auto. } *)
+(*             { exact msiSvMsgOutPred_good. } *)
+(*           * repeat (constructor; simpl). *)
+(*             red; repeat (simpl; mred). *)
+(*         + destruct H6; split. *)
+(*           * red in H6; red; simpl in *; mred. *)
+(*           * red in H7; red; simpl in *; mred. *)
         
-      - (** [parentEvictRqImmS] *)
-        disc_rule_conds_ex.
+(*       - (** [parentEvictRqImmS] *) *)
+(*         disc_rule_conds_ex. *)
 
-        split.
-        + apply Forall_app.
-          * apply forall_removeOnce.
-            eapply atomic_rqUp_preserves_msg_out_preds with (oidx:= child2Idx);
-              [exact msiSv_impl_ORqsInit
-              |exact msiSv_impl_RqRsSys|..]; eauto.
-            { intro; dest_in; discriminate. }
-            { red; auto. }
-            { exact msiSvMsgOutPred_good. }
-          * repeat (constructor; simpl).
-            red; repeat (simpl; mred).
-        + destruct H6; split.
-          * red in H6; red; simpl in *; mred; simpl.
-            destruct (oss@[child1Idx]) as [cost1|] eqn:Hcost1; simpl in *; [|auto].
-            destruct (oss@[child2Idx]) as [cost2|] eqn:Hcost2; simpl in *; [|auto].
-            destruct (orqs@[child1Idx]) as [corq1|] eqn:Hcorq1; simpl in *; [|auto].
-            destruct (orqs@[child2Idx]) as [corq2|] eqn:Hcorq2; simpl in *; [|auto].
-            destruct H6 as [[cv ?] ?].
-            red in H6; dest.
-            unfold getDir in *; simpl in *.
-            disc_rule_conds_ex.
-            destruct H6 as [|[|]];
-              [exfalso; solve_rule_conds_ex
-              | |exfalso; destruct H6 as [? [|]]; solve_rule_conds_ex].
-            split.
-            { exists cv.
-              repeat ssplit.
-              { solve_rule_conds_ex.
-                right; left; solve_msi.
-              }
-              { solve_rule_conds_ex. }
-              { solve_rule_conds_ex. }
-              { solve_rule_conds_ex. }
-            }
-            { disc_rule_conds_ex.
-              assert (In (child child2Idx ec2 ce2 c2pRq c2pRs pc2) (sys_objs impl))
-                by (simpl; tauto).
-              good_locking_get (child child2Idx ec2 ce2 c2pRq c2pRs pc2).
-              clear H6.
-              eapply upLockInvORq_rqUp_length_one_locked in H28; try reflexivity;
-                [|eapply findQ_length_ge_one; apply FirstMP_InMP; eassumption].
-              solve_rule_conds_ex.
-            }
-          * red in H7; red; simpl in *; mred.
+(*         split. *)
+(*         + apply Forall_app. *)
+(*           * apply forall_removeOnce. *)
+(*             eapply atomic_rqUp_preserves_msg_out_preds with (oidx:= child2Idx); *)
+(*               [exact msiSv_impl_ORqsInit *)
+(*               |exact msiSv_impl_RqRsSys|..]; eauto. *)
+(*             { intro; dest_in; discriminate. } *)
+(*             { red; auto. } *)
+(*             { exact msiSvMsgOutPred_good. } *)
+(*           * repeat (constructor; simpl). *)
+(*             red; repeat (simpl; mred). *)
+(*         + destruct H6; split. *)
+(*           * red in H6; red; simpl in *; mred; simpl. *)
+(*             destruct (oss@[child1Idx]) as [cost1|] eqn:Hcost1; simpl in *; [|auto]. *)
+(*             destruct (oss@[child2Idx]) as [cost2|] eqn:Hcost2; simpl in *; [|auto]. *)
+(*             destruct (orqs@[child1Idx]) as [corq1|] eqn:Hcorq1; simpl in *; [|auto]. *)
+(*             destruct (orqs@[child2Idx]) as [corq2|] eqn:Hcorq2; simpl in *; [|auto]. *)
+(*             destruct H6 as [[cv ?] ?]. *)
+(*             red in H6; dest. *)
+(*             unfold getDir in *; simpl in *. *)
+(*             disc_rule_conds_ex. *)
+(*             destruct H6 as [|[|]]; *)
+(*               [exfalso; solve_rule_conds_ex *)
+(*               | |exfalso; destruct H6 as [? [|]]; solve_rule_conds_ex]. *)
+(*             split. *)
+(*             { exists cv. *)
+(*               repeat ssplit. *)
+(*               { solve_rule_conds_ex. *)
+(*                 right; left; solve_msi. *)
+(*               } *)
+(*               { solve_rule_conds_ex. } *)
+(*               { solve_rule_conds_ex. } *)
+(*               { solve_rule_conds_ex. } *)
+(*             } *)
+(*             { disc_rule_conds_ex. *)
+(*               assert (In (child child2Idx ec2 ce2 c2pRq c2pRs pc2) (sys_objs impl)) *)
+(*                 by (simpl; tauto). *)
+(*               good_locking_get (child child2Idx ec2 ce2 c2pRq c2pRs pc2). *)
+(*               clear H6. *)
+(*               eapply upLockInvORq_rqUp_length_one_locked in H28; try reflexivity; *)
+(*                 [|eapply findQ_length_ge_one; apply FirstMP_InMP; eassumption]. *)
+(*               solve_rule_conds_ex. *)
+(*             } *)
+(*           * red in H7; red; simpl in *; mred. *)
 
-      - (** [parentEvictRqImmLastS] *)
-        disc_rule_conds_ex.
+(*       - (** [parentEvictRqImmLastS] *) *)
+(*         disc_rule_conds_ex. *)
 
-        split.
-        + apply Forall_app.
-          * apply forall_removeOnce.
-            eapply atomic_rqUp_preserves_msg_out_preds with (oidx:= child2Idx);
-              [exact msiSv_impl_ORqsInit
-              |exact msiSv_impl_RqRsSys|..]; eauto.
-            { intro; dest_in; discriminate. }
-            { red; auto. }
-            { exact msiSvMsgOutPred_good. }
-          * repeat (constructor; simpl).
-            red; repeat (simpl; mred).
-        + destruct H6; split.
-          * red in H6; red; simpl in *; mred; simpl.
-            destruct (oss@[child1Idx]) as [cost1|] eqn:Hcost1; simpl in *; [|auto].
-            destruct (oss@[child2Idx]) as [cost2|] eqn:Hcost2; simpl in *; [|auto].
-            destruct (orqs@[child1Idx]) as [corq1|] eqn:Hcorq1; simpl in *; [|auto].
-            destruct (orqs@[child2Idx]) as [corq2|] eqn:Hcorq2; simpl in *; [|auto].
-            destruct H6 as [[cv ?] ?].
-            red in H6; dest.
-            unfold getDir in *; simpl in *.
-            disc_rule_conds_ex.
-            destruct H6 as [|[|]];
-              [exfalso; solve_rule_conds_ex
-              | |exfalso; destruct H6 as [? [|]]; solve_rule_conds_ex].
-            split.
-            { exists cv.
-              repeat ssplit.
-              { solve_rule_conds_ex.
-                left; auto.
-              }
-              { solve_rule_conds_ex. }
-              { solve_rule_conds_ex. }
-              { solve_rule_conds_ex. }
-            }
-            { disc_rule_conds_ex.
-              assert (In (child child2Idx ec2 ce2 c2pRq c2pRs pc2) (sys_objs impl))
-                by (simpl; tauto).
-              good_locking_get (child child2Idx ec2 ce2 c2pRq c2pRs pc2).
-              clear H6.
-              eapply upLockInvORq_rqUp_length_one_locked in H28; try reflexivity;
-                [|eapply findQ_length_ge_one; apply FirstMP_InMP; eassumption].
-              solve_rule_conds_ex.
-            }
-          * red in H7; red; simpl in *; mred.
+(*         split. *)
+(*         + apply Forall_app. *)
+(*           * apply forall_removeOnce. *)
+(*             eapply atomic_rqUp_preserves_msg_out_preds with (oidx:= child2Idx); *)
+(*               [exact msiSv_impl_ORqsInit *)
+(*               |exact msiSv_impl_RqRsSys|..]; eauto. *)
+(*             { intro; dest_in; discriminate. } *)
+(*             { red; auto. } *)
+(*             { exact msiSvMsgOutPred_good. } *)
+(*           * repeat (constructor; simpl). *)
+(*             red; repeat (simpl; mred). *)
+(*         + destruct H6; split. *)
+(*           * red in H6; red; simpl in *; mred; simpl. *)
+(*             destruct (oss@[child1Idx]) as [cost1|] eqn:Hcost1; simpl in *; [|auto]. *)
+(*             destruct (oss@[child2Idx]) as [cost2|] eqn:Hcost2; simpl in *; [|auto]. *)
+(*             destruct (orqs@[child1Idx]) as [corq1|] eqn:Hcorq1; simpl in *; [|auto]. *)
+(*             destruct (orqs@[child2Idx]) as [corq2|] eqn:Hcorq2; simpl in *; [|auto]. *)
+(*             destruct H6 as [[cv ?] ?]. *)
+(*             red in H6; dest. *)
+(*             unfold getDir in *; simpl in *. *)
+(*             disc_rule_conds_ex. *)
+(*             destruct H6 as [|[|]]; *)
+(*               [exfalso; solve_rule_conds_ex *)
+(*               | |exfalso; destruct H6 as [? [|]]; solve_rule_conds_ex]. *)
+(*             split. *)
+(*             { exists cv. *)
+(*               repeat ssplit. *)
+(*               { solve_rule_conds_ex. *)
+(*                 left; auto. *)
+(*               } *)
+(*               { solve_rule_conds_ex. } *)
+(*               { solve_rule_conds_ex. } *)
+(*               { solve_rule_conds_ex. } *)
+(*             } *)
+(*             { disc_rule_conds_ex. *)
+(*               assert (In (child child2Idx ec2 ce2 c2pRq c2pRs pc2) (sys_objs impl)) *)
+(*                 by (simpl; tauto). *)
+(*               good_locking_get (child child2Idx ec2 ce2 c2pRq c2pRs pc2). *)
+(*               clear H6. *)
+(*               eapply upLockInvORq_rqUp_length_one_locked in H28; try reflexivity; *)
+(*                 [|eapply findQ_length_ge_one; apply FirstMP_InMP; eassumption]. *)
+(*               solve_rule_conds_ex. *)
+(*             } *)
+(*           * red in H7; red; simpl in *; mred. *)
 
-      - (** [parentEvictRqImmM] *)
-        disc_rule_conds_ex.
+(*       - (** [parentEvictRqImmM] *) *)
+(*         disc_rule_conds_ex. *)
 
-        split.
-        + apply Forall_app.
-          * apply forall_removeOnce.
-            eapply atomic_rqUp_preserves_msg_out_preds with (oidx:= child2Idx);
-              [exact msiSv_impl_ORqsInit
-              |exact msiSv_impl_RqRsSys|..]; eauto.
-            { intro; dest_in; discriminate. }
-            { red; auto. }
-            { exact msiSvMsgOutPred_good. }
-          * repeat (constructor; simpl).
-            red; repeat (simpl; mred).
-        + destruct H6; split.
-          * red in H6; red; simpl in *; mred; simpl.
-            destruct (oss@[child1Idx]) as [cost1|] eqn:Hcost1; simpl in *; [|auto].
-            destruct (oss@[child2Idx]) as [cost2|] eqn:Hcost2; simpl in *; [|auto].
-            destruct (orqs@[child1Idx]) as [corq1|] eqn:Hcorq1; simpl in *; [|auto].
-            destruct (orqs@[child2Idx]) as [corq2|] eqn:Hcorq2; simpl in *; [|auto].
-            destruct H6 as [[cv ?] ?].
-            red in H6; dest.
-            unfold getDir in *; simpl in *.
-            disc_rule_conds_ex.
-            destruct H6 as [|[|]]; try (exfalso; solve_rule_conds_ex; fail).
+(*         split. *)
+(*         + apply Forall_app. *)
+(*           * apply forall_removeOnce. *)
+(*             eapply atomic_rqUp_preserves_msg_out_preds with (oidx:= child2Idx); *)
+(*               [exact msiSv_impl_ORqsInit *)
+(*               |exact msiSv_impl_RqRsSys|..]; eauto. *)
+(*             { intro; dest_in; discriminate. } *)
+(*             { red; auto. } *)
+(*             { exact msiSvMsgOutPred_good. } *)
+(*           * repeat (constructor; simpl). *)
+(*             red; repeat (simpl; mred). *)
+(*         + destruct H6; split. *)
+(*           * red in H6; red; simpl in *; mred; simpl. *)
+(*             destruct (oss@[child1Idx]) as [cost1|] eqn:Hcost1; simpl in *; [|auto]. *)
+(*             destruct (oss@[child2Idx]) as [cost2|] eqn:Hcost2; simpl in *; [|auto]. *)
+(*             destruct (orqs@[child1Idx]) as [corq1|] eqn:Hcorq1; simpl in *; [|auto]. *)
+(*             destruct (orqs@[child2Idx]) as [corq2|] eqn:Hcorq2; simpl in *; [|auto]. *)
+(*             destruct H6 as [[cv ?] ?]. *)
+(*             red in H6; dest. *)
+(*             unfold getDir in *; simpl in *. *)
+(*             disc_rule_conds_ex. *)
+(*             destruct H6 as [|[|]]; try (exfalso; solve_rule_conds_ex; fail). *)
 
-            assert (In (child child2Idx ec2 ce2 c2pRq c2pRs pc2) (sys_objs impl))
-              by (simpl; tauto).
-            good_locking_get (child child2Idx ec2 ce2 c2pRq c2pRs pc2).
-            clear H26.
-            eapply upLockInvORq_rqUp_length_one_locked in H27; try reflexivity;
-              [|eapply findQ_length_ge_one; apply FirstMP_InMP; eassumption].
-            disc_rule_conds_ex.
+(*             assert (In (child child2Idx ec2 ce2 c2pRq c2pRs pc2) (sys_objs impl)) *)
+(*               by (simpl; tauto). *)
+(*             good_locking_get (child child2Idx ec2 ce2 c2pRq c2pRs pc2). *)
+(*             clear H26. *)
+(*             eapply upLockInvORq_rqUp_length_one_locked in H27; try reflexivity; *)
+(*               [|eapply findQ_length_ge_one; apply FirstMP_InMP; eassumption]. *)
+(*             disc_rule_conds_ex. *)
           
-            split.
-            { exists n.
-              repeat ssplit.
-              { solve_rule_conds_ex.
-                left; solve_msi.
-              }
-              { solve_rule_conds_ex; solve_msi. }
-              { solve_rule_conds_ex. }
-              { solve_rule_conds_ex. }
-            }
-            { solve_rule_conds_ex. }
-          * red in H7; red; simpl in *; mred.
+(*             split. *)
+(*             { exists n. *)
+(*               repeat ssplit. *)
+(*               { solve_rule_conds_ex. *)
+(*                 left; solve_msi. *)
+(*               } *)
+(*               { solve_rule_conds_ex; solve_msi. } *)
+(*               { solve_rule_conds_ex. } *)
+(*               { solve_rule_conds_ex. } *)
+(*             } *)
+(*             { solve_rule_conds_ex. } *)
+(*           * red in H7; red; simpl in *; mred. *)
 
-    Qed.
+(*     Qed. *)
 
-    Lemma implInv_init:
-      ImplInv (initsOf impl).
-    Proof.
-      red; simpl.
-      unfold implOStatesInit, implORqsInit; mred.
-      simpl.
-      repeat split.
-      exists 0.
-      repeat split; intros.
-      - vm_compute; intros.
-        right; left; auto.
-      - discriminate.
-      - discriminate.
-      - vm_compute; intros; auto.
-      - vm_compute; intros; auto.
-    Qed.
+(*     Lemma implInv_init: *)
+(*       ImplInv (initsOf impl). *)
+(*     Proof. *)
+(*       red; simpl. *)
+(*       unfold implOStatesInit, implORqsInit; mred. *)
+(*       simpl. *)
+(*       repeat split. *)
+(*       exists 0. *)
+(*       repeat split; intros. *)
+(*       - vm_compute; intros. *)
+(*         right; left; auto. *)
+(*       - discriminate. *)
+(*       - discriminate. *)
+(*       - vm_compute; intros; auto. *)
+(*       - vm_compute; intros; auto. *)
+(*     Qed. *)
 
-    Lemma implInv_invStep:
-      InvStep impl step_m ImplInv.
-    Proof.
-      apply invSeq_serializable_invStep.
-      - apply implInv_init.
-      - apply inv_trs_seqSteps.
-        apply msiSv_impl_InvTrs.
-      - eapply rqrs_Serializable.
-        + apply msiSv_impl_ORqsInit.
-        + apply msiSv_impl_RqRsSys.
-    Qed.
+(*     Lemma implInv_invStep: *)
+(*       InvStep impl step_m ImplInv. *)
+(*     Proof. *)
+(*       apply invSeq_serializable_invStep. *)
+(*       - apply implInv_init. *)
+(*       - apply inv_trs_seqSteps. *)
+(*         apply msiSv_impl_InvTrs. *)
+(*       - eapply rqrs_Serializable. *)
+(*         + apply msiSv_impl_ORqsInit. *)
+(*         + apply msiSv_impl_RqRsSys. *)
+(*     Qed. *)
 
-  End Facts.
+(*   End Facts. *)
   
-End Inv.
+(* End Inv. *)
 
-Hint Unfold ImplOStateM ImplOStateS ImplOStateI ImplOStateMSI
-     ImplDirM ImplDirS ImplDirI
-     ImplDirCoh ImplParentCoh ImplChildCoh1 ImplChildCoh2 ImplChildrenCoh
-     ImplStateCoh: RuleConds.
+(* Hint Unfold ImplOStateM ImplOStateS ImplOStateI ImplOStateMSI *)
+(*      ImplDirM ImplDirS ImplDirI *)
+(*      ImplDirCoh ImplParentCoh ImplChildCoh1 ImplChildCoh2 ImplChildrenCoh *)
+(*      ImplStateCoh: RuleConds. *)
 
 Close Scope list.
 Close Scope hvec.
